complete multicopy proofs

templates/multicopy/general_multicopy.v
@@ -7,7 +7,7 @@ From iris.proofmode Require Import tactics.
 From iris.heap_lang Require Import proofmode par.
 From iris.bi.lib Require Import fractional.
 Set Default Proof Using "All".
-Require Export KT_flows inset_flows_multicopy auth_ext.
+Require Export multiset_flows auth_ext.
 
 (** Algorithms **)
 
@@ -15,12 +15,10 @@ Variable inContents : val.
 Variable findNext : val.
 Variable lockLoc : Node → loc.
 Variable getLockLoc: val.
-(*Variable readClock: val.
-Variable incrementClock: val.*)
 Variable addContents: val.
-Variable set_next: val.
-Variable merge_contents: val.
-Variable allocNode: val.
+Variable mergeContents: val.
+Variable chooseNext: val.
+Variable atCapacity: val.
 
 Definition lockNode : val :=
   rec: "lockN" "x" :=
@@ -38,6 +36,13 @@ Definition traverse : val :=
   rec: "t_rec" "n" "k" :=
     lockNode "n" ;;
     let: "t" := inContents "n" "k" in
+    match: "t" with
+      SOME "t" => unlockNode "n";;
+                  "t"
+    | NONE => match: (findNext "n" "k") with
+                SOME "n'" => unlockNode "n" ;; "t_rec" "n'" "k"
+              | NONE => unlockNode "n" ;; #0 end end.
+(*              
     if: ("t" ≠ #0) 
     then
       unlockNode "n";; "t"
@@ -45,6 +50,7 @@ Definition traverse : val :=
       match: (findNext "n" "k") with
         SOME "n'" => unlockNode "n" ;; "t_rec" "n'" "k"
       | NONE => unlockNode "n" ;; #0 end.
+*)
               
 Definition search (r: Node) : val := 
   λ: "k", traverse #r "k".
@@ -68,25 +74,48 @@ Definition upsert (lc: loc) (r: Node) : val :=
       unlockNode #r;;
       "upsert_rec" "k".
 
+Definition compact : val :=
+  rec: "compact_rec" "n" :=
+    lockNode "n" ;;
+    if: atCapacity "n" then
+      let: "m" := chooseNext "n" in
+      lockNode "m" ;;
+      mergeContents "n" "m" ;;
+      unlockNode "n" ;;
+      unlockNode "m" ;;
+      "compact_rec" "m"
+    else
+      unlockNode "n".          
+
 
 (** Proof setup **)
 
 Definition K := Z.
-Definition KT := @KT K.
+Definition KT : Type := K * nat.
 Parameter KS : gset K.
 
 Definition esT : Type := gmap Node (gset K).
 Canonical Structure esRAC := leibnizO esT.
 
+Definition prod5O A B C D E :=
+  prodO (prodO (prodO (prodO A B) C) D) E.
+
+Definition per_node_gl :=
+    agreeR 
+      (prod5O gnameO gnameO gnameO gnameO (gmapO K gnameO)).
+
+Definition ghost_heapUR := gmapUR Node $ per_node_gl.  
+
 Definition contR := frac_agreeR (gmapUR K natUR).
-Definition flow_KTR := authR (KT_flowint_ur K).
-Definition flow_KR := authR (inset_flowint_ur K).
+Definition flow_KTR := authR (multiset_flowint_ur KT).
+Definition flow_KR := authR (multiset_flowint_ur K).
 Definition setR := authR (gsetUR Node).
 Definition esR := frac_agreeR (esRAC).
 Definition timeR := authR (max_natUR).
 Definition histR := authR (gsetUR (KT)).
-Definition hist_exclR := authR $ optionUR $ exclR (gsetUR KT).
+Definition hist_exclR := authR $ optionUR $ exclR (gsetO KT).
 Definition time_exclR := authR $ optionUR $ exclR natUR.
+Definition ghR := authR $ ghost_heapUR.
 
 Class multicopyG Σ := MULTICOPY {
                         multicopy_contG :> inG Σ contR;
@@ -98,19 +127,20 @@ Class multicopyG Σ := MULTICOPY {
                         multicopy_histG :> inG Σ histR;
                         multicopy_hist_exclG :> inG Σ hist_exclR;
                         multicopy_time_exclG :> inG Σ time_exclR;
+                        multicopy_ghG :> inG Σ ghR;
                        }.
 
 Definition multicopyΣ : gFunctors :=
   #[GFunctor contR; GFunctor flow_KTR; GFunctor flow_KR; GFunctor setR; 
     GFunctor esR; GFunctor timeR; GFunctor histR; GFunctor hist_exclR; 
-    GFunctor time_exclR ].
+    GFunctor time_exclR; GFunctor ghR ].
 
 Instance subG_multicopyΣ {Σ} : subG multicopyΣ Σ → multicopyG Σ.
 Proof. solve_inG. Qed.
 
 Section multicopy.
   Context {Σ} `{!heapG Σ, !multicopyG Σ}.
-  Context (N : namespace).
+(*  Context (N : namespace).*)
   Notation iProp := (iProp Σ).
   Local Notation "m !1 i" := (nzmap_total_lookup i m) (at level 20).
 
@@ -119,80 +149,110 @@ Section multicopy.
   Parameter node : Node → Node → esT → (gmap K natUR) → iProp.
 
   Parameter node_timeless_proof : ∀ r n es C, Timeless (node r n es C).
-  Instance node_timeless r n es C: Timeless (node r n es C).
+  Global Instance node_timeless r n es C: Timeless (node r n es C).
   Proof. apply node_timeless_proof. Qed.
 
-  Hypothesis node_sep_star: ∀ r n es C es' C',
+  Parameter node_sep_star: ∀ r n es C es' C',
     node r n es C ∗ node r n es' C' -∗ False.
 
-  Hypothesis node_edgeset_disjoint: ∀ r n es C,
+  Parameter node_edgeset_disjoint: ∀ r n es C,
     node r n es C -∗ ⌜∀ n1 n2, n1 ≠ n2 → es !!! n1 ∩ es !!! n2 = ∅⌝.  
 
-  Hypothesis node_edgeset_self_empty: ∀ r n es C,
-    node r n es C -∗ ⌜es !!! n = ∅⌝.
-
-  Definition out_edgeset_list (k: K) (esl : list (Node * gset K)) :=             
-    list_find (λ ns, k ∈ ns.2) esl.
-
-  Definition out_edgeset (k: K) (es: esT) : bool := 
-    match (out_edgeset_list k (map_to_list es)) with
-    | None => false
-    | _ => true end.
+  Parameter node_edgeset_empty_root_self: ∀ r n es C,
+    node r n es C -∗ ⌜es !!! r = ∅ ∧ es !!! n = ∅⌝.
 
   Definition inFP γ_f (n: Node) : iProp := own γ_f (◯ {[n]}).
 
   Definition closed γ_f (es: esT) : iProp := ∀ n, ⌜es !!! n  ≠ ∅⌝ → inFP γ_f n.
 
-  Definition inflow_zero (I: KT_flowint_ur K) := ∀ n, inset_KT I n = ∅. 
+  Definition inflow_zero (I: multiset_flowint_ur KT) := ∀ n, inset KT I n = ∅. 
 
-  Definition inflow_R (R: inset_flowint_ur K) r := 
-    ∀ n k, if n =? r then in_inset K k R n else ¬ in_inset K k R n. 
+  Definition outflow_zero (I: multiset_flowint_ur KT) := out_map I = ∅. 
 
-  Definition outflow_le_1 (I: KT_flowint_ur K) :=
+  Definition outflow_zero_R (I: multiset_flowint_ur K) := out_map I = ∅. 
+
+  Definition inflow_R (R: multiset_flowint_ur K) r := 
+    ∀ n k, k ∈ KS → if decide (n = r) then in_inset K k R n else ¬ in_inset K k R n. 
+
+  Definition outflow_le_1 (I: multiset_flowint_ur KT) :=
     ∀ n kt, out I n !1 kt ≤ 1.
 
-  Definition outflow_constraint_I (In: KT_flowint_ur K) (es: esT) 
-                          (Cn Bn: gmap K natUR) := 
-    ∀ n' k t, (k,t) ∈ outset_KT In n' ↔ 
-                          k ∈ es !!! n' ∧ (Cn !!! k = 0) ∧ (Bn !!! k = t).
-
-  Definition outflow_constraint_J (Jn: KT_flowint_ur K) (es: esT) 
-                          (Cn Bn: gmap K natUR) := 
-    ∀ n' k t, (k,t) ∈ outset_KT Jn n' ↔ 
-                          k ∈ es !!! n' ∧ (Cn !!! k = t) ∧ (Cn !!! k > 0).
-
-  Definition outflow_constraint_R (Rn: inset_flowint_ur K) (es: esT) n := 
-    ∀ n' k, in_outset K k Rn n' ↔ k ∈ es !!! n' ∧ in_inset K k Rn n.
+  Definition outflow_constraint_I (In: multiset_flowint_ur KT) (es: esT) 
+                          (Qn: gmap K natUR) := 
+    ∀ n' k t, k ∈ KS → ((k,t) ∈ outset KT In n' ↔ 
+                          k ∈ es !!! n' ∧ (Qn !! k = Some t)).
+                          
+  Definition outflow_constraint_R (Rn: multiset_flowint_ur K) (es: esT) n := 
+    ∀ n' k, k ∈ KS → (k ∈ outset K Rn n' ↔ k ∈ es !!! n' ∧ k ∈ inset K Rn n).
 
   Definition map_of_set (C: gset KT) : gmap K nat := 
-              let f := λ (kt: KT) (M: gmap K nat), if (M !!! kt.1 <=? kt.2) 
-                                 then (<[kt.1 := kt.2]> M : gmap K nat) else M in
+              let f := λ (kt: KT) (M: gmap K nat), 
+                         if (decide (M !!! kt.1 <= kt.2)) 
+                         then (<[kt.1 := kt.2]> M : gmap K nat) else M in
               set_fold f (∅: gmap K nat) C.
 
   Definition set_of_map (C: gmap K nat) : gset KT := 
              let f := λ k t H, H ∪ {[(k,t)]} in
              map_fold f (∅: gset KT) C.
 
-  Definition φ0 (Bn: gmap K natUR) (T: nat) := 
-              ∀ k, Bn !!! k ≤ T.  
+  (** ϕ_1 in the paper *)
+  Definition φ0 (es: esT) (Qn: gmap K natUR) :=
+              ∀ k, k ∈ KS → ((∀ n', k ∉ es !!! n') → Qn !! k = None).
 
-  Definition φ1 (Bn Cn: gmap K natUR) (In: KT_flowint_ur K) := 
-              ∀ k, out_KT In k ∨ (Bn !!! k = Cn !!! k).
+  (** This constraint is implicit in the paper. We track B_n 
+      explicitly as ghost state here. That is the following 
+      captures the definition of B_n in terms of C_n/Q_n given 
+      in the paper. *)
+  Definition φ1 (Bn Cn Qn: gmap K natUR) := 
+              ∀ k t, k ∈ KS → ((Cn !! k = Some t → Bn !! k = Some t)
+                 ∧ (Cn !! k = None → Bn !! k = Qn !! k)). 
 
+  (** ϕ_2 in the paper *)
   Definition φ2 n (Bn: gmap K natUR) In := 
-              ∀ k t, (k,t) ∈ inset_KT In n → Bn !!! k = t.
+              ∀ k t, k ∈ KS → ((k,t) ∈ inset KT In n → Bn !!! k = t).
 
-  Definition φ3 n (Bn: gmap K natUR) Jn :=
-              ∀ k t, (k,t) ∈ inset_KT Jn n → Bn !!! k ≤ t.
+  (** ϕ_4 in the paper *)
+  Definition φ3 n (Bn: gmap K natUR) Rn :=
+              ∀ k, k ∈ KS → (Bn !! k = None ∨ k ∈ inset K Rn n).
 
-  Definition φ4 n (Bn: gmap K natUR) Rn :=
-              ∀ k, Bn !!! k = 0 ∨ in_inset K k Rn n.
-
-  Definition φ5 n (Rn: inset_flowint_ur K) := 
+  (** ϕ_5 in the paper *)
+  Definition φ4 n (Rn: multiset_flowint_ur K) := 
               ∀ k, inf Rn n !1 k ≤ 1.
+
+  (** ϕ_3 in the paper *)
+  Definition φ5 (Bn Qn: gmap K natUR) :=
+              ∀ k, k ∈ KS → (Qn !!! k ≤ Bn !!! k).            
+
+  Definition φ6 (Bn: gmap K natUR) (t: nat) := 
+              ∀ k, k ∈ KS → (Bn !!! k ≤ t).
+  
+  Definition φ7 n (es: esT) (Rn: multiset_flowint_ur K) (Qn: gmap K natUR) :=
+              ∀ k, k ∈ KS → ((∃ n', k ∈ es !!! n') ∧ k ∈ inset K Rn n 
+                          → k ∈ dom (gset K) Qn).              
+
+  Definition φ8 (n: Node) (In: multiset_flowint_ur KT) := 
+              ∀ kt, inf In n !1 kt ≤ 1.
+
 
   Definition maxTS (t: nat) (H: gset KT) := 
               (∀ (k: K) t', (k, t') ∈ H → t' < t) ∧ (t > 0).
+  
+  Definition f_merge (Cn: gmap K nat) (Es: gset K) (Cm: gmap K nat) := 
+                    λ k o1 o2, 
+                      if (decide (Cn !! k ≠ None)) then o1
+                      else if (decide (k ∈ Es)) then o2 
+                           else (None: option nat).
+  
+  Global Instance f_merge_diag_none Cn Es Cm k : DiagNone (f_merge Cn Es Cm k).
+  Proof.
+    unfold DiagNone. unfold f_merge.
+    destruct (decide (Cn !! k ≠ None)); try by simpl.
+    destruct (decide (k ∈ Es)); try by simpl.
+  Qed.  
+  
+  Definition merge (Cn: gmap K nat) (Es: gset K) (Cm: gmap K nat) 
+                          : (gmap K nat) :=
+             gmap_imerge (f_merge Cn Es Cm) Cn Cm.            
 
   Definition MCS_auth (γ_te γ_he: gname) (t: nat) (H: gset KT) : iProp := 
       own γ_te (● Excl' t) ∗ own γ_he (● Excl' H).
@@ -200,121 +260,112 @@ Section multicopy.
   Definition MCS (γ_te γ_he: gname) (t: nat) (H: gset KT) : iProp := 
       own γ_te (◯ Excl' t) ∗ own γ_he (◯ Excl' H).
 
-  Definition frac_ghost_state γ_e γ_c γ_b (n: Node) es 
-                                  (Cn Bn: gmap K natUR): iProp :=
-      own (γ_e(n)) (to_frac_agree (1/2) (es))
-    ∗ own (γ_c(n)) (to_frac_agree (1/2) (Cn))
-    ∗ own (γ_b(n)) (to_frac_agree (1/2) (Bn)).
+  Definition frac_ghost_state γ_en γ_cn γ_bn γ_qn es 
+                                  (Cn Bn Qn: gmap K natUR): iProp :=
+      own (γ_en) (to_frac_agree (1/2) (es))
+    ∗ own (γ_cn) (to_frac_agree (1/2) (Cn))
+    ∗ own (γ_bn) (to_frac_agree (1/2) (Bn))
+    ∗ own (γ_qn) (to_frac_agree (1/2) (Qn)).
 
-  Definition singleton_interfaces_ghost_state γ_I γ_J γ_R n 
-                  (In Jn: KT_flowint_ur K) (Rn: inset_flowint_ur K) : iProp :=
+  Definition singleton_interfaces_ghost_state (γ_I γ_R: gname) (n: Node) 
+                  (In: multiset_flowint_ur KT) (Rn: multiset_flowint_ur K) : iProp :=
       own γ_I (◯ In)
-    ∗ own γ_J (◯ Jn)
     ∗ own γ_R (◯ Rn)
     ∗ ⌜domm In = {[n]}⌝
-    ∗ ⌜domm Jn = {[n]}⌝
     ∗ ⌜domm Rn = {[n]}⌝.
     
-  Definition outflow_constraints n In Jn Rn es Cn Bn : iProp :=
-      ⌜outflow_constraint_I In es Cn Bn⌝
-    ∗ ⌜outflow_constraint_J Jn es Cn Bn⌝
+  Definition outflow_constraints n In Rn es Qn : iProp :=
+      ⌜outflow_constraint_I In es Qn⌝
     ∗ ⌜outflow_constraint_R Rn es n⌝
-    ∗ ⌜outflow_le_1 In⌝
-    ∗ ⌜outflow_le_1 Jn⌝.
+    ∗ ⌜outflow_le_1 In⌝.
 
   Definition clock lc (t: nat) : iProp := lc ↦ #t.
   
-  Definition history_init (H: gset KT) : iProp := ⌜∀ k, k ∈ KS → (k, 0) ∈ H⌝.
-      
-  Definition nodePred γ_e γ_c γ_b γ_t γ_s lc r n (Cn Bn : gmap K natUR) : iProp :=
-    ∃ es t,
-      node r n es Cn
-    ∗ frac_ghost_state γ_e γ_c γ_b n es Cn Bn 
-    ∗ own γ_s (◯ set_of_map Cn)
-    ∗ (if (n =? r) then own γ_t (●{1/2} MaxNat t) ∗ clock lc t else ⌜True⌝)%I.
+  Definition history_init (H: gset KT) := ∀ k, k ∈ KS → (k, 0) ∈ H.
 
-  Definition nodeShared γ_I γ_J γ_R γ_e γ_c γ_b γ_f γ_cir
-                              r n (Cn Bn : gmap K natUR) t H : iProp :=
-    ∃ es In Jn Rn,                          
-      frac_ghost_state γ_e γ_c γ_b n es Cn Bn    
-    ∗ singleton_interfaces_ghost_state γ_I γ_J γ_R n In Jn Rn
+  Definition ghost_loc γ_en γ_cn γ_bn γ_qn (γ_cirn: gmap K gnameO) : per_node_gl := 
+        to_agree (γ_en, γ_cn, γ_bn, γ_qn, γ_cirn).
+
+  (** Predicate N_L *)
+  Definition nodePred γ_gh γ_t γ_s lc r n (Cn Bn Qn : gmap K natUR) : iProp :=
+    ∃ γ_en γ_cn γ_bn γ_qn γ_cirn es t,
+      node r n es Cn
+    ∗ own γ_gh (◯ {[n := ghost_loc γ_en γ_cn γ_bn γ_qn γ_cirn]})  
+    ∗ frac_ghost_state γ_en γ_cn γ_bn γ_qn es Cn Bn Qn
+    ∗ own γ_s (◯ set_of_map Cn)
+    ∗ (if decide (n = r) then own γ_t (●{1/2} MaxNat t) ∗ clock lc t else ⌜True⌝)%I.
+
+  (** Predicate N_S *)
+  Definition nodeShared (γ_I γ_R γ_f: gname) γ_gh r n 
+          (Cn Bn Qn : gmap K natUR) H t: iProp :=
+    ∃ γ_en γ_cn γ_bn γ_qn γ_cirn es In Rn,
+      own γ_gh (◯ {[n := ghost_loc γ_en γ_cn γ_bn γ_qn γ_cirn]})
+    ∗ frac_ghost_state γ_en γ_cn γ_bn γ_qn es Cn Bn Qn  
+    ∗ singleton_interfaces_ghost_state γ_I γ_R n In Rn 
     ∗ inFP γ_f n
     ∗ closed γ_f es
-    ∗ outflow_constraints n In Jn Rn es Cn Bn
-    ∗ (if (n =? r) then ⌜Bn = map_of_set H⌝ ∗ ⌜inflow_zero In⌝ ∗ ⌜inflow_zero Jn⌝ 
-                   else True)%I
-    ∗ ([∗ set] k ∈ KS, own (γ_cir n k) (● (MaxNat (Bn !!! k))))
-    ∗ ⌜φ0 Bn t⌝ ∗ ⌜φ1 Bn Cn In⌝ ∗ ⌜φ2 n Bn In⌝ 
-    ∗ ⌜φ3 n Bn Jn⌝ ∗ ⌜φ4 n Bn Rn⌝ ∗ ⌜φ5 n Rn⌝. 
-    
-  Definition global_state γ_te γ_he γ_s γ_t γ_I γ_J γ_R γ_f r t H I J R : iProp :=
+    ∗ outflow_constraints n In Rn es Qn
+    ∗ (if decide (n = r) then ⌜Bn = map_of_set H⌝ ∗ ⌜inflow_zero In⌝ else True)%I
+    ∗ ([∗ set] k ∈ KS, own (γ_cirn !!! (k)) (● (MaxNat (Bn !!! k))))
+    ∗ ⌜φ0 es Qn⌝ ∗ ⌜φ1 Bn Cn Qn⌝ ∗ ⌜φ2 n Bn In⌝ ∗ ⌜φ3 n Bn Rn⌝ 
+    ∗ ⌜φ4 n Rn⌝ ∗ ⌜φ5 Bn Qn⌝ ∗ ⌜φ6 Bn t⌝ ∗ ⌜φ7 n es Rn Qn⌝ ∗ ⌜φ8 n In⌝. 
+
+  (** Predicate G *)
+  Definition global_state (γ_te γ_he γ_s γ_t γ_I γ_R γ_f γ_gh: gname) 
+          (r: Node) (t: nat) (H: gset KT) 
+          (hγ: gmap Node per_node_gl) (I: multiset_flowint_ur KT) 
+          (R: multiset_flowint_ur K) : iProp :=
       MCS_auth γ_te γ_he t H
-    ∗ own γ_s (● H) ∗ (history_init H)
+    ∗ own γ_s (● H) ∗ ⌜history_init H⌝
     ∗ own γ_t (●{1/2} MaxNat t)
-    ∗ own γ_I (● I)
-    ∗ own γ_J (● J)
-    ∗ own γ_R (● R)
+    ∗ own γ_I (● I) ∗ ⌜outflow_zero I⌝
+    ∗ own γ_R (● R) ∗ ⌜outflow_zero_R R⌝ ∗ ⌜inflow_R R r⌝
     ∗ own γ_f (● domm I)
-    ∗ ⌜inflow_zero I⌝ ∗ ⌜inflow_zero J⌝ ∗ ⌜inflow_R R r⌝
+    ∗ own γ_gh (● hγ)
     ∗ inFP γ_f r
     ∗ ⌜maxTS t H⌝
-    ∗ ⌜domm I = domm J⌝ ∗ ⌜domm I = domm R⌝.
+    ∗ ⌜domm I = domm R⌝ ∗ ⌜domm I = dom (gset Node) hγ⌝.
 
-  Definition mcs γ_te γ_he γ_s γ_t γ_I γ_J γ_R γ_f γ_e γ_c γ_b γ_cir lc r : iProp :=
-    ∃ t (H: gset KT) (I J: KT_flowint_ur K) (R: inset_flowint_ur K),
-      global_state γ_te γ_he γ_s γ_t γ_I γ_J γ_R γ_f r t H I J R
-    ∗ ([∗ set] n ∈ (domm I), ∃ (bn: bool) Cn Bn, 
-          lockLoc n ↦ #bn
-        ∗ (if bn then True else nodePred γ_e γ_c γ_b γ_t γ_s lc r n Cn Bn)
-        ∗ nodeShared γ_I γ_J γ_R γ_e γ_c γ_b γ_f γ_cir r n Cn Bn t H)%I.  
+  (** Invariant Inv *)
+  Definition mcs γ_te γ_he γ_s γ_t γ_I γ_R γ_f γ_gh lc r : iProp :=
+    ∃ t (H: gset KT) hγ
+      (I: multiset_flowint_ur KT) (R: multiset_flowint_ur K),
+      global_state γ_te γ_he γ_s γ_t γ_I γ_R γ_f γ_gh r t H hγ I R
+    ∗ ([∗ set] n ∈ (domm I), ∃ (bn: bool) Cn Bn Qn, 
+          lockLoc n ↦ #bn  
+        ∗ (if bn then True else nodePred γ_gh γ_t γ_s lc r n Cn Bn Qn)
+        ∗ nodeShared γ_I γ_R γ_f γ_gh r n Cn Bn Qn H t)%I.  
 
-  Instance mcs_timeless γ_te γ_he γ_s γ_t γ_I γ_J γ_R γ_f γ_e γ_c γ_b γ_cir lc r :
-    Timeless (mcs γ_te γ_he γ_s γ_t γ_I γ_J γ_R γ_f γ_e γ_c γ_b γ_cir lc r).
-  Proof. Admitted.
+  Global Instance mcs_timeless γ_te γ_he γ_s γ_t γ_I γ_R γ_f γ_gh lc r :
+    Timeless (mcs γ_te γ_he γ_s γ_t γ_I γ_R γ_f γ_gh lc r).
+  Proof.
+    rewrite /mcs.
+    repeat (apply bi.exist_timeless; intros).
+    repeat apply bi.sep_timeless; try apply _.
+    apply big_sepS_timeless.
+    repeat (intros; apply bi.exist_timeless; intros).
+    apply bi.sep_timeless; try apply _.
+    repeat apply bi.sep_timeless; try apply _.
+    destruct x5; try apply _.
+    repeat (apply bi.exist_timeless; intros).
+    repeat apply bi.sep_timeless; try apply _.
+    destruct (decide (x4 = r)); try apply _.
+    repeat (apply bi.exist_timeless; intros).
+    repeat apply bi.sep_timeless; try apply _.
+    destruct (decide (x4 = r)); try apply _.
+  Qed.
 
-  Definition mcs_inv γ_te γ_he γ_s γ_t γ_I γ_J γ_R γ_f γ_e γ_c γ_b γ_cir lc r := 
-    inv N (mcs γ_te γ_he γ_s γ_t γ_I γ_J γ_R γ_f γ_e γ_c γ_b γ_cir lc r).
-
+  Definition mcs_inv N γ_te γ_he γ_s γ_t γ_I γ_R γ_f γ_gh lc r := 
+    inv N (mcs γ_te γ_he γ_s γ_t γ_I γ_R γ_f γ_gh lc r).
+  
   (** Helper functions Spec **)
-
-  Lemma lockNode_spec (n: Node):
-    ⊢ <<< ∀ (b: bool), (lockLoc n) ↦ #b >>>
-      lockNode #n    @ ⊤
-    <<< (lockLoc n) ↦ #true ∗ ⌜b = false⌝ , RET #() >>>.
-  Proof.
-  Admitted.
-
-  Lemma unlockNode_spec (n: Node) :
-    ⊢ <<< lockLoc n ↦ #true >>>
-      unlockNode #n    @ ⊤
-    <<< lockLoc n ↦ #false, RET #() >>>.
-  Proof.
-  Admitted.
-
-  Lemma lockNode_spec_high γ_te γ_he γ_s γ_t γ_I γ_J γ_R 
-                                      γ_f γ_e γ_c γ_b γ_cir lc r n:
-    ⊢ mcs_inv γ_te γ_he γ_s γ_t γ_I γ_J γ_R γ_f γ_e γ_c γ_b γ_cir lc r -∗
-        inFP γ_f n -∗
-              <<< True >>>
-                lockNode #n    @ ⊤ ∖ ↑N
-              <<< ∃ Cn Bn, nodePred γ_e γ_c γ_b γ_t γ_s lc r n Cn Bn, RET #() >>>.
-  Proof.
-  Admitted.
-
-  Lemma unlockNode_spec_high γ_te γ_he γ_s γ_t γ_I γ_J γ_R 
-                                        γ_f γ_e γ_c γ_b γ_cir lc r n Cn Bn:
-    ⊢ mcs_inv γ_te γ_he γ_s γ_t γ_I γ_J γ_R γ_f γ_e γ_c γ_b γ_cir lc r -∗
-        inFP γ_f n -∗ nodePred γ_e γ_c γ_b γ_t γ_s lc r n Cn Bn -∗
-              <<< True >>>
-                unlockNode #n    @ ⊤ ∖ ↑N
-              <<< True, RET #() >>>.
-  Proof.
-  Admitted.
-
+    
   Parameter inContents_spec : ∀ r n es (Cn: gmap K natUR) (k: K),
      ⊢ ({{{ node r n es Cn }}}
            inContents #n #k
-       {{{ (t: nat), RET #t; node r n es Cn ∗ ⌜Cn !!! k = t⌝ }}})%I.
+       {{{ (t: option nat), 
+              RET (match t with Some t => SOMEV #t | None => NONEV end);
+                  node r n es Cn ∗ ⌜Cn !! k = t⌝ }}})%I.
 
   Parameter findNext_spec : ∀ r n es (Cn: gmap K natUR) (k: K),
      ⊢ ({{{ node r n es Cn }}}
@@ -356,7 +407,7 @@ Section multicopy.
       apply f_equal. lia. }
     iEval (rewrite H') in "Hc".
     iFrame. by iModIntro.
-  Qed.         
+  Qed.
 
   Parameter addContents_spec : ∀ r es (Cn: gmap K natUR) (k: K) (t:nat),
      ⊢ ({{{ node r r es Cn }}}
@@ -366,49 +417,44 @@ Section multicopy.
                   node r r es Cn' ∗ if succ then ⌜Cn' = <[k := t]> Cn⌝ 
                                 else ⌜Cn' = Cn⌝ }}})%I.
 
+  Parameter atCapacity_spec : ∀ r n es (Cn: gmap K natUR),
+     ⊢ ({{{ node r n es Cn }}}
+           atCapacity #n
+       {{{ (b: bool), RET #b;
+           node r n es Cn ∗ ⌜b = true ∨ b = false⌝ }}})%I.
+           
+  Parameter chooseNext_spec : ∀ r n esn (Cn: gmap K natUR),
+     ⊢ ({{{ node r n esn Cn }}}
+           chooseNext #n
+       {{{ (m: Node) (esn' esm: esT) Cm, RET #m;
+           node r n esn' Cn ∗ ⌜esn' !!! m ≠ ∅⌝
+           ∗ (  ⌜esn' = esn⌝ 
+              ∨ ⌜esn' = <[m := (esn' !!! m)]> esn⌝ 
+                ∗ node r m esm Cm 
+                ∗ lockLoc m ↦ #false
+                ∗ ⌜Cm = ∅⌝ 
+                ∗ ⌜esm = ∅⌝) }}})%I.
+
+  Parameter mergeContents_spec : ∀ r n m esn esm (Cn Cm: gmap K natUR),
+     ⊢ ({{{ node r n esn Cn ∗ node r m esm Cm ∗ ⌜esn !!! m ≠ ∅⌝ }}}
+           mergeContents #n #m
+       {{{ Cn' Cm', RET #m;
+           node r n esn Cn' ∗ node r m esm Cm' 
+           ∗ ⌜set_of_map Cn' ⊆ set_of_map Cn⌝
+           ∗ ⌜set_of_map Cm' ⊆ set_of_map Cn ∪ set_of_map Cm⌝
+           ∗ ⌜set_of_map Cn ∩ set_of_map Cm' ## set_of_map Cn'⌝
+           ∗ ⌜dom (gset K) Cm ⊆ dom (gset K) Cm'⌝
+           ∗ ⌜merge Cn (esn !!! m) Cm = merge Cn' (esn !!! m) Cm'⌝ }}})%I.
+
   (** Useful lemmas and definitions **)
 
-(*
-  Instance test r n γ_t T : Laterable (if n =? r then 
-                                            own γ_t (●{1 / 2} T) else ⌜True⌝)%I.
+  Global Instance HnP_t_laterable (r n: Node) γ_t lc T : 
+              Laterable (if decide (n = r) 
+                         then own γ_t (●{1 / 2} MaxNat T) ∗ clock lc T 
+                         else ⌜True⌝)%I.
   Proof.
-    destruct (n =? r); try done.
-  Admitted.
-*)
-
-  Lemma out_edgeset_true k : ∀ es, out_edgeset k es = true → ∃ n, k ∈ es !!! n.
-  Proof.
-    intros es Hes.
-    unfold out_edgeset in Hes.
-    destruct (out_edgeset_list k (map_to_list es)) 
-      as [ (i, (n,s)) | ] eqn: E; try inversion Hes.
-    unfold out_edgeset_list in E.
-    rewrite list_find_Some in E *; intros E.
-    destruct E as [E1 [E2 _]].
-    simpl in E2. apply elem_of_list_lookup_2 in E1.
-    apply elem_of_map_to_list in E1.
-    exists n. rewrite /(es !!! n). 
-    unfold finmap_lookup_total. rewrite E1. by simpl.
+    destruct (decide (n = r)); apply timeless_laterable; apply _.
   Qed.
-      
-  Lemma out_edgeset_false k : ∀ es, out_edgeset k es = false → ∀ n, k ∉ es !!! n.
-  Proof.
-    intros es Hes n.
-    unfold out_edgeset in Hes.
-    destruct (out_edgeset_list k (map_to_list es)) 
-      as [ p | ] eqn: E; try inversion Hes.
-    unfold out_edgeset_list in E.
-    rewrite list_find_None in E *; intros E.
-    rewrite Forall_forall in E *; intros E.
-    rewrite /(es !!! n). 
-    unfold finmap_lookup_total.
-    destruct (es !! n) eqn:F.
-    - rewrite F. simpl.
-      rewrite <-(elem_of_map_to_list es n g) in F.
-      pose proof E (n, g) F as E. by simpl in E.
-    - rewrite F. simpl. set_solver.
-  Qed.    
-
 
   Lemma inFP_domm γ_f n D : inFP γ_f n -∗ own γ_f (● D) -∗ ⌜n ∈ D⌝.
   Proof.
@@ -420,37 +466,105 @@ Section multicopy.
     apply gset_included in H'.
     iPureIntro. set_solver.
   Qed.
-  
-  Lemma frac_eq γ_e γ_c γ_b n es Cn Bn es' Cn' Bn' : 
-              frac_ghost_state γ_e γ_c γ_b n es Cn Bn -∗
-                  frac_ghost_state γ_e γ_c γ_b n es' Cn' Bn'-∗ 
-                    ⌜es = es'⌝ ∗ ⌜Cn = Cn'⌝ ∗ ⌜Bn = Bn'⌝.
+
+  Lemma own_alloc_set (S: gset K): True ==∗ 
+          ∃ (γ: gmap K gname), ([∗ set] k ∈ S, own (γ !!! k) (● (MaxNat 0))).
+  Proof.
+    iIntros "_".
+    iInduction S as [| s S] "IH" using set_ind_L.
+    - iModIntro. iExists _. try done.
+    - iMod (own_alloc (● (MaxNat 0))) as (γs)"H'".
+      { rewrite auth_auth_valid. try done. }
+      iDestruct "IH" as ">IH".
+      iDestruct "IH" as (γ)"IH". 
+      iModIntro. iExists (<[s := γs]> γ).
+      rewrite (big_sepS_delete _ ({[s]} ∪ S) s); last by set_solver.
+      iSplitL "H'". by rewrite lookup_total_insert.
+      assert (({[s]} ∪ S) ∖ {[s]} = S) as HS. set_solver.
+      rewrite HS. 
+      iApply (big_sepS_mono 
+                  (λ y, own (γ !!! y) (● {| max_nat_car := 0 |}) )%I
+                  (λ y, own (<[s:=γs]> γ !!! y) (● {| max_nat_car := 0 |}))%I
+                  S); try done.
+      intros k k_in_S. iFrame. iIntros "H'".
+      rewrite lookup_total_insert_ne; last by set_solver. 
+      done.
+      (* No idea what is happening here *) 
+      Unshelve. exact (∅: gmap K gname).
+  Qed.
+
+  Lemma ghost_heap_sync γ_gh n γ_en γ_cn γ_bn γ_qn γ_cirn 
+                                      γ_en' γ_cn' γ_bn' γ_qn' γ_cirn' : 
+    own γ_gh (◯ {[n := ghost_loc γ_en γ_cn γ_bn γ_qn γ_cirn]}) 
+      -∗ own γ_gh (◯ {[n := ghost_loc γ_en' γ_cn' γ_bn' γ_qn' γ_cirn']}) 
+          -∗ ⌜γ_en = γ_en'⌝ ∗ ⌜γ_cn = γ_cn'⌝ ∗ ⌜γ_bn = γ_bn'⌝ 
+             ∗ ⌜γ_qn = γ_qn'⌝ ∗ ⌜γ_cirn = γ_cirn'⌝.
+  Proof.
+    iIntros "H1 H2". iCombine "H1" "H2" as "H".
+    iPoseProof (own_valid with "H") as "Valid".
+    iDestruct "Valid" as %Valid.
+    rewrite auth_frag_valid in Valid *; intros Valid.
+    apply singleton_valid in Valid.
+    apply to_agree_op_inv in Valid.
+    apply leibniz_equiv in Valid.
+    inversion Valid.
+    by iPureIntro.
+  Qed.
+
+  Lemma ghost_heap_update γ_gh (hγ: gmap Node per_node_gl) n 
+                                γ_en γ_cn γ_bn γ_qn γ_cirn :
+    ⌜n ∉ dom (gset Node) hγ⌝ -∗ 
+          own γ_gh (● hγ) ==∗ 
+            own γ_gh (● <[n := ghost_loc γ_en γ_cn γ_bn γ_qn γ_cirn]> hγ)
+          ∗ own γ_gh (◯ {[n := ghost_loc γ_en γ_cn γ_bn γ_qn γ_cirn]}).
+  Proof.
+    iIntros "%". rename H into n_notin_hγ.
+    iIntros "Hown". set (<[ n := ghost_loc γ_en γ_cn γ_bn γ_qn γ_cirn ]> hγ) as hγ'.
+    iDestruct (own_update _ _ 
+        (● hγ' ⋅ ◯ {[ n := ghost_loc γ_en γ_cn γ_bn γ_qn γ_cirn ]})
+               with "Hown") as "Hown".
+    { apply auth_update_alloc. 
+      rewrite /hγ'.
+      apply alloc_local_update; last done.
+      by rewrite <-not_elem_of_dom. }
+    iMod (own_op with "Hown") as "[Ht● Ht◯]".
+    iModIntro. iFrame.
+  Qed.    
+
+  Lemma frac_eq γ_e γ_c γ_b γ_q es Cn Bn Qn es' Cn' Bn' Qn' : 
+              frac_ghost_state γ_e γ_c γ_b γ_q es Cn Bn Qn -∗
+                  frac_ghost_state γ_e γ_c γ_b γ_q es' Cn' Bn' Qn' -∗ 
+                    ⌜es = es'⌝ ∗ ⌜Cn = Cn'⌝ ∗ ⌜Bn = Bn'⌝ ∗ ⌜Qn = Qn'⌝.
   Proof.
     iIntros "H1 H2". unfold frac_ghost_state.
-    iDestruct "H1" as "(H1_es & H1_c & H1_b)".
-    iDestruct "H2" as "(H2_es & H2_c & H2_b)".
+    iDestruct "H1" as "(H1_es & H1_c & H1_b & H1_q)".
+    iDestruct "H2" as "(H2_es & H2_c & H2_b & H2_q)".
     iPoseProof (own_valid_2 _ _ _ with "[$H1_es] [$H2_es]") as "Hes".
     iPoseProof (own_valid_2 _ _ _ with "[$H1_c] [$H2_c]") as "Hc".
     iPoseProof (own_valid_2 _ _ _ with "[$H1_b] [$H2_b]") as "Hb".
-    iDestruct "Hes" as %Hes. iDestruct "Hc" as %Hc. iDestruct "Hb" as %Hb.
+    iPoseProof (own_valid_2 _ _ _ with "[$H1_q] [$H2_q]") as "Hq".
+    iDestruct "Hes" as %Hes. iDestruct "Hc" as %Hc.
+    iDestruct "Hb" as %Hb. iDestruct "Hq" as %Hq.
     apply frac_agree_op_valid in Hes. destruct Hes as [_ Hes].
     apply frac_agree_op_valid in Hc. destruct Hc as [_ Hc].
     apply frac_agree_op_valid in Hb. destruct Hb as [_ Hb].
+    apply frac_agree_op_valid in Hq. destruct Hq as [_ Hq].
     apply leibniz_equiv_iff in Hes.
     apply leibniz_equiv_iff in Hc. 
     apply leibniz_equiv_iff in Hb.
+    apply leibniz_equiv_iff in Hq.
     iPureIntro. repeat split; try done.   
   Qed.
 
-  Lemma frac_update γ_e γ_c γ_b r es Cr Br es' Cr' Br' : 
-              frac_ghost_state γ_e γ_c γ_b r es Cr Br ∗ 
-                 frac_ghost_state γ_e γ_c γ_b r es Cr Br ==∗ 
-                      frac_ghost_state γ_e γ_c γ_b r es' Cr' Br' ∗ 
-                        frac_ghost_state γ_e γ_c γ_b r es' Cr' Br'.
+  Lemma frac_update γ_e γ_c γ_b γ_q es Cn Bn Qn es' Cn' Bn' Qn' : 
+              frac_ghost_state γ_e γ_c γ_b γ_q es Cn Bn Qn ∗ 
+                 frac_ghost_state γ_e γ_c γ_b γ_q es Cn Bn Qn ==∗ 
+                      frac_ghost_state γ_e γ_c γ_b γ_q es' Cn' Bn' Qn' ∗ 
+                        frac_ghost_state γ_e γ_c γ_b γ_q es' Cn' Bn' Qn'.
   Proof.
     iIntros "(H1 & H2)". 
-    iDestruct "H1" as "(H1_es & H1_c & H1_b)".
-    iDestruct "H2" as "(H2_es & H2_c & H2_b)".
+    iDestruct "H1" as "(H1_es & H1_c & H1_b & H1_q)".
+    iDestruct "H2" as "(H2_es & H2_c & H2_b & H2_q)".
     iCombine "H1_es H2_es" as "Hes". 
     iEval (rewrite <-frac_agree_op) in "Hes". 
     iEval (rewrite Qp_half_half) in "Hes". 
@@ -460,7 +574,10 @@ Section multicopy.
     iCombine "H1_b H2_b" as "Hb". 
     iEval (rewrite <-frac_agree_op) in "Hb". 
     iEval (rewrite Qp_half_half) in "Hb".
-    iMod ((own_update (γ_e r) (to_frac_agree 1 es) 
+    iCombine "H1_q H2_q" as "Hq". 
+    iEval (rewrite <-frac_agree_op) in "Hq". 
+    iEval (rewrite Qp_half_half) in "Hq".
+    iMod ((own_update (γ_e) (to_frac_agree 1 es) 
                   (to_frac_agree 1 es')) with "[$Hes]") as "Hes".
     { apply cmra_update_exclusive. 
       unfold valid, cmra_valid. simpl. unfold prod_valid.
@@ -468,24 +585,33 @@ Section multicopy.
     iEval (rewrite <-Qp_half_half) in "Hes".
     iEval (rewrite frac_agree_op) in "Hes".  
     iDestruct "Hes" as "(H1_es & H2_es)".            
-    iMod ((own_update (γ_c r) (to_frac_agree 1 Cr) 
-                  (to_frac_agree 1 Cr')) with "[$Hc]") as "Hc".
+    iMod ((own_update (γ_c) (to_frac_agree 1 Cn) 
+                  (to_frac_agree 1 Cn')) with "[$Hc]") as "Hc".
     { apply cmra_update_exclusive. 
       unfold valid, cmra_valid. simpl. unfold prod_valid.
       split; simpl; try done. }
     iEval (rewrite <-Qp_half_half) in "Hc".
     iEval (rewrite frac_agree_op) in "Hc".  
     iDestruct "Hc" as "(H1_c & H2_c)".
-    iMod ((own_update (γ_b r) (to_frac_agree 1 Br) 
-                  (to_frac_agree 1 Br')) with "[$Hb]") as "Hb".
+    iMod ((own_update (γ_b) (to_frac_agree 1 Bn) 
+                  (to_frac_agree 1 Bn')) with "[$Hb]") as "Hb".
     { apply cmra_update_exclusive. 
       unfold valid, cmra_valid. simpl. unfold prod_valid.
       split; simpl; try done. }
     iEval (rewrite <-Qp_half_half) in "Hb".
     iEval (rewrite frac_agree_op) in "Hb".  
     iDestruct "Hb" as "(H1_b & H2_b)".
-  iModIntro. iFrame.
+    iMod ((own_update (γ_q) (to_frac_agree 1 Qn) 
+                  (to_frac_agree 1 Qn')) with "[$Hq]") as "Hq".
+    { apply cmra_update_exclusive. 
+      unfold valid, cmra_valid. simpl. unfold prod_valid.
+      split; simpl; try done. }
+    iEval (rewrite <-Qp_half_half) in "Hq".
+    iEval (rewrite frac_agree_op) in "Hq".  
+    iDestruct "Hq" as "(H1_q & H2_q)".
+    iModIntro. iFrame.
   Qed.
+
 
   Lemma auth_agree γ xs ys :
     own γ (● (Excl' xs)) -∗ own γ (◯ (Excl' ys)) -∗ ⌜xs = ys⌝.
@@ -502,28 +628,25 @@ Section multicopy.
   Qed.
 
 
-  Lemma auth_update γ ys xs1 xs2 :
-    own γ (● (Excl' xs1)) -∗ own γ (◯ (Excl' xs2)) ==∗
-      own γ (● (Excl' ys)) ∗ own γ (◯ (Excl' ys)).
+  Lemma set_of_map_member_ne (C: gmap K nat) k :
+            C !! k = None →    
+              ∀ t, (k, t) ∉ set_of_map C.
   Proof.
-    iIntros "Hγ● Hγ◯".
-    iMod (own_update_2 _ _ _ (● Excl' ys ⋅ ◯ Excl' ys)
-      with "Hγ● Hγ◯") as "[$$]".
-    { by apply auth_update, option_local_update, exclusive_local_update. }
-    done.
+    set (P := λ (s: gset KT) (m: gmap K nat), 
+                   m !! k = None → ∀ t, (k, t) ∉ s). 
+    apply (map_fold_ind P); try done.
+    intros kx tx m r Hm HP. unfold P.
+    unfold P in HP. destruct (decide (kx = k)).
+    - subst kx. rewrite lookup_insert. try done.
+    - rewrite lookup_insert_ne; try done. 
+      intros Hm'. pose proof HP Hm' as HP. 
+      intros t. intros Hnot. 
+      rewrite elem_of_union in Hnot*; intros Hnot.
+      destruct Hnot as [Hnot | Hnot].
+      + by apply HP in Hnot.
+      + rewrite elem_of_singleton in Hnot*; intros Hnot.
+        inversion Hnot. try done.
   Qed.
-  
-  Lemma auth_update' (γ: gname) (ys xs1 xs2: gset KT) :
-    own γ (● (Excl' xs1)) -∗ own γ (◯ (Excl' xs2)) ==∗
-      own γ (● (Excl' ys)) ∗ own γ (◯ (Excl' ys)).
-  Proof.
-    iIntros "Hγ● Hγ◯".
-    iMod (own_update_2 _ _ _ (● Excl' ys ⋅ ◯ Excl' ys)
-      with "Hγ● Hγ◯") as "[$$]".
-    { admit. }  
-    (* { apply auth_update. option_local_update, exclusive_local_update. } *)
-    done.
-  Admitted.
 
   Lemma set_of_map_member (C: gmap K nat) k t :
             C !! k = Some(t) →    
@@ -540,7 +663,7 @@ Section multicopy.
     - rewrite lookup_insert_ne; try done.
       pose proof Hp j x' as Hp'. set_solver.
   Qed.
-  
+
   Lemma set_of_map_member_rev (C: gmap K nat) k t :
             (k, t) ∈ set_of_map C → 
                 C !! k = Some(t).
@@ -595,11 +718,12 @@ Section multicopy.
              intros [Hv | Hv]. assert (t = t') by set_solver. 
              lia. destruct Hp as [_ [Hp _]].
              pose proof Hp t Hv. lia. simpl.
-             assert (m !!! k <=? t' = true) as Hm.
+             assert (m !!! k <= t') as Hm.
              { unfold lookup_total, finmap_lookup_total.
                destruct Hp as [_ [_ Hp]]. rewrite Hp.
-               simpl. rewrite leb_le. lia. }
-             rewrite Hm. by rewrite lookup_insert.      
+               simpl. lia. }
+             destruct (decide (m !!! k ≤ t')); try done.  
+             by rewrite lookup_insert.      
           ** assert (t' = T ∨ t' < T) as Ht by lia. clear n. 
              exists T. destruct Hp as [Hp1 [Hp2 Hp3]].
              repeat split; first set_solver.
@@ -607,23 +731,26 @@ Section multicopy.
              intros [Hv | Hv]. assert (t = t') by set_solver. 
              lia. pose proof Hp2 t Hv. lia. simpl.
              destruct Ht as [Ht | Ht].
-             assert (m !!! k <=? t' = true) as Hm.
+             assert (m !!! k <= t') as Hm.
              { unfold lookup_total, finmap_lookup_total.
-               rewrite Hp3. simpl. rewrite leb_le. lia. }
-             rewrite Hm. rewrite lookup_insert. by rewrite Ht.
-             assert (m !!! k <=? t' = false) as Hm.
+               rewrite Hp3. simpl. lia. }
+             destruct (decide (m !!! k ≤ t')); try done.
+             rewrite lookup_insert. by rewrite Ht.
+             assert (m !!! k > t') as Hm.
              { unfold lookup_total, finmap_lookup_total.
-               rewrite Hp3. simpl. by apply leb_correct_conv. }
-             by rewrite Hm.
+               rewrite Hp3. simpl. lia. }
+             destruct (decide (m !!! k ≤ t')); try done.  
+             exfalso. lia.
         * exists t'. simpl. repeat split; first set_solver.
           intros t. rewrite elem_of_union. intros [Hv | Hv].
           assert (t = t') by set_solver. lia.
           destruct Hp as [Hp _]. 
           pose proof Hp t as Hp. set_solver.
-          assert (m !!! k <=? t' = true) as Hm.
+          assert (m !!! k ≤ t') as Hm.
           { unfold lookup_total, finmap_lookup_total.
-            destruct Hp as [_ Hp]. rewrite Hp. by simpl. }
-          rewrite Hm. by rewrite lookup_insert.
+            destruct Hp as [_ Hp]. rewrite Hp. simpl; lia. }
+          destruct (decide (m !!! k ≤ t')); try done.  
+          by rewrite lookup_insert.
       + unfold P. unfold P in Hp.
         destruct Hp as [Hp | Hp].
         * destruct Hp as [T [Hp1 [Hp2 Hp3]]].
@@ -631,14 +758,14 @@ Section multicopy.
           intros t Hkt. assert ((k,t) ∈ X) as Hx by set_solver.
           by pose proof Hp2 t Hx.
           simpl. 
-          destruct (m !!! k' <=? t'). 
+          destruct (decide (m !!! k' <= t')). 
           rewrite lookup_insert_ne; try done. done.
         * destruct Hp as [Hp1 Hp2]. right.
           repeat split; first set_solver. simpl.   
-          destruct (m !!! k' <=? t'). 
+          destruct (decide (m !!! k' <= t')). 
           rewrite lookup_insert_ne; try done. done.
-  Qed.          
-
+  Qed.
+  
   Lemma map_of_set_lookup H k T : 
         (k, T) ∈ H → (∀ t, (k, t) ∈ H → t ≤ T) →
            map_of_set H !! k = Some T.
@@ -701,1700 +828,369 @@ Section multicopy.
       rewrite lookup_insert_ne; try done.
       by rewrite Hc.
   Qed. 
+  
 
-  Lemma outflow_constraint_outset_I In es Cn Bn : 
-        ∀ k, outflow_constraint_I In es Cn Bn →
-                Cn !!! k ≠ 0 → ¬ out_KT In k.
+  Lemma flowint_update_result (γ: gname) (I I_n I_n': multiset_flowint_ur K) x :
+    ⌜flowint_update_P (_) I I_n I_n' x⌝ ∗ own γ x -∗
+    ∃ I', ⌜contextualLeq (_) I I'⌝
+          ∗ ⌜∃ I_o, I = I_n ⋅ I_o ∧ I' = I_n' ⋅ I_o⌝
+          ∗ own γ (● I' ⋅ ◯ I_n').
   Proof.
-    intros k Out Hc. unfold outflow_constraint_I in Out.
-    unfold out_KT. unfold not.
-    intros [t [n Hout]]. apply Out in Hout.
-    destruct Hout as [_ [Hout _]].
-    contradiction. 
+    unfold flowint_update_P.
+    case_eq (view_auth_proj x); last first.
+    - intros Hx. iIntros "(% & ?)". iExFalso. done.
+    - intros [q a] Hx.
+      iIntros "[HI' Hown]". iDestruct "HI'" as %HI'.
+      destruct HI' as [I' HI'].
+      destruct HI' as [Hagree [Hq [HIn [Hcontxl HIo]]]].
+      iExists I'.
+      iSplit. by iPureIntro.
+      iSplit. by iPureIntro. destruct x.
+      simpl in Hx. simpl in HIn.
+      rewrite Hx. rewrite <-HIn.
+      rewrite Hq Hagree.
+      assert (● I' ⋅ ◯ I_n' = View (Some (1%Qp, to_agree I')) I_n') as H'.
+      { rewrite /(● I' ⋅ ◯ I_n'). unfold cmra_op.
+        simpl. unfold view_op. simpl.
+        assert (ε ⋅ I_n' = I_n') as H'. by rewrite left_id.
+        rewrite H'. unfold op, cmra_op. by simpl. }   
+      by iEval (rewrite H').
   Qed.
 
-
-  (** Proofs **)  
-
-  Lemma traverse_spec γ_te γ_he γ_s γ_t γ_I γ_J γ_R 
-                                γ_f γ_e γ_c γ_b γ_cir lc r n k t0 t1:
-    ⊢ ⌜k ∈ KS⌝ -∗ mcs_inv γ_te γ_he γ_s γ_t γ_I γ_J γ_R γ_f γ_e γ_c γ_b γ_cir lc r -∗
-        inFP γ_f n -∗ own (γ_cir n k) (◯ MaxNat t1) -∗ ⌜t0 ≤ t1⌝ -∗
-          <<< ∀ t H, MCS γ_te γ_he t H >>> 
-              traverse #n #k @ ⊤ ∖ ↑N
-          <<< ∃ (t': nat), MCS γ_te γ_he t H ∗ ⌜(k, t') ∈ H⌝ 
-                                             ∗ ⌜t0 ≤ t'⌝ , RET #t' >>>.
+  Lemma flowint_update_result' (γ: gname) (I I_n I_n': multiset_flowint_ur KT) x :
+    ⌜flowint_update_P (_) I I_n I_n' x⌝ ∗ own γ x -∗
+    ∃ I', ⌜contextualLeq (_) I I'⌝
+          ∗ ⌜∃ I_o, I = I_n ⋅ I_o ∧ I' = I_n' ⋅ I_o⌝
+          ∗ own γ (● I' ⋅ ◯ I_n').
   Proof.
-    iIntros "k_in_KS #HInv". iLöb as "IH" forall (n t1).
-    iIntros "#FP_n #Hlb H". iDestruct "H" as %t0_le_t1.
-    iDestruct "k_in_KS" as %k_in_KS.
-    iIntros (Φ) "AU". wp_lam. wp_pures.
-    (** Lock node n **)
-    awp_apply lockNode_spec_high; try done.
-    iAaccIntro with ""; try eauto with iFrame. 
-    iIntros (Cn Bn)"HnP_n". iModIntro.
-    wp_pures. iDestruct "HnP_n" as (es T)"(node_n & HnP_frac & HnP_C & HnP_t)".
-    (** Check contents of n **)
-    wp_apply (inContents_spec with "node_n").
-    iIntros (t) "(node_n & H)". iDestruct "H" as %Cn_val.
-    wp_pures.
-    (** Case analysis on whether k in contents of n **)
-    case_eq (bool_decide ((#t = #0))).
-    - (** Case : k not in contents of n **)
-      intros Ht. wp_pures.
-      (** Find next node to visit **)
-      wp_apply (findNext_spec with "node_n").
-      iIntros (b n1) "(node_n & Hif)". 
-      (** Case analysis on whether there exists a next node **)
+    unfold flowint_update_P.
+    case_eq (view_auth_proj x); last first.
+    - intros Hx. iIntros "(% & ?)". iExFalso. done.
+    - intros [q a] Hx.
+      iIntros "[HI' Hown]". iDestruct "HI'" as %HI'.
+      destruct HI' as [I' HI'].
+      destruct HI' as [Hagree [Hq [HIn [Hcontxl HIo]]]].
+      iExists I'.
+      iSplit. by iPureIntro.
+      iSplit. by iPureIntro. destruct x.
+      simpl in Hx. simpl in HIn.
+      rewrite Hx. rewrite <-HIn.
+      rewrite Hq Hagree.
+      assert (● I' ⋅ ◯ I_n' = View (Some (1%Qp, to_agree I')) I_n') as H'.
+      { rewrite /(● I' ⋅ ◯ I_n'). unfold cmra_op.
+        simpl. unfold view_op. simpl.
+        assert (ε ⋅ I_n' = I_n') as H'. by rewrite left_id.
+        rewrite H'. unfold op, cmra_op. by simpl. }   
+      by iEval (rewrite H').
+  Qed.    
+
+  Lemma dom_lookup (C: gmap K nat) k :
+        C !! k ≠ None → k ∈ dom (gset K) C.
+  Proof.
+    intros Hcn. destruct (C !! k) eqn: Hcnk.
+    rewrite elem_of_dom. rewrite Hcnk.
+    by exists n. done.
+  Qed.
+  
+  Lemma contents_in_reach_bigS_update (S : gset K) (γ: gmap K gname) 
+                                          (Bm Bm': gmap K nat) :
+        ⌜∀ k, k ∈ S → Bm !!! k ≤ Bm' !!! k⌝ -∗ 
+          [∗ set] k ∈ S, own (γ !!! k) (● (MaxNat (Bm !!! k))) -∗
+            |==>  [∗ set] k ∈ S, own (γ !!! k) (● (MaxNat (Bm' !!! k))).
+  Proof.
+  Admitted.
+  
+  Definition map_subset (S: gset K) (C: gmap K nat) :=
+              let f := λ a s', s' ∪ {[(a, C !!! a)]} in
+                        set_fold f (∅: gset KT) S.          
+
+  Definition map_restriction (S: gset K) (C: gmap K nat) := 
+              let f := λ a m, <[a := C !!! a ]> m in
+                        set_fold f (∅: gmap K nat) S.
+                        
+  
+  Lemma lookup_map_restriction S (C: gmap K nat) (k: K):
+              k ∈ S → map_restriction S C !! k = Some (C !!! k).
+  Proof.
+    set (P := λ (m: gmap K nat) (X: gset K),
+                    ∀ x, x ∈ X → m !! x = Some (C !!! x)).
+    apply (set_fold_ind_L P); try done.
+    intros x X r Hx HP.
+    unfold P in HP. unfold P.
+    intros x' Hx'.
+    destruct (decide (x' = x)).
+    - subst x'. by rewrite lookup_insert.
+    - assert (x' ∈ X) as x'_in_X. set_solver.
+      rewrite lookup_insert_ne. apply HP.
+      done. done.
+  Qed.
+
+  Lemma map_subset_member S C k t:
+              (k, t) ∈ map_subset S C ↔ k ∈ S ∧ t = C !!! k.
+  Proof.
+    set (P := λ (m: gset KT) (X: gset K),
+                    ∀ kx tx, (kx, tx) ∈ m ↔ kx ∈ X ∧ tx = C !!! kx).
+    apply (set_fold_ind_L P); try done.
+    - unfold P. intros kx tx. set_solver.
+    - intros x X r Hx HP. unfold P.
+      unfold P in HP. intros kx' tx'.
+      split.
+      + intros Hktx. rewrite elem_of_union in Hktx*; intros Hktx.
+        destruct Hktx as [H' | H'].
+        * apply HP in H'. destruct H' as [H' H''].
+          split; try done. set_solver.
+        * rewrite elem_of_singleton in H'*; intros H'.
+          inversion H'. split; try done; set_solver.
+      + intros [H' H'']. rewrite elem_of_union in H'*; intros H'.
+        destruct H' as [H' | H'].
+        rewrite elem_of_singleton in H'*; intros H'.
+        rewrite H'. rewrite H''. set_solver.
+        assert ((kx', tx') ∈ r) as Hkt.
+        apply HP. split; try done.
+        set_solver.       
+  Qed.              
+
+  Lemma map_restriction_dom S C :
+              dom (gset K) (map_restriction S C) = S.
+  Proof.
+    set (P := λ (m: gmap K nat) (X: gset K), dom (gset K) m = X).
+    apply (set_fold_ind_L P); try done.
+    - unfold P; set_solver. 
+    - intros x X r Hx HP. unfold P. unfold P in HP. 
+      apply leibniz_equiv. rewrite dom_insert.
+      rewrite HP. done.
+  Qed.            
+
+  Lemma map_of_set_lookup_some_aux (H: gset KT) k :
+          (∀ t, (k,t) ∉ H) ∨ (∃ T, (k, T) ∈ H ∧ (∀ t', (k,t') ∈ H → t' ≤ T)).
+  Proof.
+    set (P := λ (X: gset KT), (∀ t, (k,t) ∉ X) ∨ 
+                  (∃ T, (k, T) ∈ X ∧ (∀ t', (k,t') ∈ X → t' ≤ T))).
+    apply (set_ind_L P); try done.
+    - unfold P. left. intros t. set_solver.
+    - intros [k' t'] X Hkt HP. subst P.
+      simpl in HP. simpl. destruct (decide (k' = k)).
+      + subst k'. destruct HP as [H' | H'].
+        * right. exists t'. split.
+          set_solver. intros t. destruct (decide (t' = t)).
+          subst t'. intros; done.
+          intros H''. assert ((k,t) ∈ X).
+          set_solver. pose proof H' t as H'.
+          done.
+        * right. destruct H' as [T H']. 
+          destruct (decide (t' < T)).
+          ** exists T. split.
+             destruct H' as [H' _].
+             set_solver. intros t Hkt'.
+             rewrite elem_of_union in Hkt'*; intros Hkt'.
+             destruct Hkt' as [Hkt' | Hkt'].
+             rewrite elem_of_singleton in Hkt'*; intros Hkt'.
+             inversion Hkt'. lia. 
+             destruct H' as [_ H'']. apply H''; try done.
+          ** exists t'. split. set_solver.
+             intros t Hkt'. rewrite elem_of_union in Hkt'*; intros Hkt'.
+             destruct Hkt' as [Hkt' | Hkt'].
+             rewrite elem_of_singleton in Hkt'*; intros Hkt'.
+             inversion Hkt'. lia.
+             destruct H' as [_ H'']. 
+             apply (Nat.le_trans _ T _); try lia.
+             apply H''. try done.
+      + destruct HP as [H' | H'].
+        * left. intros t. set_solver.
+        * right. destruct H' as [T H'].
+          exists T. destruct H' as [H' H''].
+          split. set_solver. intros t.
+          intros Hkt'. rewrite elem_of_union in Hkt'*; intros Hkt'.
+          destruct Hkt' as [Hkt' | Hkt'].
+          rewrite elem_of_singleton in Hkt'*; intros Hkt'.
+          inversion Hkt'. done. apply H''; try done.
+  Qed.
+
+  Lemma map_of_set_lookup_some (H: gset KT) k t :
+              (k, t) ∈ H → is_Some(map_of_set H !! k).
+  Proof.
+    intros Hkt.
+    pose proof map_of_set_lookup_some_aux H k as Hkt'.
+    destruct Hkt' as [Hkt' | Hkt'].
+    { pose proof Hkt' t as H'. set_solver. }
+    pose proof (map_of_set_lookup_cases H k) as H'.
+    destruct H' as [H' | H'].
+    - destruct H' as [T' H'].
+      destruct H' as [_ [_ H']].
+      rewrite H'. by exists T'.
+    - destruct Hkt' as [T Hkt'].
+      destruct Hkt' as [Hkt' _].
+      destruct H' as [H' _].
+      pose proof H' T as H'.
+      set_solver.   
+  Qed.            
+
+  (** Lock module **)
+  
+  Parameter getLockLoc_spec : ∀ (n: Node),
+    ⊢ ({{{ True }}}
+        getLockLoc #n
+       {{{ (l:loc), RET #l; ⌜lockLoc n = l⌝ }}})%I.
+  
+  Lemma lockNode_spec (n: Node):
+    ⊢ <<< ∀ (b: bool), (lockLoc n) ↦ #b >>>
+      lockNode #n    @ ⊤
+    <<< (lockLoc n) ↦ #true ∗ ⌜b = false⌝ , RET #() >>>.
+  Proof.
+    iIntros (Φ) "AU". iLöb as "IH".
+    wp_lam. wp_bind(getLockLoc _)%E.
+    wp_apply getLockLoc_spec; first done.
+    iIntros (l) "#Hl". wp_let. wp_bind (CmpXchg _ _ _)%E.
+    iMod "AU" as (b) "[Hb HAU]". iDestruct "Hl" as %Hl.
+    iEval (rewrite Hl) in "Hb". destruct b.
+    - wp_cmpxchg_fail. iDestruct "HAU" as "[HAU _]".
+      iEval (rewrite Hl) in "HAU".
+      iMod ("HAU" with "Hb") as "H".
+      iModIntro. wp_pures. iApply "IH".
+      iEval (rewrite <-Hl) in "H". done.
+    - wp_cmpxchg_suc. iDestruct "HAU" as "[_ HAU]".
+      iEval (rewrite Hl) in "HAU".
+      iMod ("HAU" with "[Hb]") as "HΦ". iFrame; done.
+      iModIntro. wp_pures. done.
+  Qed.
+
+  Lemma lockNode_spec_high N γ_te γ_he γ_s γ_t γ_I γ_R γ_f γ_gh lc r n:
+    ⊢ mcs_inv N γ_te γ_he γ_s γ_t γ_I γ_R γ_f γ_gh lc r -∗
+        inFP γ_f n -∗
+              <<< True >>>
+                lockNode #n    @ ⊤ ∖ ↑N
+              <<< ∃ Cn Bn Qn, nodePred γ_gh γ_t γ_s lc r n Cn Bn Qn, RET #() >>>.
+  Proof.
+    iIntros "#mcsInv #FP_n".
+    iIntros (Φ) "AU".
+    awp_apply (lockNode_spec n).
+    iInv "mcsInv" as ">mcs". iDestruct "mcs" as (T H hγ I R) "(Hglob & Hstar)".
+    iDestruct "Hglob" as "(MCS_auth & HH & Hist & Ht & HI & Out_I & HR 
+            & Out_R & Inf_R & Hf & Hγ & FP_r & Max_ts & domm_IR & domm_Iγ)".
+    iPoseProof (inFP_domm with "[$FP_n] [$]") as "%". rename H0 into n_in_I.
+    iEval (rewrite (big_sepS_elem_of_acc (_) (domm I) n); 
+           last by eauto) in "Hstar".
+    iDestruct "Hstar" as "(Hn & Hstar')".
+    iDestruct "Hn" as (b Cn Bn Qn) "(Hlock & Hnp & Hns)".
+    iAaccIntro with "Hlock".
+    { iIntros "Hlockn". iModIntro.
+      iSplitR "AU".
+      { iExists T, H, hγ, I, R. iFrame.
+        iPoseProof ("Hstar'" with "[-]") as "Hstar".
+        iExists b, Cn, Bn, Qn. iFrame.
+        iNext. iFrame.
+      }
+      iFrame.
+    }
+    iIntros "(Hlockn & %)". subst b.
+    iMod "AU" as "[_ [_ Hclose]]".
+    iMod ("Hclose" with "[Hnp]") as "HΦ"; try done.
+    iModIntro. iSplitR "HΦ".
+    iNext. iExists T, H, hγ, I, R.
+    iPoseProof ("Hstar'" with "[Hlockn Hns]") as "Hstar".
+    iExists true, Cn, Bn, Qn. iFrame.
+    iSplitR "Hstar". iFrame. iFrame. done.
+  Qed.
+
+  Lemma unlockNode_spec (n: Node) :
+    ⊢ <<< lockLoc n ↦ #true >>>
+      unlockNode #n    @ ⊤
+    <<< lockLoc n ↦ #false, RET #() >>>.
+  Proof.
+    iIntros (Φ) "AU". wp_lam. wp_bind(getLockLoc _)%E.
+    wp_apply getLockLoc_spec; first done.
+    iIntros (l) "#Hl". wp_let.
+    iMod "AU" as "[Hy [_ Hclose]]".
+    iDestruct "Hl" as %Hl.
+    iEval (rewrite Hl) in "Hy".
+    wp_store. iEval (rewrite Hl) in "Hclose".
+    iMod ("Hclose" with "Hy") as "HΦ".
+    iModIntro. done.
+  Qed.
+(*  
+  Lemma int_domm γ_te γ_he γ_s γ_t γ_I γ_R γ_f γ_gh r t H hγ I R n In :
+    own γ_I (◯ In) -∗ ⌜domm In = {[n]}⌝
+    -∗ global_state γ_te γ_he γ_s γ_t γ_I γ_R γ_f γ_gh r t H hγ I R
+    -∗ ⌜n ∈ domm I⌝.
+  Proof.
+    iIntros "Hi Dom_In Hglob".
+    iDestruct "Dom_In" as %Dom_In.
+    iDestruct "Hglob" as "(MCS_auth & HH & Hist & Ht & HI & Out_I & HR 
+            & Out_R & Inf_R & Hf & Hγ & FP_r & Max_ts & domm_IR & domm_Iγ)".
+    iPoseProof ((auth_own_incl γ_I (I) (In)) with "[$]") as "%".
+    rename H0 into I_incl. destruct I_incl as [Io I_incl].
+    iPoseProof (own_valid with "HI") as "%". rename H0 into Valid_I.
+    iPureIntro. rewrite I_incl. rewrite flowint_comp_fp.
+    rewrite Dom_In. set_solver. rewrite <- I_incl.
+    by apply auth_auth_valid.
+  Qed.
+*)
+  Lemma unlockNode_spec_high N γ_te γ_he γ_s γ_t γ_I γ_R γ_f γ_gh lc r n Cn Bn Qn:
+    ⊢ mcs_inv N γ_te γ_he γ_s γ_t γ_I γ_R γ_f γ_gh lc r -∗
+        inFP γ_f n -∗ nodePred γ_gh γ_t γ_s lc r n Cn Bn Qn -∗
+              <<< True >>>
+                unlockNode #n    @ ⊤ ∖ ↑N
+              <<< True, RET #() >>>.
+  Proof.
+    iIntros "#mcsInv #FP_n Hnp". iIntros (Φ) "AU".
+    awp_apply (unlockNode_spec n).
+    iInv "mcsInv" as ">mcs". iDestruct "mcs" as (T H hγ I R) "(Hglob & Hstar)".
+    iDestruct "Hglob" as "(MCS_auth & HH & Hist & Ht & HI & Out_I & HR 
+            & Out_R & Inf_R & Hf & Hγ & FP_r & Max_ts & domm_IR & domm_Iγ)".
+    iPoseProof (inFP_domm with "[$FP_n] [$]") as "%". rename H0 into n_in_I.
+    iEval (rewrite (big_sepS_elem_of_acc (_) (domm I) n); 
+           last by eauto) in "Hstar".
+    iDestruct "Hstar" as "(Hn & Hstar')".
+    iDestruct "Hn" as (b Cn' Bn' Qn') "(Hlock & Hnp' & Hns)".
+    iAssert (lockLoc n ↦ #true ∗ nodePred γ_gh γ_t γ_s lc r n Cn Bn Qn)%I
+      with "[Hlock Hnp Hnp']" as "(Hlock & Hnp)".
+    {
       destruct b.
-      + (** Case : exists next node n' **)
-        wp_pures. iDestruct "Hif" as %k_in_es.
-        iApply fupd_wp.
-        (** Open invariant to establish resources
-            required to apply induction hypothesis IH
-            on node n' **)
-        iInv "HInv" as ">H".
-        iDestruct "H" as (T' H I J R) "(Hglob & Hstar)".
-        iAssert (⌜n ∈ domm I⌝)%I as "%". 
-        { iDestruct "Hglob" as "(MCS_auth & HH & Hist & Ht & HI & HJ & HR & Hf 
-                & Inf_I & Inf_J & Inf_R & _ & Max_ts & domm_IJ & domm_IR)".
-          by iPoseProof (inFP_domm _ _ _ with "[$FP_n] [$Hf]") as "H'". }
-        rewrite (big_sepS_delete _ (domm I) n); last by eauto.
-        iDestruct "Hstar" as "(H_n & Hstar')".
-        iDestruct "H_n" as (bn Cn' Bn')"(Hl_n & Hlif_n & HnS_n)".
-        iDestruct "HnS_n" as (es' In Jn Rn) "(HnS_frac & HnS_si & HnS_FP 
-                                & HnS_cl & HnS_oc & HnS_H & HnS_star & Hφ)".
-        iPoseProof (frac_eq with "[$HnP_frac] [$HnS_frac]") as "%".
-        destruct H1 as [Hes [Hc Hb]]. subst es'. subst Cn'. subst Bn'.
-        iAssert (inFP γ_f n1)%I as "#FP_n1".
-        { iApply "HnS_cl". iPureIntro. 
-          clear -k_in_es. set_solver. }
-        iAssert (⌜(k, Bn !!! k) ∈ outset_KT In n1⌝)%I as %outflow_n_n1.
-        { iDestruct "HnS_oc" as "(H' & _)".
-          iDestruct "H'" as %H'. iPureIntro. 
-          apply (H' n1 k (Bn !!! k)).
-          repeat split; try done. apply bool_decide_eq_true in Ht.
-          inversion Ht as [H'']. rewrite Cn_val.
-          clear -H''. lia. }
-        iAssert (⌜n1 ∈ domm I⌝)%I as %n_in_I.
-        { iDestruct "Hglob" as "(_ & _ & _ & _ & _ & _ & _ & Hf & _)". 
-          by iPoseProof (inFP_domm _ _ _ with "[$FP_n1] [$Hf]") as "H'". }
-        iAssert (⌜n ≠ n1⌝)%I as %n_neq_n1.
-        { destruct (decide (n = n1)); try done.
-          iPoseProof (node_edgeset_self_empty with "node_n") as "%".
-          rename H1 into Es_n. rewrite <-e in k_in_es.
-          clear -k_in_es Es_n. set_solver. } 
-        rewrite (big_sepS_delete _ (domm I ∖ {[n]}) n1); last by set_solver.
-        iDestruct "Hstar'" as "(H_n1 & Hstar'')".
-        iDestruct "H_n1" as (bn1 Cn1 Bn1)"(Hl_n1 & Hlif_n1 & HnS_n1)".
-        iDestruct "HnS_n1" as (es1 In1 Jn1 Rn1) 
-         "(HnS_frac1 & HnS_si1 & HnS_FP1 & HnS_cl1 & 
-                          HnS_oc1 & HnS_H1 & HnS_star1 & Hφ1)".
-        iAssert (⌜(k, Bn !!! k) ∈ inset_KT In1 n1⌝)%I as %inflow_n1.
-        { iDestruct "HnS_si" as "(H'&_)".
-          iDestruct "HnS_si1" as "(H1'&_&_&%&_)".
-          rename H1 into Domm_In1.
-          assert (n1 ∈ domm In1) as H''. 
-          { clear -Domm_In1. set_solver. }
-          iCombine "H'" "H1'" as "H'".
-          iPoseProof (own_valid with "[$H']") as "%".
-          rename H1 into Valid_InIn1.
-          rewrite auth_frag_valid in Valid_InIn1 *; intros Valid_InIn1.
-          pose proof intComp_unfold_inf_2 In In1 Valid_InIn1 n1 H''.
-          rename H1 into H'. unfold ccmop, ccm_op in H'.
-          simpl in H'. unfold lift_op in H'.
-          iPureIntro. rewrite nzmap_eq in H' *; intros H'.
-          pose proof H' (k, Bn !!! k) as H'.
-          rewrite nzmap_lookup_merge in H'.
-          unfold ccmop, ccm_op in H'. simpl in H'.
-          unfold nat_op in H'.
-          assert (1 ≤ out In n1 !1 (k, Bn !!! k)) as Hout.
-          { unfold outset_KT, KT_flows.dom_ms in outflow_n_n1.
-            rewrite nzmap_elem_of_dom_total in outflow_n_n1 *; 
-            intros outflow_n_n1.
-            unfold ccmunit, ccm_unit in outflow_n_n1.
-            simpl in outflow_n_n1. unfold nat_unit in outflow_n_n1.
-            clear - outflow_n_n1. lia. }
-          assert (1 ≤ inf In1 n1 !1 (k, Bn !!! k)) as Hin.
-          { clear -H' Hout. 
-            assert (∀ (x y z: nat), 1 ≤ y → x = z + y → 1 ≤ x) as H''.
-            lia. by pose proof H'' _ _ _ Hout H'. }
-          unfold inset_KT. rewrite nzmap_elem_of_dom_total.
-          unfold ccmunit, ccm_unit. simpl. unfold nat_unit.
-          clear -Hin. lia. }    
-        iAssert (⌜Bn1 !!! k = Bn !!! k⌝)%I as %Bn1_eq_Bn.
-        { iDestruct "Hφ1" as "(_ & _ & % & _)". rename H1 into Hφ2.
-          by pose proof Hφ2 k (Bn !!! k) inflow_n1. } 
-        iEval (rewrite (big_sepS_elem_of_acc (_) (KS) k); last by eauto) 
-                                                                in "HnS_star".
-        iDestruct "HnS_star" as "(Hcirk_n & HnS_star')".
-        iAssert (⌜t1 ≤ Bn !!! k⌝)%I as %lb_t1.
-        { iPoseProof (own_valid_2 with "[$Hcirk_n] [$Hlb]") as "%".
-          rename H1 into Valid_Bnt.
-          apply auth_both_valid_discrete in Valid_Bnt.
-          destruct Valid_Bnt as [H' _].
-          apply max_nat_included in H'.
-          simpl in H'. by iPureIntro. }
-        iEval (rewrite (big_sepS_elem_of_acc (_) (KS) k); last by eauto) 
-                                                                in "HnS_star1".
-        iDestruct "HnS_star1" as "(Hcirk_n1 & HnS_star1')".
-        iMod (own_update (γ_cir n1 k) (● MaxNat (Bn1 !!! k)) 
-              ((● MaxNat (Bn1 !!! k)) ⋅ (◯ MaxNat (Bn1 !!! k))) 
-                  with "[Hcirk_n1]") as "(Hcirk_n1 & #Hlb_1)".
-        { apply (auth_update_alloc _ (MaxNat (Bn1 !!! k)) 
-                              (MaxNat (Bn1 !!! k))).
-          apply max_nat_local_update. 
-          simpl. lia. } { iFrame. }
-        (** Closing the invariant **)
-        iModIntro. iSplitR "node_n HnP_frac HnP_C HnP_t AU". iNext.
-        iExists T', H, I, J, R. iFrame "Hglob".
-        rewrite (big_sepS_delete _ (domm I) n); last by eauto.
-        rewrite (big_sepS_delete _ (domm I ∖ {[n]}) n1); last set_solver.
-        iFrame "Hstar''". iSplitL "Hl_n Hlif_n HnS_frac HnS_si HnS_FP
-                         HnS_cl HnS_oc HnS_H Hcirk_n HnS_star' Hφ".
-        iExists bn, Cn, Bn. iFrame "Hl_n Hlif_n".
-        iExists es, In, Jn, Rn. iFrame. by iApply "HnS_star'".                  
-        iExists bn1, Cn1, Bn1. iFrame "Hl_n1 Hlif_n1".
-        iExists es1, In1, Jn1, Rn1. iFrame. by iApply "HnS_star1'".
-        iModIntro.
-        (** Unlock node n **)       
-        awp_apply (unlockNode_spec_high with "[] [] 
-            [HnP_frac HnP_C HnP_t node_n]"); try done. iExists es, T.
-        iFrame.                
-        iAaccIntro with ""; try eauto with iFrame.
-        iIntros "_". iModIntro. wp_pures.
-        (** Apply IH on node n' **)
-        iApply "IH"; try done. iPureIntro.
-        apply leibniz_equiv_iff in Bn1_eq_Bn.
-        rewrite <-Bn1_eq_Bn in lb_t1. clear -lb_t1 t0_le_t1.
-        apply (Nat.le_trans t0 t1 _); try done.
-      + (** Case : no next node from n **)
-        wp_pures. iDestruct "Hif" as %Not_in_es.
-        iApply fupd_wp. 
-        (** Linearization Point: key k has not been found in the 
-            data structure. Open invariant to obtain resources 
-            required to establish post-condition **)
-        iInv "HInv" as ">H".
-        iDestruct "H" as (T' H I J R) "(Hglob & Hstar)".
-        iAssert (⌜n ∈ domm I⌝)%I as "%".
-        { iDestruct "Hglob" as "(MCS_auth & HH & Hist & Ht & HI & HJ & HR & Hf 
-                & Inf_I & Inf_J & Inf_R & _ & Max_ts & domm_IJ & domm_IR)".
-          by iPoseProof (inFP_domm _ _ _ with "[$FP_n] [$Hf]") as "H'". }
-        rewrite (big_sepS_delete _ (domm I) n); last by eauto.
-        iDestruct "Hstar" as "(H_n & Hstar')".
-        iDestruct "H_n" as (bn Cn' Bn')"(Hl_n & Hlif_n & HnS_n)".
-        iDestruct "HnS_n" as (es' In Jn Rn) 
-            "(HnS_frac & HnS_si & HnS_FP & HnS_cl & HnS_oc & 
-                                    HnS_H & HnS_star & Hφ0 & Hφ1 & Hφ)".
-        iPoseProof (frac_eq with "[$HnP_frac] [$HnS_frac]") as "%".
-        destruct H1 as [Hes [Hc Hb]]. subst es'. subst Cn'. subst Bn'.
-        iDestruct "Hφ1" as %Hφ. pose proof Hφ k as Hφ1. 
-        destruct Hφ1 as [Hφ1 | Hφ1].
-        { unfold out_KT in Hφ1. destruct Hφ1 as [tw [n' Hφ1]].
-          iDestruct "HnS_oc" as "(HnS_ocI & HnS_os')". 
-          iDestruct "HnS_ocI" as %HnS_ocI. 
-          pose proof HnS_ocI n' k tw as Hoc.
-          destruct Hoc as [Hoc _].
-          pose proof Hoc Hφ1 as Hoc.
-          destruct Hoc as [Hoc [_ _]].
-          pose proof Not_in_es n'. contradiction. }
-        iEval (rewrite (big_sepS_elem_of_acc (_) (KS) k); last by eauto) 
-                                                       in "HnS_star".
-        iDestruct "HnS_star" as "(Hcirk_n & HnS_star')".
-        iAssert (⌜t1 ≤ Bn !!! k⌝)%I as %lb_t1.
-        { iPoseProof (own_valid_2 with "[$Hcirk_n] [$Hlb]") as "%".
-          rename H1 into Valid_Bnt.
-          apply auth_both_valid_discrete in Valid_Bnt.
-          destruct Valid_Bnt as [H' _].
-          apply max_nat_included in H'.
-          simpl in H'. by iPureIntro. }
-        iAssert (⌜t0 = 0⌝)%I as %t0_zero. 
-        { iPureIntro. rewrite bool_decide_eq_true in Ht *; intros Ht.
-          rewrite Cn_val in Hφ1. rewrite Hφ1 in lb_t1.
-          inversion Ht. clear -H2 lb_t1 t0_le_t1.
-          lia. } subst t0.
-        (** Linearization **)  
-        iMod "AU" as (t' H') "[MCS [_ Hclose]]". 
-        iAssert (⌜H' = H⌝)%I as %H1. 
-        { iDestruct "Hglob" as "(MCS_auth & HH & Hist & Ht & HI & HJ & HR & Hf 
-                  & Inf_I & Inf_J & Inf_R & _ & Max_ts & domm_IJ & domm_IR)".
-          iPoseProof ((auth_agree' γ_he) with "[MCS_auth] [MCS]") as "%".
-          unfold MCS_auth. by iDestruct "MCS_auth" as "(_ & H'')".
-          by iDestruct "MCS" as "(_ & H')".
-          by iPureIntro. } subst H'.
-        iAssert (⌜(k,0) ∈ H⌝)%I as "%". 
-        { iDestruct "Hglob" as "(MCS_auth & HH & Hist & Ht & HI & HJ & HR & Hf 
-                  & Inf_I & Inf_J & Inf_R & _ & Max_ts & domm_IJ & domm_IR)".
-          iDestruct "Hist" as %Hist. iPureIntro. 
-          by pose proof Hist k k_in_KS as Hist. }
-        rename H1 into k0_in_H.  
-        iSpecialize ("Hclose" $! 0).
-        iMod ("Hclose" with "[MCS]") as "HΦ". iFrame. 
-        iPureIntro. split; try done.
-        (** Closing the invariant **)
-        iModIntro. iSplitR "node_n HnP_frac HnP_C HnP_t HΦ". iNext.
-        iExists T', H, I, J, R. iFrame "Hglob".
-        rewrite (big_sepS_delete _ (domm I) n); last by eauto.
-        iFrame "Hstar'". iExists bn, Cn, Bn.
-        iFrame "Hl_n Hlif_n". iExists es, In, Jn, Rn.
-        iFrame "∗%". by iApply "HnS_star'". iModIntro.
-        (** Unlock node n **)
-        awp_apply (unlockNode_spec_high with "[] [] 
-               [HnP_frac HnP_C HnP_t node_n]") without "HΦ"; try done. 
-        iExists es, T. iFrame.
-        iAaccIntro with ""; try eauto with iFrame.
-        iIntros "_". iModIntro. iIntros "HΦ". by wp_pures.
-    - (** Case : k in contents of n **)
-      intros Ht. wp_pures.                                         
-      iApply fupd_wp. 
-      (** Linearization Point: key k has been found. Open 
-          invariant to obtain resources required to 
-          establish post-condition **)
-      iInv "HInv" as ">H".
-      iDestruct "H" as (T' H I J R) "(Hglob & Hstar)".
-      iAssert (⌜n ∈ domm I⌝)%I as "%". 
-      { iDestruct "Hglob" as "(MCS_auth & HH & Hist & Ht & HI & HJ & HR & Hf 
-                & Inf_I & Inf_J & Inf_R & _ & Max_ts & domm_IJ & domm_IR)".
-        by iPoseProof (inFP_domm _ _ _ with "[$FP_n] [$Hf]") as "H'". }
-      rewrite (big_sepS_delete _ (domm I) n); last by eauto.
-      iDestruct "Hstar" as "(H_n & Hstar')".
-      iDestruct "H_n" as (bn Cn' Bn')"(Hl_n & Hlif_n & HnS_n)".
-      iDestruct "HnS_n" as (es' In Jn Rn) 
-          "(HnS_frac & HnS_si & HnS_FP & HnS_cl & HnS_oc & 
-                                  HnS_H & HnS_star & Hφ0 & Hφ1 & Hφ)".
+    - (* Case n locked *)
+      iFrame "∗".
+    - (* Case n unlocked: impossible *)
+      iDestruct "Hnp" as (? ? ? ? ? ? ?) "(n & _)".
+      iDestruct "Hnp'" as (? ? ? ? ? ? ?) "(n' & _)".
+      iExFalso. iApply (node_sep_star r n). iFrame.
+    }
+    iAaccIntro with "Hlock".
+    { iIntros "Hlock". iModIntro.
+      iSplitR "Hnp AU".
+      iExists T, H, hγ, I, R. iNext. iFrame.
+      iPoseProof ("Hstar'" with "[Hlock Hns]") as "Hstar".
+      iExists true, Cn', Bn', Qn'. iFrame.
+      iFrame. iFrame. 
+    }
+    iIntros "Hlock".
+    iMod "AU" as "[_ [_ Hclose]]".
+    iMod ("Hclose" with "[]") as "HΦ"; try done.
+    iModIntro. iSplitR "HΦ".
+    iNext. iExists T, H, hγ, I, R.
+    iPoseProof ("Hstar'" with "[Hlock Hns Hnp]") as "Hstar".
+    iExists false, Cn, Bn, Qn.
+    iAssert (nodePred γ_gh γ_t γ_s lc r n Cn Bn Qn
+                      ∗ nodeShared γ_I γ_R γ_f γ_gh r n Cn Bn Qn H T)%I
+      with "[Hns Hnp]" as "(Hns & Hnp)".
+    {
+      iDestruct "Hnp" as (γ_en γ_cn γ_bn γ_qn γ_cirn esn T')
+                             "(node_n & HnP_gh & HnP_frac & HnP_C & HnP_t)".
+      iDestruct "Hns" as (γ_en' γ_cn' γ_bn' γ_qn' γ_cirn' es' In0 Rn0) 
+                           "(HnS_gh & HnS_frac & HnS_si & HnS_FP 
+                            & HnS_cl & HnS_oc & HnS_H & HnS_star & Hφ)".
+      iPoseProof (ghost_heap_sync with "[$HnP_gh] [$HnS_gh]") 
+        as "(% & % & % & % & %)".
+      subst γ_en'. subst γ_cn'. subst γ_bn'. subst γ_qn'. subst γ_cirn'.
       iPoseProof (frac_eq with "[$HnP_frac] [$HnS_frac]") as "%".
-      destruct H1 as [Hes [Hc Hb]]. subst es'. subst Cn'. subst Bn'.
-      iEval (rewrite (big_sepS_elem_of_acc (_) (KS) k); last by eauto) 
-                                                      in "HnS_star".
-      iDestruct "HnS_star" as "(Hcirk_n & HnS_star')".
-      iAssert (⌜t1 ≤ Bn !!! k⌝)%I as %lb_t1.
-      { iPoseProof (own_valid_2 with "[$Hcirk_n] [$Hlb]") as "%".
-        rename H1 into Valid_Bnt.
-        apply auth_both_valid_discrete in Valid_Bnt.
-        destruct Valid_Bnt as [H' _].
-        apply max_nat_included in H'.
-        simpl in H'. by iPureIntro. }
-      iDestruct "Hφ1" as %Hφ. pose proof Hφ k as Hφ1. 
-      destruct Hφ1 as [Hφ1 | Hφ1].
-      { unfold out_KT in Hφ1. destruct Hφ1 as [tw [n' Hφ1]].
-        iDestruct "HnS_oc" as "(HnS_ocI & HnS_os')". 
-        iDestruct "HnS_ocI" as %HnS_ocI. 
-        pose proof HnS_ocI n' k tw as Hoc.
-        destruct Hoc as [Hoc _].
-        pose proof Hoc Hφ1 as Hoc.
-        destruct Hoc as [_ [Hoc _]].
-        rewrite Cn_val in Hoc. unfold bool_decide in Ht.
-        rewrite Hoc in Ht. simpl in Ht. inversion Ht. }
-      iAssert (⌜set_of_map Cn ⊆ H⌝)%I as %Cn_Sub_H.
-      { iDestruct "Hglob" as "(MCS_auth & HH & Hist & Ht & HI & HJ & HR & Hf 
-                & Inf_I & Inf_J & Inf_R & _ & Max_ts & domm_IJ & domm_IR)".
-        iPoseProof ((auth_own_incl γ_s H _) with "[$HH $HnP_C]") as "%".
-        rename H1 into H'. by apply gset_included in H'. }  
-      iAssert (⌜(k,t) ∈ set_of_map Cn⌝)%I as %kt_in_Cn.
-      { iPureIntro. apply set_of_map_member.
-        rewrite /(Cn !!! k) in Cn_val.
-        unfold finmap_lookup_total, inhabitant in Cn_val.
-        simpl in Cn_val. 
-        destruct (Cn !! k) as [cnk | ] eqn: Hcnk.
-        - rewrite Hcnk. apply f_equal. 
-          by simpl in Cn_val.
-        - simpl in Cn_val.
-          apply bool_decide_eq_false_1 in Ht.
-          exfalso. apply Ht. replace t. try done. }
-      (** Linearization **)      
-      iMod "AU" as (t' H') "[MCS [_ Hclose]]". 
-      iSpecialize ("Hclose" $! t).
-      iAssert (⌜H' = H⌝)%I as %H1. 
-      { iDestruct "Hglob" as "(MCS_auth & HH & Hist & Ht & HI & HJ & HR & Hf 
-                & Inf_I & Inf_J & Inf_R & _ & Max_ts & domm_IJ & domm_IR)".
-        iPoseProof ((auth_agree' γ_he) with "[MCS_auth] [MCS]") as "%".
-        unfold MCS_auth. by iDestruct "MCS_auth" as "(_ & H'')".
-        by iDestruct "MCS" as "(_ & H')".
-        by iPureIntro. } replace H'.
-      iMod ("Hclose" with "[MCS]") as "HΦ". iFrame. 
-      iPureIntro. split. set_solver. rewrite Hφ1 in lb_t1.
-      rewrite Cn_val in lb_t1. lia.
-      (** Closing the invariant **)
-      iModIntro. iSplitR "node_n HnP_frac HnP_C HnP_t HΦ". iNext.
-      iExists T', H, I, J, R. iFrame "Hglob".
-      rewrite (big_sepS_delete _ (domm I) n); last by eauto.
-      iFrame "Hstar'". iExists bn, Cn, Bn.
-      iFrame "Hl_n Hlif_n". iExists es, In, Jn, Rn.
-      iFrame "∗%". by iApply "HnS_star'". iModIntro.
-      (** Unlock node n **)
-      awp_apply (unlockNode_spec_high with "[] [] 
-                [HnP_frac HnP_C HnP_t node_n]") without "HΦ"; 
-                      try done. iExists es, T. iFrame.
-      iAaccIntro with ""; try eauto with iFrame.
-      iIntros "_". iModIntro. iIntros "HΦ". by wp_pures.
-  Qed.  
-
-
-  Lemma upsert_spec γ_te γ_he γ_s γ_t γ_I γ_J γ_R 
-                                  γ_f γ_e γ_c γ_b γ_cir lc r (k: K) :
-    ⊢ ⌜k ∈ KS⌝ -∗ 
-          mcs_inv γ_te γ_he γ_s γ_t γ_I γ_J γ_R γ_f γ_e γ_c γ_b γ_cir lc r -∗
-                <<< ∀ t H, MCS γ_te γ_he t H >>> 
-                    upsert lc r #k @ ⊤ ∖ ↑N
-                <<< MCS γ_te γ_he (t + 1) (H ∪ {[(k, t)]}), RET #() >>>.
-  Proof.
-    iIntros "H". iDestruct "H" as %k_in_KS.
-    iIntros "#HInv". iLöb as "IH".
-    iIntros (Φ) "AU". wp_lam.
-    iApply fupd_wp. 
-    (** Open invariant to establish root node in footprint **)
-    iInv "HInv" as ">H".
-    iDestruct "H" as (T0 H0 I0 J0 R0) "(Hglob & Hstar)".
-    iDestruct "Hglob" as "(MCS & HH & Hist & Ht & HI & HJ & HR & Hf 
-                & Inf_I & Inf_J & Inf_R & #FP_r & Max_ts & domm_IJ & domm_IR)".
-    iModIntro. iSplitR "AU". iNext. 
-    iExists T0, H0, I0, J0, R0. iFrame "∗ #". iModIntro.
-    (** Lock the node r **)
-    awp_apply lockNode_spec_high; try done.
-    iAaccIntro with ""; try eauto with iFrame. 
-    iIntros (Cr Br)"HnP_n". iModIntro. wp_pures.
-    iDestruct "HnP_n" as (es T)"(node_r & HnP_frac & HnP_C & HnP_t)".
-    iEval (rewrite <-beq_nat_refl) in "HnP_t".
-    wp_apply (readClock_spec with "[HnP_t]"); try done.
-    iIntros "HnP_t". wp_pures.
-    wp_apply (addContents_spec with "node_r").
-    iIntros (b Cr')"(node_r & Hif)".
-    (** Case analysis on whether addContents is successful **)
-    destruct b; last first.
-    - (** Case : addContents fails. Unlock root node and apply 
-                 inductive hypothesis IH **) 
-      iDestruct "Hif" as %HCr. replace Cr'. wp_pures.
-      awp_apply (unlockNode_spec_high with "[] [] [-AU]"); try done.
-      { iExists es, T. iFrame. iEval (rewrite <-beq_nat_refl); try done. }
-      iAaccIntro with ""; try eauto with iFrame.
-      iIntros "_". iModIntro. wp_pures.
-      by iApply "IH".
-    - (** Case : addContent successful **)
-      (** Linearization Point: open invariant and update the resources **)
-      awp_apply (incrementClock_spec γ_t lc T). iInv "HInv" as ">H". 
-      iDestruct "H" as (T1 H1 I1 J1 R1) "(Hglob & Hstar)".
-      iDestruct "Hglob" as "(MCS_auth & HH & Hist & Ht & HI & HJ & HR & Hf 
-                & Inf_I & Inf_J & Inf_R & _ & Max_ts & domm_IJ & domm_IR)".
-      iDestruct "Hif" as %HCr. wp_pures.
-      iAssert (⌜T = T1⌝)%I as %HT. 
-      { iDestruct "HnP_t" as "(HnP_t & Hc)".
-        iPoseProof ((own_valid_2 _ _ _) with "[$HnP_t] [$Ht]") as "H'".
-        iDestruct "H'" as %H'. 
-        pose proof (auth_auth_frac_op_inv _ _ _ _ H') as H''.
-        inversion H''. by iPureIntro. } replace T1.
-      (** Updating the clock value **)            
-      iAssert (own γ_t (● (MaxNat T)) ∗ clock lc T)%I 
-                                        with "[Ht HnP_t]" as "H".
-      { iDestruct "HnP_t" as "(Ht' & Hc)".
-        iCombine "Ht Ht'" as "H'". iFrame. }
-      iAaccIntro with "H".
-      { iIntros "H". iDestruct "H" as "(Ht & Hc)".
-        iDestruct "Ht" as "(Ht & HnP_t)".
-        iCombine "HnP_t Hc" as "HnP_t". 
-        iModIntro. iSplitR "AU HnP_frac HnP_C node_r HnP_t".
-        iNext. iExists T, H1, I1, J1, R1. iFrame "∗ #". iFrame.
-        by iPureIntro. }
-      iIntros "H". iDestruct "H" as "(Ht & Hc)".
-      iDestruct "Ht" as "(Ht & HnP_t)".
-      iCombine "HnP_t Hc" as "HnP_t".
-      iPoseProof ((auth_own_incl γ_s H1 _) with "[$HH $HnP_C]") as "%".
-      rename H into Cr_sub_H1. apply gset_included in Cr_sub_H1.
-      iDestruct "Max_ts" as %Max_tsH1.
-      (** Re-establish maxTS for updated T and H **)
-      assert (maxTS (T+1) (H1 ∪ {[(k, T)]})) as Max_ts.
-      { split. intros k' t' H.
-        assert (((k',t') ∈ H1) ∨ (k' = k ∧ t' = T)) as Hor by set_solver.
-        destruct Hor as [Hor | Hor]. 
-        destruct Max_tsH1 as [Max_tsH1 _].
-        pose proof Max_tsH1 k' t' Hor as Hres. lia.
-        destruct Hor as [_ Hor]. replace t'. lia.
-        destruct Max_tsH1 as [_ Max_tsH1]. lia. }       
-      iAssert (⌜set_of_map Cr' ⊆ H1 ∪ {[(k,T)]}⌝)%I as %Cr_sub_H1'.
-      { iPureIntro. replace Cr'.
-        pose proof (set_of_map_insert_subseteq Cr k T) as H'.
-        assert (set_of_map Cr = set_of_map Cr) as H'' by done. 
-        set_solver. }
-      (** Update the (● H) resource **)  
-      iMod (own_update γ_s (● H1) (● (H1 ∪ {[(k,T)]})) with "[$HH]") as "HH".
-      { apply (auth_update_auth _ _ (H1 ∪ {[(k,T)]})).
-        apply gset_local_update. set_solver. }
-      iMod (own_update γ_s (● (H1 ∪ {[(k, T)]})) 
-             (● (H1 ∪ {[(k, T)]}) ⋅ ◯ (set_of_map Cr')) with "[$HH]") as "HH".
-      { apply (auth_update_alloc _ (H1 ∪ {[(k,T)]}) (set_of_map Cr')).
-        apply local_update_discrete. intros m Valid_H1 H1_eq.
-        split; try done. rewrite /(ε ⋅? m) in H1_eq.
-        destruct m. rewrite gset_op_union in H1_eq. 
-        rewrite left_id in H1_eq *; intros H1_eq.
-        rewrite <-H1_eq. 
-        rewrite /(set_of_map Cr' ⋅? Some (H1 ∪ {[k, T]})).
-        rewrite gset_op_union.
-        rewrite /(ε) in H1_eq. unfold ucmra_unit in H1_eq.
-        simpl in H1_eq.
-        assert ((k,T) ∈ set_of_map Cr') as H'.
-        { replace Cr'. apply set_of_map_member.
-          apply lookup_insert. } 
-        clear - H' Cr_sub_H1 Cr_sub_H1'. set_solver.
-        exfalso. clear -H1_eq. set_solver. }
-      (** Re-establish history_init **)   
-      iAssert (history_init (H1 ∪ {[(k, T)]})) with "[Hist]" as "Hist".
-      { iDestruct "Hist" as %Hist.
-        unfold history_init. iPureIntro.
-        clear -Hist. set_solver. }  
-      iDestruct "HnP_C" as "_".  
-      iDestruct "HH" as "(HH & HnP_C)".   
-      iAssert (⌜r ∈ domm I1⌝)%I as %r_in_I.
-      { by iPoseProof (inFP_domm _ _ _ with "[$FP_r] [$Hf]") as "H'". }
-      rewrite (big_sepS_delete _ (domm I1) r); last by eauto.
-      iDestruct "Hstar" as "(H_r & Hstar')".
-      iDestruct "H_r" as (br Cr'' Br'')"(Hl_r & Hlif_r & HnS_r)".
-      iAssert (⌜br = true⌝)%I as %Hbr.
-      { destruct br; try done.
-        iDestruct "Hlif_r" as (es' T')"(node' & _)".
-        iPoseProof ((node_sep_star r r) with "[$]") as "%".
-        contradiction. } replace br.
-      iDestruct "HnS_r" as (es' Ir Jr Rr) 
-            "(HnS_frac & HnS_si & HnS_FP & HnS_cl & HnS_oc & 
-                                        HnS_if & HnS_star & Hφ)".
-      iPoseProof (frac_eq with "[$HnP_frac] [$HnS_frac]") as "%".
-      destruct H as [Hes [Hc Hb]]. subst es'. subst Cr''. subst Br''.
-      (** Update contents-in-reach of r **)
-      set (Br' := <[k := T]>Br).
-      assert (Br' = <[k := T]>Br) as HBr'. try done.
-      iEval (rewrite <-beq_nat_refl) in "HnS_if".
-      iDestruct "HnS_if" as "(H' & H'' & H''')".
-      iDestruct "H'" as %Br_eq_H1. 
-      iDestruct "H''" as %Infz_rI.
-      iDestruct "H'''" as %Infz_rJ.
-      iAssert (⌜Br' = map_of_set (H1 ∪ {[(k, T)]})⌝)%I as %Br'_eq_H1.
-      { iPureIntro.
-        apply map_of_set_insert_eq; try done.
-        intros t. 
-        destruct Max_tsH1 as [Max_tsH1 _].
-        by pose proof Max_tsH1 k t. }
-      (** Case analysis on whether there exists n s.t. k in es(r,n) **)  
-      destruct (out_edgeset k es) eqn: Hes.
-      + (** Case : there exists n s.t. k in es(r,n) **)
-        apply out_edgeset_true in Hes.
-        destruct Hes as [n k_in_es].
-        iPoseProof (node_edgeset_self_empty with "node_r") as "%".
-        rename H into Self_es.
-        assert (n ≠ r) as n_neq_r.
-        { destruct (decide (n = r)); try done.
-          rewrite e in k_in_es.
-          clear -Self_es k_in_es.
-          set_solver. }
-        (** Case analysis on whether k was 
-            contained in old contents of r **)   
-        destruct (decide (Cr !!! k  = 0)) as [ Cr_k | Cr_k ]; last first.
-        * (** Case : k in old contents of r **) 
-          iEval (rewrite (big_sepS_delete (_) (KS) k); last by eauto) in "HnS_star".
-          iDestruct "HnS_star" as "(Hk & HnS_star')".
-          iAssert (⌜Br !!! k ≤ T⌝)%I as %Br_le_T.
-          { iDestruct "HnS_oc" as "(% & _)". rename H into HocI.
-            pose proof outflow_constraint_outset_I Ir es Cr Br k HocI Cr_k as H'.
-            iDestruct "Hφ" as "(_ & % & _)". rename H into Hφ1.
-            pose proof Hφ1 k as Hφ1. 
-            destruct Hφ1 as [Hφ1 | Hφ1]; try done.
-            destruct (Cr !! k) eqn: Hc.
-            assert (Hc' := Hc).
-            apply set_of_map_member in Hc.
-            assert ((k,u) ∈ H1) as Hu by set_solver.
-            unfold maxTS in Max_tsH1.
-            apply Max_tsH1 in Hu.
-            iPureIntro. rewrite Hφ1. 
-            rewrite /(Cr !!! k).
-            unfold finmap_lookup_total.
-            rewrite Hc'. simpl. lia.
-            rewrite /(Cr !!! k) in Cr_k.
-            unfold finmap_lookup_total in Cr_k.
-            rewrite Hc in Cr_k. simpl in Cr_k. lia. }
-          (** Update Maxnat Br resources **)  
-          iMod (own_update (γ_cir r k) (● (MaxNat (Br !!! k))) 
-                  (● (MaxNat (Br' !!! k))) with "Hk") as "Hk".
-          { apply (auth_update_auth _ _ (MaxNat (Br' !!! k))).
-            apply max_nat_local_update.
-            simpl. rewrite HBr'.
-            by rewrite lookup_total_insert. }        
-          iAssert ([∗ set] k0 ∈ KS, own (γ_cir r k0) 
-                      (● {| max_nat_car := Br' !!! k0 |}))%I 
-              with "[HnS_star' Hk]" as "HnS_star".
-          { iEval (rewrite (big_sepS_delete (_) (KS) k); last by eauto).
-            iFrame "Hk".        
-            iApply (big_opS_proper 
-                   (λ y, own (γ_cir r y) (● {| max_nat_car := Br' !!! y |}))
-                   (λ y, own (γ_cir r y) (● {| max_nat_car := Br !!! y |})) 
-                   (KS ∖ {[k]})).
-            intros x Hx. assert (x ≠ k) as H' by set_solver.
-            iFrame. iSplit. 
-            iIntros "H". iEval (rewrite HBr') in "H".
-            assert (<[k:=T]> Br !!! x = Br !!! x) as H''. 
-            { apply lookup_total_insert_ne; try done. } 
-            by iEval (rewrite H'') in "H".       
-            iIntros "H". iEval (rewrite HBr').
-            assert (<[k:=T]> Br !!! x = Br !!! x) as H''. 
-            { apply lookup_total_insert_ne; try done. } 
-            by iEval (rewrite H'').
-            done. }
-          (** Update fractional resources **)  
-          iMod ((frac_update γ_e γ_c γ_b r es Cr Br es Cr' Br') 
-                      with "[$HnP_frac $HnS_frac]") as "(HnP_frac & HnS_frac)".
-          (** Update J-interface of r. I-interface and 
-              R-interface of r do not change in this case **)            
-          set (Jr_temp := outflow_delete_KT Jr n k (Cr !!! k)).
-          set (Jr' := outflow_insert_KT Jr_temp n k T).
-          iPoseProof (node_edgeset_disjoint with "node_r") as "%".
-          rename H into Disj_es.
-          assert (Cr !!! k < T) as Crk_le_T. 
-          { destruct (Cr !! k) as [crk | ] eqn: Hcrk.
-            assert (Hcrk' := Hcrk).
-            apply set_of_map_member in Hcrk.
-            pose proof Cr_sub_H1 (k,crk) Hcrk as H'.
-            destruct Max_tsH1 as [H'' _].
-            pose proof H'' k crk H'.
-            apply lookup_total_correct in Hcrk'.
-            by rewrite Hcrk'.
-            rewrite /(Cr !!! k) in Cr_k.
-            unfold finmap_lookup_total in Cr_k.
-            rewrite Hcrk in Cr_k.
-            simpl in Cr_k. contradiction. }
-          iDestruct "HnS_oc" as "(% & % & % & % & %)".
-          rename H into OC_1. rename H2 into OC_2.
-          rename H3 into OC_3. rename H4 into Ole_I.
-          rename H5 into Ole_J.
-          (** Re-establish outflow_constraints of 
-              singleton interfaces of r **)
-          iAssert (outflow_constraints r Ir Jr' Rr es Cr' Br')%I 
-                                              as "HnS_oc".
-          { iPureIntro. split; last split; last split; 
-            last split; try done.
-            - intros n' k' t'. split.
-              + intros Hout.
-                apply OC_1 in Hout.
-                destruct Hout as [Hout1 [Hout2 Hout3]].
-                destruct (decide (k' = k)).
-                * replace k' in Hout2.
-                  contradiction.
-                * repeat split; try done.
-                  rewrite /(Cr' !!! k'). 
-                  unfold finmap_lookup_total.
-                  replace Cr'. rewrite lookup_insert_ne; try done.
-                  rewrite /(Br' !!! k'). 
-                  unfold finmap_lookup_total.
-                  rewrite HBr'. rewrite lookup_insert_ne; try done.
-              + intros [Hout1 [Hout2 Hout3]].
-                apply OC_1. split; try done.
-                destruct (decide (k' = k)).
-                * replace k'.
-                  rewrite e in Hout2. replace Cr' in Hout2.
-                  rewrite lookup_total_insert in Hout2.
-                  clear -Max_tsH1 Hout2.
-                  destruct Max_tsH1 as [_ Max_tsH1].
-                  lia.
-                * rewrite /(Cr' !!! k') in Hout2.
-                  unfold finmap_lookup_total in Hout2.
-                  replace Cr' in Hout2. 
-                  rewrite lookup_insert_ne in Hout2; try done.
-                  rewrite /(Br' !!! k') in Hout3.
-                  unfold finmap_lookup_total in Hout3; try done.
-                  rewrite HBr' in Hout3. 
-                  rewrite lookup_insert_ne in Hout3; try done.
-            - intros n' k' t'.
-              destruct (decide (n' = n)).
-              + replace n'.
-                assert (outset_KT Jr' n = 
-                      (outset_KT Jr n ∖ {[k, Cr !!! k]}) ∪ {[k, T]}) as Outset.
-                { pose proof outflow_insert_outset_KT Jr_temp n k T Jr' as Houts.
-                  assert (Jr' = outflow_insert_KT Jr_temp n k T) as HJr' by done.
-                  pose proof Houts HJr' as Hp.
-                  pose proof outflow_delete_outset_KT Jr n k (Cr !!! k) Jr_temp 
-                    as Houts'. 
-                  assert (Jr_temp = outflow_delete_KT Jr n k (Cr !!! k)) 
-                    as HJr_t by done.  
-                  pose proof Houts' HJr_t as [Hp' _].
-                  pose proof Ole_J n (k,Cr !!! k) as Ole_J.
-                  pose proof Hp' Ole_J as Hp'.
-                  by rewrite Hp' in Hp. }  
-                assert ((k',t') ∈ outset_KT Jr' n → 
-                       ((k',t') ∈ outset_KT Jr n) ∨ (k',t') = (k, T)) as Hkt'.
-                { intros Hout. rewrite Outset in Hout.
-                  set_solver. }
-                split.
-                * intros Hout. pose proof Hkt' Hout as Hkt'.
-                  destruct Hkt' as [Hkt' | Hkt'].
-                  ** apply OC_2 in Hkt'.
-                     destruct Hkt' as [Hkt'_1 [Hkt'_2 Hkt'_3]]. 
-                     split; try done. split.
-                     destruct (decide (k' = k)).
-                     rewrite e0 in Hkt'_2.
-                     rewrite e0 in Hout.
-                     rewrite <-Hkt'_2 in Hout.
-                     assert ((k, Cr !!! k) ∉ outset_KT Jr' n).
-                     { destruct (Cr !! k) eqn: Hc.
-                       assert (Hc' := Hc).
-                       apply set_of_map_member in Hc.
-                       assert ((k,u) ∈ H1) as H' by set_solver.
-                       destruct Max_tsH1 as [Max_tsH1 _].
-                       apply Max_tsH1 in H'.
-                       assert (Cr !!! k ≠ T).
-                       rewrite /(Cr !!! k).
-                       unfold finmap_lookup_total.
-                       rewrite Hc'. simpl. lia.
-                       set_solver.
-                       rewrite /(Cr !!! k) in Cr_k.
-                       unfold finmap_lookup_total in Cr_k.
-                       rewrite Hc in Cr_k. simpl in Cr_k. lia. }
-                     contradiction.
-                     replace Cr'. 
-                     rewrite lookup_total_insert_ne; try done.
-                     destruct (decide (k' = k)).
-                     rewrite e0.
-                     replace Cr'.
-                     rewrite lookup_total_insert. 
-                     by destruct Max_tsH1 as [_ H'].
-                     replace Cr'.
-                     rewrite lookup_total_insert_ne; try done.
-                  ** inversion Hkt'.
-                     repeat split; try done.
-                     replace Cr'.
-                     rewrite lookup_total_insert; try done.
-                     replace Cr'.
-                     rewrite lookup_total_insert. 
-                     by destruct Max_tsH1 as [_ H'].
-                * intros [Hk1 [Hk2 Hk3]].
-                  destruct (decide (k' = k)).
-                  ** replace k'.
-                     rewrite e0 in Hk1.
-                     rewrite e0 in Hk2.
-                     replace Cr' in Hk2. 
-                     rewrite lookup_total_insert in Hk2.
-                     replace t'. rewrite Outset.
-                     set_solver.
-                  ** replace Cr' in Hk2.
-                     rewrite lookup_total_insert_ne in Hk2; try done.
-                     replace Cr' in Hk3.
-                     rewrite lookup_total_insert_ne in Hk3; try done.
-                     assert (k' ∈ es !!! n ∧ Cr !!! k' = t' ∧ Cr !!! k' > 0) 
-                                        as Hkt; try done.
-                     apply OC_2 in Hkt.
-                     rewrite Outset.
-                     clear -Hkt n0. set_solver.
-              + assert (outset_KT Jr' n' = outset_KT Jr n') as Outset.
-                { pose proof outflow_insert_outset_ne_KT Jr_temp n k T Jr' n' n0
-                                                                 as Houts.
-                  assert (Jr' = outflow_insert_KT Jr_temp n k T) as HJr' by done.
-                  pose proof Houts HJr' as Hp.
-                  pose proof outflow_delete_outset_ne_KT Jr n k (Cr !!! k) 
-                                            Jr_temp n' n0 as Houts'. 
-                  assert (Jr_temp = outflow_delete_KT Jr n k (Cr !!! k)) 
-                    as HJr_t by done.  
-                  pose proof Houts' HJr_t as Hp'.
-                  by rewrite Hp' in Hp. }
-                rewrite Outset.
-                split.
-                * intros Hout.
-                  apply OC_2 in Hout.
-                  destruct Hout as [Hout1 [Hout2 Hout3]].
-                  split; try done.
-                  destruct (decide (k' = k)).
-                  ** rewrite e in Hout1.
-                     pose proof Disj_es n' n n0 as H'.
-                     clear -H' Hout1 k_in_es. 
-                     set_solver.
-                  ** replace Cr'.
-                     rewrite lookup_total_insert_ne; try done.
-                * intros [Hout1 [Hout2 Hout3]].
-                  destruct (decide (k' = k)).
-                  ** rewrite e in Hout1.
-                     pose proof Disj_es n' n n0 as H'.
-                     clear -H' Hout1 k_in_es. 
-                     set_solver.
-                  ** replace Cr' in Hout2.
-                     rewrite lookup_total_insert_ne in Hout2; try done.
-                     replace Cr' in Hout3.
-                     rewrite lookup_total_insert_ne in Hout3; try done.
-                     apply OC_2.
-                     split; try done.
-            - intros n' kt'. subst Jr'. unfold outflow_insert_KT.
-              unfold out at 1, out_map at 1. simpl.
-              destruct (decide (n' = n)).
-              + subst n'. rewrite nzmap_lookup_total_insert.
-                destruct (decide (kt' = (k,T))).
-                * subst kt'. rewrite nzmap_lookup_total_insert.
-                  subst Jr_temp. unfold outflow_delete_KT.
-                  unfold out at 1, out_map at 1.
-                  simpl. rewrite nzmap_lookup_total_insert.
-                  rewrite nzmap_lookup_total_decrement_ne; last first.
-                  clear -Crk_le_T. intros H'; inversion H'; lia.
-                  pose proof Ole_J n (k,T) as Ole_J.
-                  assert (out Jr n !1 (k,T) = 0 ∨ out Jr n !1 (k,T) = 1) as H'.
-                  { clear -Ole_J.
-                    assert (∀ (x: nat), x ≤ 1 → x = 0 ∨ x = 1) as H'.
-                    lia. by apply H'. }
-                  destruct H' as [H' | H'].
-                  ** rewrite H'. lia.
-                  ** assert ((k,T) ∈ outset_KT Jr n) as H''.
-                     { unfold outset_KT, KT_flows.dom_ms.
-                       rewrite nzmap_elem_of_dom.
-                       destruct (out Jr n !! (k,T)) eqn: Hout.
-                       by exists n0.
-                       unfold nzmap_total_lookup in H'.
-                       rewrite Hout in H'. simpl in H'.
-                       unfold ccmunit, ccm_unit, nat_unit in H'.
-                       lia. }
-                     apply OC_2 in H''. destruct H'' as [_ [H'' _]].
-                     clear -H'' Crk_le_T. lia. 
-                * rewrite nzmap_lookup_total_insert_ne; try done.
-                  subst Jr_temp. unfold outflow_delete_KT.
-                  unfold out at 1, out_map at 1. simpl.
-                  rewrite nzmap_lookup_total_insert.
-                  destruct (decide (kt' = (k, Cr !!! k))).
-                  ** subst kt'. rewrite nzmap_lookup_total_decrement.
-                     pose proof Ole_J n (k, Cr !!! k) as Ole_J. 
-                     clear -Ole_J. lia.
-                  ** rewrite nzmap_lookup_total_decrement_ne; try done.
-              + rewrite nzmap_lookup_total_insert_ne; try done.
-                rewrite nzmap_lookup_total_insert_ne; try done.
-                pose proof Ole_J n' kt' as Ole_J.
-                by unfold out in Ole_J. }     
-          iAssert (inFP γ_f n)%I as "#FP_n".
-          { iApply "HnS_cl". iPureIntro.
-          clear -k_in_es. set_solver. }
-          iAssert (⌜n ∈ domm I1⌝)%I as %n_in_I.
-          { by iPoseProof (inFP_domm _ _ _ with "[$FP_n] [$Hf]") as "H'". }
-          rewrite (big_sepS_delete _ (domm I1 ∖ {[r]}) n); last by set_solver.
-          iDestruct "Hstar'" as "(H_n & Hstar')".
-          iDestruct "H_n" as (bn Cn Bn)"(Hl_n & Hlif_n & HnS_n)".
-          iDestruct "HnS_n" as (es_n In Jn Rn) 
-            "(HnS_fracn & HnS_sin & HnS_FPn & HnS_cln & HnS_ocn & 
-                                        HnS_ifn & HnS_starn & Hφn)".
-          (** Update J-interface of n **)                              
-          set (Jn_temp := inflow_delete_KT Jn n k (Cr !!! k)).
-          set (Jn' := inflow_insert_KT Jn_temp n k T).
-          (** Re-establish outflow_constraints of 
-              singleton interfaces of n **)
-          iAssert (outflow_constraints n In Jn' Rn es_n Cn Bn)%I
-            with "[HnS_ocn]" as "HnS_ocn".
-          { iDestruct "HnS_ocn" as "(% & % & %)".
-            rename H into OCn_1. rename H2 into OCn_2.
-            rename H3 into OCn_3. 
-            iPureIntro. split; last split; try done. }
-          (** Update singleton interfaces of r and n **)  
-          iAssert (singleton_interfaces_ghost_state γ_I γ_J γ_R r Ir Jr' Rr
-            ∗ singleton_interfaces_ghost_state γ_I γ_J γ_R n In Jn' Rn)%I 
-                    with "[HnS_si HnS_sin]" as "(HnS_si & HnS_sin)".
-          { unfold singleton_interfaces_ghost_state. 
-            iDestruct "HnS_si" as "(HrI & HrJ & HrR & % & % & %)".
-            iDestruct "HnS_sin" as "(HnI & HnJ & HnR & % & % & %)".
-            rename H into Domm_Ir. rename H2 into Domm_Jr.
-            rename H3 into Domm_Rr. rename H4 into Domm_In.
-            rename H5 into Domm_Jn. rename H6 into Domm_Rn.
-            assert (Jn_temp = inflow_delete_KT Jn n k (Cr !!! k)) 
-                          as HJn't by done.
-            assert (Jn' = inflow_insert_KT Jn_temp n k T) as HJn' by done.
-            pose proof (inflow_delete_domm Jn n k (Cr !!! k) Jn_temp HJn't) 
-                                          as Domm_Jntemp .
-            pose proof (inflow_insert_domm Jn_temp n k T Jn' HJn')
-                                          as Domm_Jn'.
-            assert (domm Jn' = domm Jn) as Domm_Jn'_eq_Jn.
-            { clear -Domm_Jn' Domm_Jntemp Domm_Jn. set_solver. }
-            assert (domm Jn_temp = domm Jn) as Domm_Jntemp_eq_Jn.
-            { clear -Domm_Jn' Domm_Jntemp Domm_Jn. set_solver. }
-            rewrite Domm_Jn'_eq_Jn. iFrame.
-            iCombine "HrJ HnJ" as "HrnJ".
-            iPoseProof (own_valid with "[$HrnJ]") as "%".
-            rename H into Valid_rnJ. 
-            rewrite auth_frag_valid in Valid_rnJ *; intros Valid_rnJ.
-            assert (Jr ⋅ Jn = Jr_temp ⋅ Jn_temp) as H'.
-            { apply (flowint_delete_eq_KT Jr Jr_temp _ _ n k (Cr !!! k));
-                        try done.
-              clear -Domm_Jn. set_solver.
-              pose proof Ole_J n (k, Cr !!! k) as Ole_J.
-              assert ((k, Cr !!! k) ∈ outset_KT Jr n) as H''.
-              { apply OC_2. repeat split; try done. lia. } 
-              unfold outset_KT, KT_flows.dom_ms in H''.
-              rewrite nzmap_elem_of_dom_total in H'' *; intros H''.
-              unfold ccmunit, ccm_unit in H''; simpl in H''; 
-              unfold nat_unit in H''.
-              clear -Ole_J H''.
-              assert (∀ (x: nat), x ≤ 1 → x ≠ 0 → 1 ≤ x) as H'. lia.
-              apply H'; try done. }
-            iEval (rewrite H') in "HrnJ".  
-            iPoseProof (own_valid with "[$HrnJ]") as "%".
-            rename H into Valid_rnJtemp. 
-            rewrite auth_frag_valid in Valid_rnJtemp *; intros Valid_rnJtemp.
-            assert (Jr_temp ⋅ Jn_temp = Jr' ⋅ Jn') as H''.
-            { apply (flowint_insert_eq_KT Jr_temp Jr' _ _ n k T);
-                         try done.
-              clear -Domm_Jntemp. set_solver.
-              unfold domm, dom, flowint_dom. 
-              subst Jr_temp. unfold outflow_delete_KT.
-              unfold inf_map at 1. simpl.
-              unfold domm, dom, flowint_dom in Domm_Jr.
-              clear -Domm_Jr. set_solver. }
-            iEval (rewrite H'') in "HrnJ".
-            iEval (rewrite auth_frag_op) in "HrnJ".
-            iDestruct "HrnJ" as "(HrJ & HnJ)". iFrame "∗%". }
-          iDestruct "Inf_R" as %Inf_R.
-          iPoseProof ((auth_own_incl γ_R R1 Rr) with "[HR HnS_si]")
-              as (Ro) "%". 
-          { unfold singleton_interfaces_ghost_state.
-            iDestruct "HnS_si" as "(_ & _ & H' & _)". 
-            iFrame. } rename H into Incl_R1.
-          iPoseProof (own_valid with "HR") as "%".
-          rename H into Valid_R1.
-          iAssert (⌜domm Rr = {[r]}⌝)%I as "%".
-          { by iDestruct "HnS_si" as "(_&_&_&_&_&H')". }
-          rename H into Domm_Rr.
-          (** Re-establish φ_i's of r **)
-          iAssert (⌜φ0 Br' (T+1)⌝ ∗ ⌜φ1 Br' Cr' Ir⌝ ∗ ⌜φ2 r Br' Ir⌝ ∗ ⌜φ3 r Br' Jr'⌝ 
-                  ∗ ⌜φ4 r Br' Rr⌝ ∗ ⌜φ5 r Rr⌝)%I with "[Hφ]" as "Hφ".
-          { iDestruct "Hφ" as %Hφ. 
-            destruct Hφ as [Hφ0 [Hφ1 [Hφ2 [Hφ3 [Hφ4 Hφ5]]]]].
-            iPureIntro. repeat split; try done.
-            - intros k'. destruct (decide (k' = k)).
-              rewrite HBr'. rewrite e. rewrite lookup_total_insert. lia.
-              rewrite HBr'. rewrite lookup_total_insert_ne; try done.
-              pose proof Hφ0 k' as H'. clear -H'.
-              apply (Nat.le_trans _ T _); try done. lia. 
-            - intros k'. pose proof Hφ1 k' as Hφ1.
-              destruct Hφ1 as [Hφ1 | Hφ1].
-              by left.
-              destruct (decide (k' = k)).
-              replace k'. right.
-              replace Cr'. rewrite HBr'.
-              rewrite lookup_total_insert.
-              by rewrite lookup_total_insert.
-              right.    
-              replace Cr'. rewrite HBr'.
-              rewrite lookup_total_insert_ne; try done.
-              rewrite lookup_total_insert_ne; try done.
-            - intros k' t' Hins.
-              pose proof Infz_rI r as Infz_rI.
-              rewrite Infz_rI in Hins.
-              exfalso. clear -Hins. set_solver.
-            - intros k' t' Hins.
-              pose proof Infz_rJ r as Infz_rJ.
-              assert (inset_KT Jr' r = inset_KT Jr r) as H'.
-              { assert (inset_KT Jr_temp r = inset_KT Jr r) as H'.
-                apply (outflow_delete_inf_eq_KT _ n k (Cr !!! k)); try done.
-                assert (inset_KT Jr' r = inset_KT Jr_temp r) as H''.
-                apply (outflow_insert_inf_eq_KT _ n k T); try done.
-                by rewrite <-H'. }
-              rewrite H' in Hins. rewrite Infz_rJ in Hins.
-              exfalso. clear -Hins. set_solver.
-            - intros k'. right.
-              apply (inset_monotone R1 Rr Ro); try done.
-              by rewrite <-auth_auth_valid.
-              pose proof Inf_R r k' as Inf_R.
-              by rewrite <-beq_nat_refl in Inf_R.
-              rewrite Domm_Rr. clear. set_solver. } 
-          (** Re-establish φ_i's of n **)    
-          iAssert (⌜φ0 Bn (T+1)⌝ ∗ ⌜φ1 Bn Cn In⌝ ∗ ⌜φ2 n Bn In⌝ ∗ ⌜φ3 n Bn Jn'⌝ 
-                  ∗ ⌜φ4 n Bn Rn⌝ ∗ ⌜φ5 n Rn⌝)%I with "[Hφn]" as "Hφn".
-          { iDestruct "Hφn" as %Hφ. 
-            destruct Hφ as [Hφ0 [Hφ1 [Hφ2 [Hφ3 [Hφ4 Hφ5]]]]].
-            iPureIntro. repeat split; try done.
-            intros k'. pose proof Hφ0 k' as H'.
-            apply (Nat.le_trans _ T _); try done. lia. 
-            intros k' t'. 
-            assert (inset_KT Jn' n ⊆ inset_KT Jn n ∪ {[k, T]}) as Inset.
-            { assert (Jn' = inflow_insert_KT Jn_temp n k T) as HJn' by done.
-              pose proof inflow_insert_inset_KT Jn_temp n k T Jn' HJn' as Hin.
-              assert (Jn_temp = inflow_delete_KT Jn n k (Cr !!! k)) 
-                    as HJn_t by done.  
-              pose proof inflow_delete_inset_KT Jn n k (Cr !!! k) 
-                                          Jn_temp HJn_t as Hin'. 
-              destruct (decide (inf Jn n !1 (k, Cr !!! k) ≤ 1)) as [Hi1 | Hi1].
-              destruct Hin' as [Hin' _].
-              apply Hin' in Hi1. rewrite Hi1 in Hin.
-              clear -Hin. set_solver.
-              destruct Hin' as [_ Hin']. apply not_le in Hi1.
-              apply Hin' in Hi1. rewrite Hi1 in Hin.
-              clear -Hin. set_solver. } 
-            assert ((k',t') ∈ inset_KT Jn' n → 
-                       ((k',t') ∈ inset_KT Jn n) ∨ (k',t') = (k, T)) as Hkt'.
-            { intros Hin. clear -Hin Inset. set_solver. }
-            intros Hin. apply Hkt' in Hin.
-            destruct Hin as [Hin | Hin].
-            by pose proof Hφ3 k' t' Hin as Hφ3.
-            inversion Hin.
-            by pose proof Hφ0 k. }
-          (** Linearization **)    
-          iMod "AU" as (t' H')"[MCS [_ Hclose]]".
-          iAssert (⌜t' = T⌝)%I as %Ht'. 
-          { iPoseProof ((auth_agree γ_te) with "[MCS_auth] [MCS]") as "%".
-            unfold MCS_auth. by iDestruct "MCS_auth" as "(H' & _)".
-            by iDestruct "MCS" as "(H' & _)".
-            by iPureIntro. } replace t'.
-          iAssert (⌜H' = H1⌝)%I as %H1'.
-          { iPoseProof ((auth_agree' γ_he) with "[MCS_auth] [MCS]") as "%".
-            unfold MCS_auth. by iDestruct "MCS_auth" as "(_ & H'')".
-            by iDestruct "MCS" as "(_ & H')".
-            by iPureIntro. } replace H'.
-          iDestruct "MCS" as "(MCS◯t & MCS◯h)".
-          iDestruct "MCS_auth" as "(MCS●t & MCS●h)".
-          iMod ((auth_update γ_te (T+1) T T) with "MCS●t MCS◯t") 
-                                              as "(MCS●t & MCS◯t)".
-          iMod ((auth_update' γ_he (H1 ∪ {[(k, T)]}) H1 H1) with "MCS●h MCS◯h") 
-                                              as "(MCS●h & MCS◯h)".
-          iCombine "MCS◯t MCS◯h" as "MCS".
-          iCombine "MCS●t MCS●h" as "MCS_auth".
-          iMod ("Hclose" with "MCS") as "HΦ".
-          (** Close the invariant **)            
-          iModIntro.
-          iSplitR "HΦ node_r HnP_t HnP_C HnP_frac".
-          { iNext. iExists (T+1), (H1 ∪ {[(k, T)]}), I1, J1, R1.
-            iFrame "∗ %".   
-            rewrite (big_sepS_delete _ (domm I1) r); last by eauto.
-            iSplitL "Hl_r Hlif_r HnS_cl HnS_star Hφ HnS_frac HnS_oc HnS_si".
-            { iExists true, Cr', Br'. iFrame.
-              unfold nodeShared. iExists es, Ir, Jr', Rr.
-              iFrame "∗#". iEval (rewrite <-beq_nat_refl). 
-              iFrame "%∗". }        
-            rewrite (big_sepS_delete _ (domm I1 ∖ {[r]}) n); last by set_solver.
-            iSplitL "Hl_n Hlif_n HnS_cln HnS_starn Hφn HnS_fracn HnS_ocn 
-                        HnS_sin HnS_ifn".
-            { iExists bn, Cn, Bn. iFrame. iExists es_n, In, Jn', Rn.
-              iFrame "∗#". assert (n =? r = false) as Hnr. 
-              { by rewrite beq_nat_false_iff. } 
-              by rewrite Hnr. }
-            iApply (big_sepS_mono (λ y, ∃ (bn0 : bool) (Cn0 Bn0 : gmap K natUR),
-                                      lockLoc y ↦ #bn0
-                                    ∗ (if bn0 then True else
-                                       nodePred γ_e γ_c γ_b γ_t γ_s lc r y Cn0 Bn0)
-                                    ∗ nodeShared γ_I γ_J γ_R γ_e γ_c γ_b γ_f γ_cir
-                                              r y Cn0 Bn0 T H1 )%I
-                                   (λ y, ∃ (bn0 : bool) (Cn0 Bn0 : gmap K natUR),
-                                      lockLoc y ↦ #bn0
-                                    ∗ (if bn0 then True else
-                                       nodePred γ_e γ_c γ_b γ_t γ_s lc r y Cn0 Bn0)
-                                    ∗ nodeShared γ_I γ_J γ_R γ_e γ_c γ_b γ_f γ_cir
-                                              r y Cn0 Bn0 (T+1) (H1 ∪ {[(k, T)]}) )%I
-                                   (domm I1 ∖ {[r]} ∖ {[n]})); try done.
-            intros y y_dom. assert (y ≠ r) as Hy by set_solver. iFrame.
-            iIntros "Hstar". iDestruct "Hstar" as (b C B)"(Hl & Hlif & HnS)".
-            iExists b, C, B. iFrame. 
-            iDestruct "HnS" as (esy Iy Jy Ry)"(HnS_frac & HnS_si & HnS_FP 
-                          & HnS_cl & HnS_oc & HnS_if & HnS_star & Hφ0 & Hφ)".
-            iExists esy, Iy, Jy, Ry. iFrame.
-            iDestruct "Hφ0" as %Hφ0. 
-            assert (y =? r = false) as Hyr by (rewrite beq_nat_false_iff; done).
-            iEval (rewrite Hyr). iPureIntro. split; try done.
-            intros k'. pose proof Hφ0 k'. 
-            apply (Nat.le_trans _ T _); try done. lia. } 
-          wp_pures. 
-          (** Unlock node r **) 
-          awp_apply (unlockNode_spec_high with "[] [] [HnP_t HnP_C HnP_frac node_r]")
-                without "HΦ"; try done. iExists es, (T + 1). iFrame.
-                by iEval (rewrite <-beq_nat_refl).
-          iAaccIntro with ""; try eauto with iFrame.
-        * iEval (rewrite (big_sepS_delete (_) (KS) k); last by eauto) in "HnS_star".
-          iDestruct "HnS_star" as "(Hk & HnS_star')".
-          iAssert (⌜Br !!! k ≤ T⌝)%I as %Br_le_T. 
-          { 
-            iDestruct "Hφ" as "(% & _)".
-            iPureIntro. rename H into H'.
-            by pose proof H' k. }
-          iMod (own_update (γ_cir r k) (● (MaxNat (Br !!! k))) 
-                    (● (MaxNat (Br' !!! k))) with "Hk") as "Hk".
-          { apply (auth_update_auth _ _ (MaxNat (Br' !!! k))).
-            apply max_nat_local_update.
-            simpl. rewrite HBr'.
-            by rewrite lookup_total_insert. }        
-          iAssert ([∗ set] k0 ∈ KS, own (γ_cir r k0) 
-                      (● {| max_nat_car := Br' !!! k0 |}))%I 
-              with "[HnS_star' Hk]" as "HnS_star".
-          { iEval (rewrite (big_sepS_delete (_) (KS) k); last by eauto).
-            iFrame "Hk".        
-            iApply (big_opS_proper 
-                 (λ y, own (γ_cir r y) (● {| max_nat_car := Br' !!! y |}))
-                 (λ y, own (γ_cir r y) (● {| max_nat_car := Br !!! y |})) 
-                 (KS ∖ {[k]})).
-            intros x Hx. assert (x ≠ k) as H' by set_solver.
-            iFrame. iSplit. 
-            iIntros "H". iEval (rewrite HBr') in "H".
-            assert (<[k:=T]> Br !!! x = Br !!! x) as H''. 
-            { apply lookup_total_insert_ne; try done. } 
-            by iEval (rewrite H'') in "H".       
-            iIntros "H". iEval (rewrite HBr').
-            assert (<[k:=T]> Br !!! x = Br !!! x) as H''. 
-            { apply lookup_total_insert_ne; try done. } 
-            by iEval (rewrite H'').
-            done. }
-          iMod ((frac_update γ_e γ_c γ_b r es Cr Br es Cr' Br') 
-                      with "[$HnP_frac $HnS_frac]") as "(HnP_frac & HnS_frac)".
-          set (Ir' := outflow_delete_KT Ir n k (Br !!! k)).
-          set (Jr' := outflow_insert_KT Jr n k T).
-          iPoseProof (node_edgeset_disjoint with "node_r") as "%".
-          rename H into Disj_es. 
-          iDestruct "HnS_oc" as "(% & % & % & % & %)".
-          rename H into OC_1. rename H2 into OC_2.
-          rename H3 into OC_3. rename H4 into Ole_I.
-          rename H5 into Ole_J.
-          assert (Cr !!! k < T) as Crk_le_T. 
-          { rewrite Cr_k.
-            by destruct Max_tsH1 as [_ H'']. }
-          iAssert (outflow_constraints r Ir' Jr' Rr es Cr' Br')%I 
-                                              as "HnS_oc".
-          { iPureIntro. split; last split; last split; 
-            last split; try done.
-            - intros n' k' t'.
-              destruct (decide (n' = n)).
-              + assert (outset_KT Ir' n = (outset_KT Ir n) ∖ {[(k, Br !!! k)]}) 
-                                                                   as Out_eq.
-                { pose proof outflow_delete_outset_KT Ir n k (Br !!! k) Ir' as H'. 
-                  assert (Ir' = outflow_delete_KT Ir n k (Br !!! k)) as HIr' by done.
-                  pose proof H' HIr' as [Hout _].
-                  pose proof Ole_I n (k, Br !!! k) as Ole_I.
-                  by apply Hout in Ole_I. }
-                replace n'. split.
-                * intros Hout.
-                  assert ((k', t') ∈ outset_KT Ir n) as Hkt'.
-                  { clear -Out_eq Hout. set_solver. }
-                  apply OC_1 in Hkt'.
-                  destruct (decide (k' = k)).
-                  rewrite e0 in Hout.
-                  destruct Hkt' as [_ [_ Hkt']].
-                  rewrite e0 in Hkt'.
-                  rewrite <-Hkt' in Hout.
-                  clear -Hout Out_eq.
-                  set_solver.
-                  replace Cr'.
-                  rewrite lookup_total_insert_ne; try done.
-                  rewrite HBr'.
-                  rewrite lookup_total_insert_ne; try done.
-                * intros Hout.
-                  destruct (decide (k' = k)).
-                  destruct Hout as [_ [Hout _]].
-                  rewrite e0 in Hout.
-                  replace Cr' in Hout.
-                  rewrite lookup_total_insert in Hout.
-                  destruct Max_tsH1 as [_ H']. lia.
-                  replace Cr' in Hout.
-                  rewrite lookup_total_insert_ne in Hout; try done.
-                  rewrite HBr' in Hout.
-                  rewrite lookup_total_insert_ne in Hout; try done.
-                  apply OC_1 in Hout.
-                  clear -Hout Out_eq n0. set_solver.
-              + assert (outset_KT Ir' n' = outset_KT Ir n') as Out_eq.
-                { assert (Ir' = outflow_delete_KT Ir n k (Br !!! k)) 
-                                                        as HIr' by done.
-                  by pose proof outflow_delete_outset_ne_KT Ir n k (Br !!! k)
-                                                   Ir' n' n0 HIr' as H'. }
-                rewrite Out_eq.
-                split.
-                * intros Hout.
-                  apply OC_1 in Hout.
-                  destruct (decide (k' = k)).
-                  destruct Hout as [H' _].
-                  rewrite e in H'.
-                  pose proof Disj_es n' n n0 as H''.
-                  clear -H'' H' k_in_es. 
-                  set_solver.
-                  replace Cr'.
-                  rewrite lookup_total_insert_ne; try done.
-                  rewrite HBr'.
-                  rewrite lookup_total_insert_ne; try done.
-                * intros Hout.
-                  destruct (decide (k' = k)).
-                  destruct Hout as [H' _].
-                  rewrite e in H'.
-                  pose proof Disj_es n' n n0 as H''.
-                  clear -H'' H' k_in_es. 
-                  set_solver.
-                  replace Cr' in Hout.
-                  rewrite lookup_total_insert_ne in Hout; try done.
-                  rewrite HBr' in Hout.
-                  rewrite lookup_total_insert_ne in Hout; try done.
-                  by apply OC_1 in Hout.
-            - intros n' k' t'.
-              destruct (decide (n' = n)).
-              + assert (outset_KT Jr' n = outset_KT Jr n ∪ {[k, T]}) as Outset.
-                { assert (Jr' = outflow_insert_KT Jr n k T) as HJr' by done.
-                  by pose proof outflow_insert_outset_KT Jr n k T 
-                                              Jr' HJr' as Houts. }
-                replace n'.  
-                assert ((k',t') ∈ outset_KT Jr' n → 
-                       ((k',t') ∈ outset_KT Jr n) ∨ (k',t') = (k, T)) as Hkt'.
-                { intros Hout. rewrite Outset in Hout.
-                  set_solver. }
-                split.
-                * intros Hout. pose proof Hkt' Hout as Hkt'.
-                  destruct Hkt' as [Hkt' | Hkt'].
-                  ** apply OC_2 in Hkt'.
-                     destruct Hkt' as [Hkt'_1 [Hkt'_2 Hkt'_3]]. 
-                     split; try done.
-                     destruct (decide (k' = k)).
-                     rewrite e0 in Hkt'_3.
-                     clear -Cr_k Hkt'_3. lia.
-                     replace Cr'. 
-                     rewrite lookup_total_insert_ne; try done.
-                  ** inversion Hkt'.
-                     repeat split; try done.
-                     replace Cr'.
-                     rewrite lookup_total_insert; try done.
-                     replace Cr'.
-                     rewrite lookup_total_insert; try done.
-                     by destruct Max_tsH1 as [_ H'].
-                * intros [Hk1 [Hk2 Hk3]].
-                  destruct (decide (k' = k)).
-                  ** replace k'.
-                     rewrite e0 in Hk1.
-                     rewrite e0 in Hk2.
-                     replace Cr' in Hk2. 
-                     rewrite lookup_total_insert in Hk2.
-                     replace t'. rewrite Outset.
-                     set_solver.
-                  ** replace Cr' in Hk2.
-                     rewrite lookup_total_insert_ne in Hk2; try done.
-                     replace Cr' in Hk3.
-                     rewrite lookup_total_insert_ne in Hk3; try done.
-                     assert (k' ∈ es !!! n ∧ Cr !!! k' = t' ∧ Cr !!! k' > 0) 
-                                        as Hkt; try done.
-                     apply OC_2 in Hkt.
-                     rewrite Outset.
-                     clear -Hkt n0. set_solver.
-              + assert (outset_KT Jr' n' = outset_KT Jr n') as Outset.
-                { assert (Jr' = outflow_insert_KT Jr n k T) as HJr' by done.
-                  by pose proof outflow_insert_outset_ne_KT Jr n k T 
-                                                Jr' n' n0 HJr' as Houts. }
-                rewrite Outset.
-                split.
-                * intros Hout.
-                  apply OC_2 in Hout.
-                  destruct Hout as [Hout1 [Hout2 Hout3]].
-                  split; try done.
-                  destruct (decide (k' = k)).
-                  ** rewrite e in Hout1.
-                     pose proof Disj_es n' n n0 as H'.
-                     clear -H' Hout1 k_in_es. 
-                     set_solver.
-                  ** replace Cr'.
-                     rewrite lookup_total_insert_ne; try done.
-                * intros [Hout1 [Hout2 Hout3]].
-                  destruct (decide (k' = k)).
-                  ** rewrite e in Hout1.
-                     pose proof Disj_es n' n n0 as H'.
-                     clear -H' Hout1 k_in_es. 
-                     set_solver.
-                  ** replace Cr' in Hout2.
-                     rewrite lookup_total_insert_ne in Hout2; try done.
-                     replace Cr' in Hout3.
-                     rewrite lookup_total_insert_ne in Hout3; try done.
-                     apply OC_2.
-                     split; try done.
-            - intros n' kt'. subst Ir'. unfold outflow_delete_KT.
-              unfold out at 1, out_map at 1. simpl.
-              destruct (decide (n' = n)).
-              + subst n'. rewrite nzmap_lookup_total_insert.
-                destruct (decide (kt' = (k,Br !!! k))).
-                * subst kt'. rewrite nzmap_lookup_total_decrement.
-                  pose proof Ole_I n (k, Br !!! k) as Ole_I.
-                  clear -Ole_I. lia.
-                * rewrite nzmap_lookup_total_decrement_ne; try done.
-              + rewrite nzmap_lookup_total_insert_ne; try done.
-                pose proof Ole_I n' kt' as Ole_I.
-                by unfold out in Ole_I.
-            - intros n' kt'. subst Jr'. unfold outflow_insert_KT.
-              unfold out at 1, out_map at 1. simpl.
-              destruct (decide (n' = n)).
-              + subst n'. rewrite nzmap_lookup_total_insert.
-                destruct (decide (kt' = (k, T))).
-                * subst kt'. rewrite nzmap_lookup_total_insert.
-                  pose proof Ole_J n (k, T) as Ole_J.
-                  assert (out Jr n !1 (k,T) = 0 ∨ out Jr n !1 (k,T) = 1) as H'.
-                  { clear -Ole_J.
-                    assert (∀ (x: nat), x ≤ 1 → x = 0 ∨ x = 1) as H'.
-                    lia. by apply H'. }
-                  destruct H' as [H' | H'].
-                  ** rewrite H'. lia.
-                  ** assert ((k,T) ∈ outset_KT Jr n) as H''.
-                     { unfold outset_KT, KT_flows.dom_ms.
-                       rewrite nzmap_elem_of_dom.
-                       destruct (out Jr n !! (k,T)) eqn: Hout.
-                       by exists n0.
-                       unfold nzmap_total_lookup in H'.
-                       rewrite Hout in H'. simpl in H'.
-                       unfold ccmunit, ccm_unit, nat_unit in H'.
-                       lia. }
-                     apply OC_2 in H''. destruct H'' as [_ [H'' _]].
-                     clear -H'' Crk_le_T. lia. 
-                * rewrite nzmap_lookup_total_insert_ne; try done.
-              + rewrite nzmap_lookup_total_insert_ne; try done.
-                pose proof Ole_J n' kt' as Ole_J.
-                by unfold out in Ole_J. }
-          iAssert (inFP γ_f n)%I as "#FP_n". 
-          { iApply "HnS_cl". iPureIntro.
-            clear -k_in_es. set_solver. }
-          iAssert (⌜n ∈ domm I1⌝)%I as %n_in_I.
-          { by iPoseProof (inFP_domm _ _ _ with "[$FP_n] [$Hf]") as "H'". }
-          rewrite (big_sepS_delete _ (domm I1 ∖ {[r]}) n); last by set_solver.
-          iDestruct "Hstar'" as "(H_n & Hstar')".
-          iDestruct "H_n" as (bn Cn Bn)"(Hl_n & Hlif_n & HnS_n)".
-          iDestruct "HnS_n" as (es_n In Jn Rn) 
-            "(HnS_fracn & HnS_sin & HnS_FPn & HnS_cln & HnS_ocn & 
-                                        HnS_ifn & HnS_starn & Hφn)".
-          set (In' := inflow_delete_KT In n k (Br !!! k)).
-          set (Jn' := inflow_insert_KT Jn n k T).
-          iAssert (singleton_interfaces_ghost_state γ_I γ_J γ_R r Ir' Jr' Rr
-            ∗ singleton_interfaces_ghost_state γ_I γ_J γ_R n In' Jn' Rn)%I 
-                    with "[HnS_si HnS_sin]" as "(HnS_si & HnS_sin)".
-          { unfold singleton_interfaces_ghost_state. 
-            iDestruct "HnS_si" as "(HrI & HrJ & HrR & % & % & %)".
-            iDestruct "HnS_sin" as "(HnI & HnJ & HnR & % & % & %)".
-            rename H into Domm_Ir. rename H2 into Domm_Jr.
-            rename H3 into Domm_Rr. rename H4 into Domm_In.
-            rename H5 into Domm_Jn. rename H6 into Domm_Rn.
-            assert (Jn' = inflow_insert_KT Jn n k T) as HJn' by done.
-            pose proof (inflow_insert_domm Jn n k T Jn' HJn')
-                                          as Domm_Jn'.
-            assert (domm Jn' = domm Jn) as Domm_Jn'_eq_Jn.
-            { clear -Domm_Jn' Domm_Jn. set_solver. }
-            assert (In' = inflow_delete_KT In n k (Br !!! k)) 
-                                              as HIn' by done.
-            pose proof (inflow_delete_domm In n k (Br !!! k) In' HIn')
-                                          as Domm_In'.
-            assert (domm In' = domm In) as Domm_In'_eq_In.
-            { clear -Domm_In' Domm_In. set_solver. }
-            rewrite Domm_In'_eq_In Domm_Jn'_eq_Jn. iFrame "∗%".
-            iCombine "HrJ HnJ" as "HrnJ".
-            iCombine "HrI HnI" as "HrnI".
-            iPoseProof (own_valid with "[$HrnJ]") as "%".
-            rename H into Valid_rnJ. 
-            rewrite auth_frag_valid in Valid_rnJ *; intros Valid_rnJ.
-            assert (Jr ⋅ Jn = Jr' ⋅ Jn') as H'.
-            { apply (flowint_insert_eq_KT Jr Jr' _ _ n k T);
-                         try done.
-              clear -Domm_Jn. set_solver.
-              clear -Domm_Jr. set_solver. }
-            iPoseProof (own_valid with "[$HrnI]") as "%".
-            rename H into Valid_rnI. 
-            rewrite auth_frag_valid in Valid_rnI *; intros Valid_rnI.
-            assert (Ir ⋅ In = Ir' ⋅ In') as H''.
-            { apply (flowint_delete_eq_KT Ir Ir' _ _ n k (Br !!! k));
-                         try done.
-              clear -Domm_In. set_solver.
-              assert ((k, Br !!! k) ∈ outset_KT Ir n) as H''.
-              { apply OC_1. repeat split; try done. } 
-              unfold outset_KT, KT_flows.dom_ms in H''.
-              rewrite nzmap_elem_of_dom_total in H'' *; intros H''.
-              unfold ccmunit, ccm_unit in H''; simpl in H''; 
-              unfold nat_unit in H''.
-              pose proof Ole_I n (k, Br !!! k) as Ole_I.
-              clear -H'' Ole_I. 
-              assert (∀ (x: nat), x ≤ 1 → x ≠ 0 → 1 ≤ x) as H'.
-              lia. apply H'; try done. }
-            rewrite H' H''.
-            iEval (rewrite auth_frag_op) in "HrnJ".
-            iEval (rewrite auth_frag_op) in "HrnI".
-            iDestruct "HrnJ" as "(HrJ & HnJ)".
-            iDestruct "HrnI" as "(HrI & HnI)". iFrame. }
-          iAssert (outflow_constraints n In' Jn' Rn es_n Cn Bn)%I
-            with "[HnS_ocn]" as "HnS_ocn".
-          { iDestruct "HnS_ocn" as "(% & % & % & % & %)".
-            rename H into OCn_1. rename H2 into OCn_2.
-            rename H3 into OCn_3. rename H4 into Olen_I.
-            rename H5 into Olen_J. 
-            iPureIntro. split; last split; try done. }
-          iDestruct "Inf_R" as %Inf_R.
-          iPoseProof ((auth_own_incl γ_R R1 Rr) with "[HR HnS_si]")
-              as (Ro) "%". 
-          { unfold singleton_interfaces_ghost_state.
-            iDestruct "HnS_si" as "(_ & _ & H' & _)". 
-            iFrame. } rename H into Incl_R1.
-          iPoseProof (own_valid with "HR") as "%".
-          rename H into Valid_R1.
-          iAssert (⌜domm Rr = {[r]}⌝)%I as "%".
-          { by iDestruct "HnS_si" as "(_&_&_&_&_&H')". }
-          rename H into Domm_Rr.
-          iAssert (⌜φ0 Br' (T+1)⌝ ∗ ⌜φ1 Br' Cr' Ir'⌝ ∗ ⌜φ2 r Br' Ir'⌝ 
-               ∗ ⌜φ3 r Br' Jr'⌝ ∗ ⌜φ4 r Br' Rr⌝ ∗ ⌜φ5 r Rr⌝)%I with "[Hφ]" as "Hφ".
-          { iDestruct "Hφ" as %Hφ. 
-            destruct Hφ as [Hφ0 [Hφ1 [Hφ2 [Hφ3 [Hφ4 Hφ5]]]]].
-            iPureIntro. repeat split; try done.
-            - intros k'. destruct (decide (k' = k)).
-              rewrite HBr'. rewrite e. rewrite lookup_total_insert. lia.
-              rewrite HBr'. rewrite lookup_total_insert_ne; try done.
-              pose proof Hφ0 k' as H'. clear -H'.
-              apply (Nat.le_trans _ T _); try done. lia. 
-            - intros k'.
-              destruct (decide (k' = k)).
-              + right. replace Cr'. rewrite HBr'.
-                replace k'.
-                rewrite lookup_total_insert.
-                by rewrite lookup_total_insert.
-              + pose proof Hφ1 k' as Hφ1.
-                destruct Hφ1 as [Hφ1 | Hφ1].
-                destruct Hφ1 as [t' [n' Hφ1]].
-                destruct (decide (n' = n)).
-                * subst n'.
-                  assert (outset_KT Ir' n = (outset_KT Ir n) ∖ {[(k, Br !!! k)]}) 
-                                                                  as Out_eq.
-                  { pose proof outflow_delete_outset_KT Ir n k 
-                                                       (Br !!! k) Ir' as H'. 
-                    assert (Ir' = outflow_delete_KT Ir n k 
-                                                    (Br !!! k)) as HIr' by done.
-                    pose proof H' HIr' as [Hout _].
-                    pose proof Ole_I n (k, Br !!! k) as Ole_I.
-                    by apply Hout in Ole_I. }
-                  left. exists t', n.
-                  clear -n0 Out_eq Hφ1. set_solver.
-                * assert (outset_KT Ir' n' = outset_KT Ir n') as Out_eq.
-                  { assert (Ir' = outflow_delete_KT Ir n k (Br !!! k)) 
-                                                          as HIr' by done.
-                    by pose proof outflow_delete_outset_ne_KT Ir n k (Br !!! k)
-                                                   Ir' n' n1 HIr' as H'. }
-                  rewrite <-Out_eq in Hφ1.
-                  left. exists t', n'. done.
-                * right. rewrite HBr'.
-                  rewrite lookup_total_insert_ne; try done.
-                  replace Cr'.
-                  rewrite lookup_total_insert_ne; try done.
-            - intros k' t' Hins.
-              pose proof Infz_rI r as Infz_rI.
-              assert (Ir' = outflow_delete_KT Ir n k (Br !!! k)) as H' by done.
-              pose proof outflow_delete_inf_eq_KT Ir n k (Br !!! k) Ir' H' r as H''.
-              rewrite <-H'' in Infz_rI.
-              rewrite Infz_rI in Hins.
-              exfalso. clear -Hins. set_solver.
-            - intros k' t' Hins.
-              pose proof Infz_rJ r as Infz_rJ.
-              assert (inset_KT Jr' r = inset_KT Jr r) as H'.
-              { assert (inset_KT Jr' r = inset_KT Jr r) as H''.
-                apply (outflow_insert_inf_eq_KT _ n k T); try done.
-                done. }
-              rewrite H' in Hins. rewrite Infz_rJ in Hins.
-              exfalso. clear -Hins. set_solver.
-            - intros k'. right.
-              apply (inset_monotone R1 Rr Ro); try done.
-              by rewrite <-auth_auth_valid.
-              pose proof Inf_R r k' as Inf_R.
-              by rewrite <-beq_nat_refl in Inf_R.
-              rewrite Domm_Rr. clear. set_solver. } 
-          iAssert (⌜φ0 Bn (T+1)⌝ ∗ ⌜φ1 Bn Cn In'⌝ ∗ ⌜φ2 n Bn In'⌝ ∗ ⌜φ3 n Bn Jn'⌝ 
-                  ∗ ⌜φ4 n Bn Rn⌝ ∗ ⌜φ5 n Rn⌝)%I with "[Hφn]" as "Hφn".
-          { iDestruct "Hφn" as %Hφ. 
-            destruct Hφ as [Hφ0 [Hφ1 [Hφ2 [Hφ3 [Hφ4 Hφ5]]]]].
-            iPureIntro. repeat split; try done.
-            - intros k'. pose proof Hφ0 k' as H'.
-              apply (Nat.le_trans _ T _); try done. lia. 
-            - intros k' t'. 
-              assert (inset_KT In' n ⊆ inset_KT In n) as Inset.
-              { assert (In' = inflow_delete_KT In n k (Br !!! k)) 
-                                                    as HIn' by done.
-                pose proof inflow_delete_inset_KT In n k (Br !!! k)
-                                                      In' HIn' as Hin.
-                destruct (decide (inf In n !1 (k, Br !!! k) ≤ 1)) as [Hi1 | Hi1].
-                destruct Hin as [Hin _].
-                apply Hin in Hi1. 
-                clear -Hi1. set_solver.
-                destruct Hin as [_ Hin]. apply not_le in Hi1.
-                apply Hin in Hi1. clear -Hi1. 
-                rewrite -Hi1. set_solver. } 
-              intros Hin. 
-              assert ((k', t') ∈ inset_KT In n) as H'.
-              { clear -Hin Inset. set_solver. } 
-              by pose proof Hφ2 k' t' H' as Hφ2.
-            - intros k' t'. 
-              assert (inset_KT Jn' n = inset_KT Jn n ∪ {[k, T]}) as Inset.
-              { assert (Jn' = inflow_insert_KT Jn n k T) as HJn' by done.
-                by pose proof inflow_insert_inset_KT Jn n k T 
-                                                    Jn' HJn' as Hin. }
-              assert ((k',t') ∈ inset_KT Jn' n → 
-                         ((k',t') ∈ inset_KT Jn n) ∨ (k',t') = (k, T)) as Hkt'.
-              { intros Hin. rewrite Inset in Hin. set_solver. }
-              intros Hin. apply Hkt' in Hin.
-              destruct Hin as [Hin | Hin].
-              by pose proof Hφ3 k' t' Hin as Hφ3.
-              inversion Hin.
-              by pose proof Hφ0 k. }  
-          iMod "AU" as (t' H')"[MCS [_ Hclose]]".
-          iAssert (⌜t' = T⌝)%I as %Ht'. 
-          { iPoseProof ((auth_agree γ_te) with "[MCS_auth] [MCS]") as "%".
-            unfold MCS_auth. by iDestruct "MCS_auth" as "(H' & _)".
-            by iDestruct "MCS" as "(H' & _)".
-            by iPureIntro. } replace t'.
-          iAssert (⌜H' = H1⌝)%I as %H1'.
-          { iPoseProof ((auth_agree' γ_he) with "[MCS_auth] [MCS]") as "%".
-            unfold MCS_auth. by iDestruct "MCS_auth" as "(_ & H'')".
-            by iDestruct "MCS" as "(_ & H')".
-            by iPureIntro. } replace H'.
-          iDestruct "MCS" as "(MCS◯t & MCS◯h)".
-          iDestruct "MCS_auth" as "(MCS●t & MCS●h)".
-          iMod ((auth_update γ_te (T+1) T T) with "MCS●t MCS◯t") 
-                                              as "(MCS●t & MCS◯t)".
-          iMod ((auth_update' γ_he (H1 ∪ {[(k, T)]}) H1 H1) with "MCS●h MCS◯h") 
-                                              as "(MCS●h & MCS◯h)".
-          iCombine "MCS◯t MCS◯h" as "MCS".
-          iCombine "MCS●t MCS●h" as "MCS_auth".
-          iMod ("Hclose" with "MCS") as "HΦ".            
-          iModIntro.
-          iSplitR "HΦ node_r HnP_t HnP_C HnP_frac".
-          { iNext. iExists (T+1), (H1 ∪ {[(k, T)]}), I1, J1, R1.
-            iFrame "∗%".   
-            rewrite (big_sepS_delete _ (domm I1) r); last by eauto.
-            iSplitL "Hl_r Hlif_r HnS_cl HnS_star Hφ HnS_frac HnS_oc HnS_si".
-            { iExists true, Cr', Br'. iFrame.
-              unfold nodeShared. iExists es, Ir', Jr', Rr.
-              iFrame "∗#".
-              iEval (rewrite <-beq_nat_refl). iFrame "%∗". }        
-            rewrite (big_sepS_delete _ (domm I1 ∖ {[r]}) n); last by set_solver.
-            iSplitL "Hl_n Hlif_n HnS_cln HnS_starn Hφn HnS_fracn HnS_ocn 
-                        HnS_sin HnS_ifn".
-            { iExists bn, Cn, Bn. iFrame. iExists es_n, In', Jn', Rn.
-              iFrame "∗#". assert (n =? r = false) as Hnr. 
-              { by rewrite beq_nat_false_iff. } 
-              by rewrite Hnr. }
-            iApply (big_sepS_mono (λ y, ∃ (bn0 : bool) (Cn0 Bn0 : gmap K natUR),
-                                      lockLoc y ↦ #bn0
-                                    ∗ (if bn0 then True else
-                                       nodePred γ_e γ_c γ_b γ_t γ_s lc r y Cn0 Bn0)
-                                    ∗ nodeShared γ_I γ_J γ_R γ_e γ_c γ_b γ_f γ_cir
-                                              r y Cn0 Bn0 T H1 )%I
-                                   (λ y, ∃ (bn0 : bool) (Cn0 Bn0 : gmap K natUR),
-                                      lockLoc y ↦ #bn0
-                                    ∗ (if bn0 then True else
-                                       nodePred γ_e γ_c γ_b γ_t γ_s lc r y Cn0 Bn0)
-                                     ∗ nodeShared γ_I γ_J γ_R γ_e γ_c γ_b γ_f γ_cir
-                                              r y Cn0 Bn0 (T+1) (H1 ∪ {[(k, T)]}) )%I
-                                   (domm I1 ∖ {[r]} ∖ {[n]})); try done.
-            intros y y_dom. assert (y ≠ r) as Hy by set_solver. iFrame.
-            iIntros "Hstar". iDestruct "Hstar" as (b C B)"(Hl & Hlif & HnS)".
-            iExists b, C, B; iFrame. 
-            iDestruct "HnS" as (esy Iy Jy Ry)"(HnS_frac & HnS_si & HnS_FP 
-                        & HnS_cl & HnS_oc & HnS_if & HnS_star & Hφ0 & Hφ)".
-            iExists esy, Iy, Jy, Ry; iFrame. 
-            assert (y =? r = false) as Hyr by (rewrite beq_nat_false_iff; done).
-            iEval (rewrite Hyr).
-            iDestruct "Hφ0" as %Hφ0. iPureIntro; split; try done.
-            intros k'; pose proof Hφ0 k' as Hφ0.
-            apply (Nat.le_trans _ T _); try done. lia. } 
-            wp_pures.  
-            awp_apply (unlockNode_spec_high 
-                  with "[] [] [HnP_t HnP_C HnP_frac node_r]")
-                  without "HΦ"; try done. iExists es, (T + 1). iFrame.
-                  by iEval (rewrite <-beq_nat_refl).
-            iAaccIntro with ""; try eauto with iFrame.
-        + pose proof (out_edgeset_false k es Hes) as H'.
-          clear Hes. rename H' into Hes.
-          iMod ((frac_update γ_e γ_c γ_b r es Cr Br es Cr' Br') 
-               with "[$HnP_frac $HnS_frac]") as "(HnP_frac & HnS_frac)".
-          iAssert (⌜Br !!! k ≤ T⌝)%I as %Br_le_T. 
-          { iDestruct "Hφ" as "(% & _)".
-            iPureIntro. rename H into H'.
-            by pose proof H' k. }
-          iEval (rewrite (big_sepS_delete (_) (KS) k); last by eauto) in "HnS_star".
-          iDestruct "HnS_star" as "(Hk & HnS_star')".          
-          iMod (own_update (γ_cir r k) (● (MaxNat (Br !!! k))) 
-                    (● (MaxNat (Br' !!! k))) with "Hk") as "Hk".
-          { apply (auth_update_auth _ _ (MaxNat (Br' !!! k))).
-            apply max_nat_local_update.
-            simpl. rewrite HBr'.
-            by rewrite lookup_total_insert. }        
-          iAssert ([∗ set] k0 ∈ KS, own (γ_cir r k0) 
-                      (● {| max_nat_car := Br' !!! k0 |}))%I 
-              with "[HnS_star' Hk]" as "HnS_star".
-          { iEval (rewrite (big_sepS_delete (_) (KS) k); last by eauto).
-            iFrame "Hk".        
-            iApply (big_opS_proper 
-                 (λ y, own (γ_cir r y) (● {| max_nat_car := Br' !!! y |}))
-                 (λ y, own (γ_cir r y) (● {| max_nat_car := Br !!! y |})) 
-                 (KS ∖ {[k]})).
-            intros x Hx. assert (x ≠ k) as H' by set_solver.
-            iFrame. iSplit. 
-            iIntros "H". iEval (rewrite HBr') in "H".
-            assert (<[k:=T]> Br !!! x = Br !!! x) as H''. 
-            { apply lookup_total_insert_ne; try done. } 
-            by iEval (rewrite H'') in "H".       
-            iIntros "H". iEval (rewrite HBr').
-            assert (<[k:=T]> Br !!! x = Br !!! x) as H''. 
-            { apply lookup_total_insert_ne; try done. } 
-            by iEval (rewrite H'').
-            done. }
-          iAssert (outflow_constraints r Ir Jr Rr es Cr' Br')%I 
-                      with "[HnS_oc]" as "HnS_oc".
-          { iDestruct "HnS_oc" as "(% & % & %)".
-            rename H into OC_1. rename H2 into OC_2.
-            rename H3 into OC_3.
-            iPureIntro. split; last split; try done.
-            - intros n' k' t'. split.
-              + intros Hout.
-                pose proof OC_1 n' k' t' as [H' _].
-                apply H' in Hout.
-                destruct (decide (k' = k)).
-                * destruct Hout as [Hout _].
-                  rewrite e in Hout.
-                  pose proof Hes n' as Hes.
-                  clear - Hes Hout. set_solver.
-                * replace Cr'.
-                  rewrite lookup_total_insert_ne; try done.
-                  rewrite HBr'.
-                  rewrite lookup_total_insert_ne; try done.  
-              + intros Hout.
-                destruct (decide (k' = k)).
-                * destruct Hout as [Hout _].
-                  pose proof Hes n' as Hes.
-                  rewrite e in Hout.
-                  clear - Hes Hout. set_solver.
-                * replace Cr' in Hout.
-                  rewrite lookup_total_insert_ne in Hout; try done.
-                  rewrite HBr' in Hout.
-                  rewrite lookup_total_insert_ne in Hout; try done.
-                  by apply OC_1 in Hout.  
-            - intros n' k' t'. split.
-              + intros Hout.
-                pose proof OC_2 n' k' t' as [H' _].
-                apply H' in Hout.
-                destruct (decide (k' = k)).
-                * destruct Hout as [Hout _].
-                  rewrite e in Hout.
-                  pose proof Hes n' as Hes.
-                  clear - Hes Hout. set_solver.
-                * replace Cr'.
-                  rewrite lookup_total_insert_ne; try done.
-              + intros Hout.
-                destruct (decide (k' = k)).
-                * destruct Hout as [Hout _].
-                  pose proof Hes n' as Hes.
-                  rewrite e in Hout.
-                  clear - Hes Hout. set_solver.
-                * replace Cr' in Hout.
-                  rewrite lookup_total_insert_ne in Hout; try done.
-                  by apply OC_2 in Hout. }
-          iDestruct "Inf_R" as %Inf_R.
-          iPoseProof ((auth_own_incl γ_R R1 Rr) with "[HR HnS_si]")
-              as (Ro) "%". 
-          { unfold singleton_interfaces_ghost_state.
-            iDestruct "HnS_si" as "(_ & _ & H' & _)". 
-            iFrame. } rename H into Incl_R1.
-          iPoseProof (own_valid with "HR") as "%".
-          rename H into Valid_R1.
-          iAssert (⌜domm Rr = {[r]}⌝)%I as "%".
-          { by iDestruct "HnS_si" as "(_&_&_&_&_&H')". }
-          rename H into Domm_Rr.
-          iAssert (⌜φ0 Br' (T+1)⌝ ∗ ⌜φ1 Br' Cr' Ir⌝ ∗ ⌜φ2 r Br' Ir⌝ ∗ ⌜φ3 r Br' Jr⌝ 
-                  ∗ ⌜φ4 r Br' Rr⌝ ∗ ⌜φ5 r Rr⌝)%I with "[Hφ]" as "Hφ".
-          { iDestruct "Hφ" as %Hφ. 
-            destruct Hφ as [Hφ0 [Hφ1 [Hφ2 [Hφ3 [Hφ4 Hφ5]]]]].
-            iPureIntro. repeat split; try done.
-            - intros k'. destruct (decide (k' = k)).
-              rewrite HBr'. rewrite e. rewrite lookup_total_insert. lia.
-              rewrite HBr'. rewrite lookup_total_insert_ne; try done.
-              pose proof Hφ0 k' as H'. clear -H'.
-              apply (Nat.le_trans _ T _); try done. lia. 
-            - intros k'. pose proof Hφ1 k' as H'.
-              destruct H' as [H' | H'].
-              by left.
-              destruct (decide (k' = k)).
-              right. replace k'.
-              rewrite lookup_total_insert.
-              replace Cr'.
-              by rewrite lookup_total_insert.
-              right.
-              rewrite lookup_total_insert_ne; try done.
-              replace Cr'.
-              rewrite lookup_total_insert_ne; try done.
-            - intros k' t' Hins.
-              pose proof Infz_rI r as Infz_rI.
-              rewrite Infz_rI in Hins.
-              exfalso. clear -Hins. set_solver.
-            - intros k' t' Hins.
-              pose proof Infz_rJ r as Infz_rJ.
-              rewrite Infz_rJ in Hins.
-              exfalso. clear -Hins. set_solver.
-            - intros k'. right.
-              apply (inset_monotone R1 Rr Ro); try done.
-              by rewrite <-auth_auth_valid.
-              pose proof Inf_R r k' as Inf_R.
-              by rewrite <-beq_nat_refl in Inf_R.
-              rewrite Domm_Rr. clear. set_solver. } 
-          iMod "AU" as (t' H')"[MCS [_ Hclose]]".
-          iAssert (⌜t' = T⌝)%I as %Ht'. 
-          { iPoseProof ((auth_agree γ_te) with "[MCS_auth] [MCS]") as "%".
-            unfold MCS_auth. by iDestruct "MCS_auth" as "(H' & _)".
-            by iDestruct "MCS" as "(H' & _)".
-            by iPureIntro. } replace t'.
-          iAssert (⌜H' = H1⌝)%I as %H1'.
-          { iPoseProof ((auth_agree' γ_he) with "[MCS_auth] [MCS]") as "%".
-            unfold MCS_auth. by iDestruct "MCS_auth" as "(_ & H'')".
-            by iDestruct "MCS" as "(_ & H')".
-            by iPureIntro. } replace H'.
-          iDestruct "MCS" as "(MCS◯t & MCS◯h)".
-          iDestruct "MCS_auth" as "(MCS●t & MCS●h)".
-          iMod ((auth_update γ_te (T+1) T T) with "MCS●t MCS◯t") 
-                                              as "(MCS●t & MCS◯t)".
-          iMod ((auth_update' γ_he (H1 ∪ {[(k, T)]}) H1 H1) with "MCS●h MCS◯h") 
-                                              as "(MCS●h & MCS◯h)".
-          iCombine "MCS◯t MCS◯h" as "MCS".
-          iCombine "MCS●t MCS●h" as "MCS_auth".
-          iMod ("Hclose" with "MCS") as "HΦ".            
-                      
-            
-            
-          iModIntro.
-          iSplitR "HΦ node_r HnP_t HnP_C HnP_frac".
-          { iNext. iExists (T+1), (H1 ∪ {[(k, T)]}), I1, J1, R1.
-            iFrame "∗%".   
-            rewrite (big_sepS_delete _ (domm I1) r); last by eauto.
-            iSplitL "Hl_r Hlif_r HnS_cl HnS_star Hφ HnS_frac HnS_oc HnS_si".
-            { iExists true, Cr', Br'. iFrame.
-            unfold nodeShared. iExists es, Ir, Jr, Rr.
-            iFrame "∗#".
-            iEval (rewrite <-beq_nat_refl). iFrame "%∗". }        
-          iApply (big_sepS_mono (λ y, ∃ (bn0 : bool) (Cn0 Bn0 : gmap K natUR),
-                                    lockLoc y ↦ #bn0
-                                  ∗ (if bn0 then True else
-                                     nodePred γ_e γ_c γ_b γ_t γ_s lc r y Cn0 Bn0)
-                                  ∗ nodeShared γ_I γ_J γ_R γ_e γ_c γ_b γ_f γ_cir
-                                            r y Cn0 Bn0 T H1 )%I
-                                 (λ y, ∃ (bn0 : bool) (Cn0 Bn0 : gmap K natUR),
-                                    lockLoc y ↦ #bn0
-                                  ∗ (if bn0 then True else
-                                     nodePred γ_e γ_c γ_b γ_t γ_s lc r y Cn0 Bn0)
-                                  ∗ nodeShared γ_I γ_J γ_R γ_e γ_c γ_b γ_f γ_cir
-                                            r y Cn0 Bn0 (T+1) (H1 ∪ {[(k, T)]}) )%I
-                                 (domm I1 ∖ {[r]})); try done.
-            intros y y_dom. assert (y ≠ r) as Hy by set_solver. iFrame. 
-            iIntros "Hstar"; iDestruct "Hstar" as (b C B)"(Hl & Hlif & HnS)".
-            iExists b, C, B; iFrame. 
-            iDestruct "HnS" as (esy Iy Jy Ry)"(HnS_frac & HnS_si & HnS_FP 
-                          & HnS_cl & HnS_oc & HnS_if & HnS_star & Hφ0 & Hφ)";
-            iExists esy, Iy, Jy, Ry; iFrame. 
-            assert (y =? r = false) as Hyr by (rewrite beq_nat_false_iff; done);
-            iEval (rewrite Hyr).
-            iDestruct "Hφ0" as %Hφ0.
-            iPureIntro; split; try done.
-            intros k'. pose proof Hφ0 k' as Hφ0.
-            apply (Nat.le_trans _ T _); try done. lia. } 
-          wp_pures.  
-          awp_apply (unlockNode_spec_high with "[] [] [HnP_t HnP_C HnP_frac node_r]")
-                without "HΦ"; try done. iExists es, (T + 1). iFrame.
-                by iEval (rewrite <-beq_nat_refl).
-          iAaccIntro with ""; try eauto with iFrame.
+      destruct H0 as [Hes [Hc [Hb Hq]]]. 
+      subst es'. subst Cn'. subst Bn'. subst Qn'.
+      iSplitL "node_n HnP_gh HnP_frac HnP_C HnP_t".
+      iExists γ_en, γ_cn, γ_bn, γ_qn, γ_cirn, esn, T'.
+      iFrame.
+      iExists γ_en, γ_cn, γ_bn, γ_qn, γ_cirn, esn, In0, Rn0.
+      iFrame.
+    }
+    iFrame. iFrame. iFrame.
   Qed.
-
-End multicopy.             
-                    
-                       
-
-      
-      
-      
-
-                    
-       
-       
-    
-                                        
-        
-    
-    
-                                                  
-    
-  
-  
-  
-  
-  
   
 
+End multicopy.
