templates/multicopy/general_multicopy_search.v
@@ -1,0 +1,378 @@
+From iris.algebra Require Import excl auth cmra gmap agree gset numbers.
+From iris.algebra.lib Require Import frac_agree.
+From iris.heap_lang Require Export notation locations lang.
+From iris.base_logic.lib Require Export invariants.
+From iris.program_logic Require Export atomic.
+From iris.proofmode Require Import tactics.
+From iris.heap_lang Require Import proofmode par.
+From iris.bi.lib Require Import fractional.
+Set Default Proof Using "All".
+Require Import general_multicopy.
+
+Section search_proof.
+  Context {Σ} `{!heapG Σ, !multicopyG Σ}.
+  Notation iProp := (iProp Σ).  
+  Local Notation "m !1 i" := (nzmap_total_lookup i m) (at level 20).
+
+  Lemma traverse_spec N γ_te γ_he γ_s γ_t γ_I γ_R γ_f γ_gh lc r 
+                          γ_en γ_cn γ_bn γ_qn γ_cirn n (k: K) t0 t1 :
+    ⊢ ⌜k ∈ KS⌝ -∗ mcs_inv N γ_te γ_he γ_s γ_t γ_I γ_R γ_f γ_gh lc r -∗
+        inFP γ_f n -∗ 
+          own γ_gh (◯ {[n := ghost_loc γ_en γ_cn γ_bn γ_qn γ_cirn]}) -∗ 
+            own (γ_cirn !!! k) (◯ MaxNat t1) -∗ ⌜t0 ≤ t1⌝ -∗
+              <<< ∀ t H, MCS γ_te γ_he t H >>> 
+                  traverse #n #k @ ⊤ ∖ ↑N
+              <<< ∃ (t': nat), MCS γ_te γ_he t H ∗ ⌜(k, t') ∈ H⌝ 
+                                             ∗ ⌜t0 ≤ t'⌝ , RET #t' >>>.
+  Proof.
+    iIntros "k_in_KS #HInv". 
+    iLöb as "IH" forall (n t1 γ_en γ_cn γ_bn γ_qn γ_cirn).
+    iIntros "#FP_n #Hgh #Hlb H". iDestruct "H" as %t0_le_t1.
+    iDestruct "k_in_KS" as %k_in_KS.
+    iIntros (Φ) "AU". wp_lam. wp_pures.
+    (** Lock node n **)
+    awp_apply lockNode_spec_high; try done.
+    iAaccIntro with ""; try eauto with iFrame. 
+    iIntros (Cn Bn Qn)"HnP_n". iModIntro. wp_pures. 
+    iDestruct "HnP_n" as (γ_en' γ_bn' γ_cn' γ_qn' γ_cirn' es T)
+                    "(node_n & HnP_gh & HnP_frac & HnP_C & HnP_t)".
+    iPoseProof (ghost_heap_sync with "[$HnP_gh] [$Hgh]") 
+                                  as "(% & % & % & % & %)".
+    subst γ_en'. subst γ_cn'. subst γ_bn'. subst γ_qn'. subst γ_cirn'.
+    (** Check contents of n **)
+    wp_apply (inContents_spec with "node_n").
+    iIntros (t) "(node_n & H)". iDestruct "H" as %Cn_val.
+    wp_pures.
+    (** Case analysis on whether k in contents of n **)
+    destruct t as [t |]; last first.
+    - (** Case : k not in contents of n **)
+      wp_pures.
+      (** Find next node to visit **)
+      wp_apply (findNext_spec with "node_n").
+      iIntros (b n1) "(node_n & Hif)". 
+      (** Case analysis on whether there exists a next node **)
+      destruct b.
+      + (** Case : exists next node n' **)
+        wp_pures. iDestruct "Hif" as %k_in_es.
+        iApply fupd_wp.
+        (** Open invariant to establish resources
+            required to apply induction hypothesis IH
+            on node n' **)
+        iInv "HInv" as ">H".
+        iDestruct "H" as (T' H hγ I R) "(Hglob & Hstar)".
+        iAssert (⌜n ∈ domm I⌝)%I as "%". 
+        { iDestruct "Hglob" as "(MCS_auth & HH & Hist & Ht & HI & Out_I & HR 
+            & Out_R & Inf_R & Hf & Hγ & FP_r & Max_ts & domm_IR & domm_Iγ)".
+          by iPoseProof (inFP_domm _ _ _ with "[$FP_n] [$Hf]") as "H'". }
+        rewrite (big_sepS_delete _ (domm I) n); last by eauto.
+        iDestruct "Hstar" as "(H_n & Hstar')".
+        iDestruct "H_n" as (bn Cn' Bn' Qn')"(Hl_n & Hlif_n & HnS_n)".
+        iDestruct "HnS_n" as (γ_en' γ_cn' γ_bn' γ_qn' γ_cirn' es' In Rn) 
+                      "(HnS_gh & HnS_frac & HnS_si & HnS_FP 
+                                & HnS_cl & HnS_oc & HnS_H & HnS_star & Hφ)".
+        iPoseProof (ghost_heap_sync with "[$HnP_gh] [$HnS_gh]") 
+                                  as "(% & % & % & % & %)".
+        subst γ_en'. subst γ_cn'. subst γ_bn'. subst γ_qn'. subst γ_cirn'.
+        iPoseProof (frac_eq with "[$HnP_frac] [$HnS_frac]") as "%".
+        destruct H1 as [Hes [Hc [Hb Hq]]]. 
+        subst es'. subst Cn'. subst Bn'. subst Qn'.
+        iAssert (inFP γ_f n1)%I as "#FP_n1".
+        { iApply "HnS_cl". iPureIntro. 
+          clear -k_in_es. set_solver. }
+             
+        iAssert (⌜n1 ∈ domm I⌝)%I as %n_in_I.
+        { iDestruct "Hglob" as "(MCS_auth & HH & Hist & Ht & HI & Out_I & HR 
+            & Out_R & Inf_R & Hf & Hγ & FP_r & Max_ts & domm_IR & domm_Iγ)".
+          by iPoseProof (inFP_domm _ _ _ with "[$FP_n1] [$Hf]") as "H'". }
+        iAssert (⌜n ≠ n1⌝)%I as %n_neq_n1.
+        { destruct (decide (n = n1)); try done.
+          iPoseProof (node_edgeset_empty_root_self with "node_n") as "%".
+          destruct H1 as [_ Es_n]. rewrite <-e in k_in_es.
+          clear -k_in_es Es_n. set_solver. } 
+        rewrite (big_sepS_delete _ (domm I ∖ {[n]}) n1); last by set_solver.
+        iDestruct "Hstar'" as "(H_n1 & Hstar'')".
+        iDestruct "H_n1" as (bn1 Cn1 Bn1 Qn1)"(Hl_n1 & Hlif_n1 & HnS_n1)".
+        iDestruct "HnS_n1" as (γ_en1 γ_cn1 γ_bn1 γ_qn1 γ_cirn1 es1 In1 Rn1) 
+                  "(HnS_gh1 & HnS_frac1 & HnS_si1 & HnS_FP1 
+                       & HnS_cl1 & HnS_oc1 & HnS_H1 & HnS_star1 & Hφ1)".
+
+        iEval (rewrite (big_sepS_elem_of_acc (_) (KS) k); 
+                              last by eauto) in "HnS_star".
+        iDestruct "HnS_star" as "(Hcirk_n & HnS_star')".
+        iEval (rewrite (big_sepS_elem_of_acc (_) (KS) k);
+                                     last by eauto) in "HnS_star1".
+        iDestruct "HnS_star1" as "(Hcirk_n1 & HnS_star1')".
+        iMod (own_update (γ_cirn1 !!! k) (● MaxNat (Bn1 !!! k)) 
+              ((● MaxNat (Bn1 !!! k)) ⋅ (◯ MaxNat (Bn1 !!! k))) 
+                  with "[Hcirk_n1]") as "(Hcirk_n1 & #Hlb_1)".
+        { apply (auth_update_alloc _ (MaxNat (Bn1 !!! k)) 
+                              (MaxNat (Bn1 !!! k))).
+          apply max_nat_local_update. 
+          simpl. lia. } { iFrame. }
+
+        iAssert (⌜t0 ≤ Bn1 !!! k⌝)%I as "%".
+        { iAssert (⌜t1 ≤ Bn !!! k⌝)%I as %lb_t1.
+          { iPoseProof (own_valid_2 with "[$Hcirk_n] [$Hlb]") as "%".
+            rename H1 into Valid_Bnt.
+            apply auth_both_valid_discrete in Valid_Bnt.
+            destruct Valid_Bnt as [H' _].
+            apply max_nat_included in H'.
+            simpl in H'. by iPureIntro. }
+          destruct (Qn !! k) as [tq | ] eqn: Hqn.
+          - iAssert (⌜(k, Qn !!! k) ∈ outset KT In n1⌝)%I as %outflow_n_n1.
+            { iDestruct "HnS_oc" as "(H' & _)".
+              iDestruct "H'" as %H'. iPureIntro.    
+              apply (H' n1 k (Qn !!! k)).
+              unfold outflow_constraint_I in H'.
+              done. repeat split; try done. 
+              rewrite lookup_total_alt. 
+              rewrite Hqn. by simpl. }
+            iAssert (⌜(k, Qn !!! k) ∈ inset KT In1 n1⌝)%I as %inflow_n1.
+            { iDestruct "HnS_si" as "(H'&_)".
+              iDestruct "HnS_si1" as "(H1'&_&%&_)".
+              rename H1 into Domm_In1.
+              assert (n1 ∈ domm In1) as H''. 
+              { clear -Domm_In1. set_solver. }
+              iCombine "H'" "H1'" as "H'".
+              iPoseProof (own_valid with "[$H']") as "%".
+              rename H1 into Valid_InIn1.
+              rewrite auth_frag_valid in Valid_InIn1 *; intros Valid_InIn1.
+              pose proof intComp_unfold_inf_2 In In1 Valid_InIn1 n1 H''.
+              rename H1 into H'. unfold ccmop, ccm_op in H'.
+              simpl in H'. unfold lift_op in H'.
+              iPureIntro. rewrite nzmap_eq in H' *; intros H'.
+              pose proof H' (k, Qn !!! k) as H'.
+              rewrite nzmap_lookup_merge in H'.
+              unfold ccmop, ccm_op in H'. simpl in H'.
+              unfold nat_op in H'.
+              assert (1 ≤ out In n1 !1 (k, Qn !!! k)) as Hout.
+              { unfold outset, dom_ms in outflow_n_n1.
+                rewrite nzmap_elem_of_dom_total in outflow_n_n1 *; 
+                intros outflow_n_n1.
+                unfold ccmunit, ccm_unit in outflow_n_n1.
+                simpl in outflow_n_n1. unfold nat_unit in outflow_n_n1.
+                clear - outflow_n_n1. lia. }
+              assert (1 ≤ inf In1 n1 !1 (k, Qn !!! k)) as Hin.
+              { clear -H' Hout. 
+                assert (∀ (x y z: nat), 1 ≤ y → x = z + y → 1 ≤ x) as H''.
+                lia. by pose proof H'' _ _ _ Hout H'. }
+              unfold inset. rewrite nzmap_elem_of_dom_total.
+              unfold ccmunit, ccm_unit. simpl. unfold nat_unit.
+              clear -Hin. lia. }
+            iAssert (⌜Bn1 !!! k = Qn !!! k⌝)%I as %Bn1_eq_Bn.
+            { iDestruct "Hφ1" as "(_ & _& % & _)". 
+              rename H1 into Hφ2. 
+              pose proof Hφ2 k (Qn !!! k) k_in_KS inflow_n1 as H'.
+              iPureIntro. done. } 
+            iAssert (⌜Bn !!! k = Qn !!! k⌝)%I as %Bn_eq_Qn.
+            { iDestruct "Hφ" as "(_ & % & _)". rename H1 into Hφ1.
+              pose proof Hφ1 k as [_ H']. done.
+              iPureIntro. pose proof H' Cn_val as H'. 
+              rewrite /(Bn !!! k). unfold finmap_lookup_total.
+              by rewrite H'.  } 
+            iPureIntro. rewrite Bn1_eq_Bn.
+            rewrite <-Bn_eq_Qn. clear -lb_t1 t0_le_t1.
+            apply (Nat.le_trans _ t1 _); try done.
+          - iDestruct "Hφ" as "(_ & % & _)".
+            rename H1 into Hφ1. apply Hφ1 in Cn_val.
+            rewrite <-Cn_val in Hqn.
+            rewrite lookup_total_alt in lb_t1.
+            rewrite Hqn in lb_t1.
+            simpl in lb_t1. iPureIntro.
+            clear -lb_t1 t0_le_t1. lia.
+            try done. done. }
+ 
+        iAssert (own γ_gh (◯ {[n1 := 
+                      ghost_loc γ_en1 γ_cn1 γ_bn1 γ_qn1 γ_cirn1]}))%I
+                            with "HnS_gh1" as "#Hgh1".  
+        (** Closing the invariant **)
+        iModIntro. iSplitR "node_n HnP_gh HnP_frac HnP_C HnP_t AU". iNext.
+        iExists T', H, hγ, I, R. iFrame "Hglob".
+        rewrite (big_sepS_delete _ (domm I) n); last by eauto.
+        rewrite (big_sepS_delete _ (domm I ∖ {[n]}) n1); last set_solver.
+        iFrame "Hstar''". iSplitL "Hl_n Hlif_n HnS_gh HnS_frac 
+                    HnS_si HnS_FP HnS_cl HnS_oc HnS_H Hcirk_n HnS_star' Hφ".
+        iExists bn, Cn, Bn, Qn. iFrame "Hl_n Hlif_n".
+        iExists γ_en, γ_cn, γ_bn, γ_qn, γ_cirn, es, In, Rn.
+        iFrame. by iApply "HnS_star'".                  
+        iExists bn1, Cn1, Bn1, Qn1. iFrame "Hl_n1 Hlif_n1".
+        iExists γ_en1, γ_cn1, γ_bn1, γ_qn1, γ_cirn1, es1, In1, Rn1.
+        iFrame. by iApply "HnS_star1'".
+        iModIntro.
+        (** Unlock node n **)       
+        awp_apply (unlockNode_spec_high with "[] [] 
+            [HnP_gh HnP_frac HnP_C HnP_t node_n]"); try done.
+        iExists γ_en, γ_cn, γ_bn, γ_qn, γ_cirn, es, T.
+        iFrame.                
+        iAaccIntro with ""; try eauto with iFrame.
+        iIntros "_". iModIntro. wp_pures.
+        (** Apply IH on node n' **)
+        iApply "IH"; try done. 
+      + (** Case : no next node from n **)
+        wp_pures. iDestruct "Hif" as %Not_in_es.
+        iApply fupd_wp. 
+        (** Linearization Point: key k has not been found in the 
+            data structure. Open invariant to obtain resources 
+            required to establish post-condition **)
+        iInv "HInv" as ">H".
+        iDestruct "H" as (T' H hγ I R) "(Hglob & Hstar)".
+        iAssert (⌜n ∈ domm I⌝)%I as "%". 
+        { iDestruct "Hglob" as "(MCS_auth & HH & Hist & Ht & HI & Out_I & HR 
+            & Out_R & Inf_R & Hf & Hγ & FP_r & Max_ts & domm_IR & domm_Iγ)".
+          by iPoseProof (inFP_domm _ _ _ with "[$FP_n] [$Hf]") as "H'". }
+        rewrite (big_sepS_delete _ (domm I) n); last by eauto.
+        iDestruct "Hstar" as "(H_n & Hstar')".
+        iDestruct "H_n" as (bn Cn' Bn' Qn')"(Hl_n & Hlif_n & HnS_n)".
+        iDestruct "HnS_n" as (γ_en' γ_cn' γ_bn' γ_qn' γ_cirn' es' In Rn) 
+                      "(HnS_gh & HnS_frac & HnS_si & HnS_FP 
+                                & HnS_cl & HnS_oc & HnS_H & HnS_star & Hφ)".
+        iPoseProof (ghost_heap_sync with "[$HnP_gh] [$HnS_gh]") 
+                                  as "(% & % & % & % & %)".
+        subst γ_en'. subst γ_cn'. subst γ_bn'. subst γ_qn'. subst γ_cirn'.
+        iPoseProof (frac_eq with "[$HnP_frac] [$HnS_frac]") as "%".
+        destruct H1 as [Hes [Hc [Hb Hq]]]. 
+        subst es'. subst Cn'. subst Bn'. subst Qn'.
+        iAssert (⌜Bn !!! k = 0⌝)%I as %Bn_eq_0.
+        { iDestruct "Hφ" as "(Hφ0 & Hφ1 & _)".
+          iDestruct "Hφ0" as %Hφ0.
+          iDestruct "Hφ1" as %Hφ1.
+          pose proof Hφ0 k k_in_KS Not_in_es as Hφ0.
+          pose proof Hφ1 k as [_ H']. done.
+          pose proof H' Cn_val as H'. 
+          iPureIntro.
+          rewrite lookup_total_alt.
+          rewrite H' Hφ0. by simpl. }          
+        iEval (rewrite (big_sepS_elem_of_acc (_) (KS) k); last by eauto) 
+                                                       in "HnS_star".
+        iDestruct "HnS_star" as "(Hcirk_n & HnS_star')".
+        iAssert (⌜t1 ≤ Bn !!! k⌝)%I as %lb_t1.
+        { iPoseProof (own_valid_2 with "[$Hcirk_n] [$Hlb]") as "%".
+          rename H1 into Valid_Bnt.
+          apply auth_both_valid_discrete in Valid_Bnt.
+          destruct Valid_Bnt as [H' _].
+          apply max_nat_included in H'.
+          simpl in H'. by iPureIntro. }
+        iAssert (⌜t0 = 0⌝)%I as %t0_zero. 
+        { iPureIntro. rewrite Bn_eq_0 in lb_t1. 
+          clear -lb_t1 t0_le_t1. lia. } subst t0.
+        (** Linearization **)  
+        iMod "AU" as (t' H') "[MCS [_ Hclose]]". 
+        iAssert (⌜H' = H⌝)%I as %H1. 
+        { iDestruct "Hglob" as "(MCS_auth & HH & Hist & Ht & HI & Out_I & HR 
+            & Out_R & Inf_R & Hf & Hγ & FP_r & Max_ts & domm_IR & domm_Iγ)".
+          iPoseProof ((auth_agree' γ_he) with "[MCS_auth] [MCS]") as "%".
+          unfold MCS_auth. by iDestruct "MCS_auth" as "(_ & H'')".
+          by iDestruct "MCS" as "(_ & H')".
+          by iPureIntro. } subst H'.
+        iAssert (⌜(k,0) ∈ H⌝)%I as "%". 
+        { iDestruct "Hglob" as "(MCS_auth & HH & Hist & Ht & HI & Out_I & HR 
+            & Out_R & Inf_R & Hf & Hγ & FP_r & Max_ts & domm_IR & domm_Iγ)".
+          iDestruct "Hist" as %Hist. iPureIntro. 
+          by pose proof Hist k k_in_KS as Hist. }
+        rename H1 into k0_in_H.  
+        iSpecialize ("Hclose" $! 0).
+        iMod ("Hclose" with "[MCS]") as "HΦ". iFrame. 
+        iPureIntro. split; try done.
+        (** Closing the invariant **)
+        iModIntro. iSplitR "node_n HnP_gh HnP_frac HnP_C HnP_t HΦ". iNext.
+        iExists T', H, hγ, I, R. iFrame "Hglob".
+        rewrite (big_sepS_delete _ (domm I) n); last by eauto.
+        iFrame "Hstar'". iExists bn, Cn, Bn, Qn.
+        iFrame "Hl_n Hlif_n". 
+        iExists γ_en, γ_cn, γ_bn, γ_qn, γ_cirn, es, In, Rn.
+        iFrame "∗%". by iApply "HnS_star'". iModIntro.
+        (** Unlock node n **)
+        awp_apply (unlockNode_spec_high with "[] [] 
+               [HnP_gh HnP_frac HnP_C HnP_t node_n]") without "HΦ"; try done. 
+        iExists γ_en, γ_cn, γ_bn, γ_qn, γ_cirn, es, T. iFrame.
+        iAaccIntro with ""; try eauto with iFrame.
+        iIntros "_". iModIntro. iIntros "HΦ". by wp_pures.
+    - (** Case : k in contents of n **)
+      wp_pures.                                         
+      iApply fupd_wp. 
+      (** Linearization Point: key k has been found. Open 
+          invariant to obtain resources required to 
+          establish post-condition **)
+      iInv "HInv" as ">H".
+      iDestruct "H" as (T' H hγ I R) "(Hglob & Hstar)".
+      iAssert (⌜n ∈ domm I⌝)%I as "%". 
+      { iDestruct "Hglob" as "(MCS_auth & HH & Hist & Ht & HI & Out_I & HR 
+            & Out_R & Inf_R & Hf & Hγ & FP_r & Max_ts & domm_IR & domm_Iγ)".
+        by iPoseProof (inFP_domm _ _ _ with "[$FP_n] [$Hf]") as "H'". }
+      rewrite (big_sepS_delete _ (domm I) n); last by eauto.
+      iDestruct "Hstar" as "(H_n & Hstar')".
+      iDestruct "H_n" as (bn Cn' Bn' Qn')"(Hl_n & Hlif_n & HnS_n)".
+      iDestruct "HnS_n" as (γ_en' γ_cn' γ_bn' γ_qn' γ_cirn' es' In Rn) 
+                    "(HnS_gh & HnS_frac & HnS_si & HnS_FP 
+                              & HnS_cl & HnS_oc & HnS_H & HnS_star & Hφ)".
+      iPoseProof (ghost_heap_sync with "[$HnP_gh] [$HnS_gh]") 
+                                as "(% & % & % & % & %)".
+      subst γ_en'. subst γ_cn'. subst γ_bn'. subst γ_qn'. subst γ_cirn'.
+      iPoseProof (frac_eq with "[$HnP_frac] [$HnS_frac]") as "%".
+      destruct H1 as [Hes [Hc [Hb Hq]]]. 
+      subst es'. subst Cn'. subst Bn'. subst Qn'.
+      iEval (rewrite (big_sepS_elem_of_acc (_) (KS) k); last by eauto) 
+                                                      in "HnS_star".
+      iDestruct "HnS_star" as "(Hcirk_n & HnS_star')".
+      iAssert (⌜t1 ≤ Bn !!! k⌝)%I as %lb_t1.
+      { iPoseProof (own_valid_2 with "[$Hcirk_n] [$Hlb]") as "%".
+        rename H1 into Valid_Bnt.
+        apply auth_both_valid_discrete in Valid_Bnt.
+        destruct Valid_Bnt as [H' _].
+        apply max_nat_included in H'.
+        simpl in H'. by iPureIntro. }
+      iAssert (⌜Bn !!! k = Cn !!! k⌝)%I as %Bn_eq_Cn.
+      { iDestruct "Hφ" as "(_ & Hφ1 & _)".
+        iDestruct "Hφ1" as %Hφ1.
+        pose proof Hφ1 k t as [H' _].
+        done. iPureIntro.
+        rewrite !lookup_total_alt.
+        pose proof H' Cn_val as H'.
+        by rewrite Cn_val H'. }          
+      iAssert (⌜set_of_map Cn ⊆ H⌝)%I as %Cn_Sub_H.
+      { iDestruct "Hglob" as "(MCS_auth & HH & Hist & Ht & HI & Out_I & HR 
+            & Out_R & Inf_R & Hf & Hγ & FP_r & Max_ts & domm_IR & domm_Iγ)".
+        iPoseProof ((auth_own_incl γ_s H _) with "[$HH $HnP_C]") as "%".
+        rename H1 into H'. by apply gset_included in H'. }  
+      iAssert (⌜(k,t) ∈ set_of_map Cn⌝)%I as %kt_in_Cn.
+      { iPureIntro. apply set_of_map_member.
+        rewrite /(Cn !!! k) in Cn_val.
+        unfold finmap_lookup_total, inhabitant in Cn_val.
+        simpl in Cn_val. 
+        destruct (Cn !! k) as [cnk | ] eqn: Hcnk.
+        - rewrite Hcnk. apply f_equal.
+          by inversion Cn_val. 
+        - try done.  }
+      (** Linearization **)      
+      iMod "AU" as (t' H') "[MCS [_ Hclose]]". 
+      iSpecialize ("Hclose" $! t).
+      iAssert (⌜H' = H⌝)%I as %H1. 
+      { iDestruct "Hglob" as "(MCS_auth & HH & Hist & Ht & HI & Out_I & HR 
+            & Out_R & Inf_R & Hf & Hγ & FP_r & Max_ts & domm_IR & domm_Iγ)".
+        iPoseProof ((auth_agree' γ_he) with "[MCS_auth] [MCS]") as "%".
+        unfold MCS_auth. by iDestruct "MCS_auth" as "(_ & H'')".
+        by iDestruct "MCS" as "(_ & H')".
+        by iPureIntro. } replace H'.
+      iMod ("Hclose" with "[MCS]") as "HΦ". iFrame. 
+      iPureIntro. split. set_solver. rewrite Bn_eq_Cn in lb_t1.
+      rewrite lookup_total_alt in lb_t1.
+      rewrite Cn_val in lb_t1. simpl in lb_t1. lia.
+      (** Closing the invariant **)
+      iModIntro. iSplitR "node_n HnP_gh HnP_frac HnP_C HnP_t HΦ".
+      iNext. iExists T', H, hγ, I, R. iFrame "Hglob".
+      rewrite (big_sepS_delete _ (domm I) n); last by eauto.
+      iFrame "Hstar'". iExists bn, Cn, Bn, Qn.
+      iFrame "Hl_n Hlif_n". 
+      iExists γ_en, γ_cn, γ_bn, γ_qn, γ_cirn, es, In, Rn.
+      iFrame "∗%". by iApply "HnS_star'". iModIntro.
+      (** Unlock node n **)
+      awp_apply (unlockNode_spec_high with "[] [] 
+                [HnP_gh HnP_frac HnP_C HnP_t node_n]") without "HΦ"; 
+                      try done.
+      iExists γ_en, γ_cn, γ_bn, γ_qn, γ_cirn, es, T. iFrame.
+      iAaccIntro with ""; try eauto with iFrame.
+      iIntros "_". iModIntro. iIntros "HΦ". by wp_pures.
+      Unshelve. try done. try done.
+  Qed.
+
+End search_proof.
