templates/multicopy/general_multicopy_upsert.v
@@ -1,0 +1,319 @@
+From iris.algebra Require Import excl auth cmra gmap agree gset numbers.
+From iris.algebra.lib Require Import frac_agree.
+From iris.heap_lang Require Export notation locations lang.
+From iris.base_logic.lib Require Export invariants.
+From iris.program_logic Require Export atomic.
+From iris.proofmode Require Import tactics.
+From iris.heap_lang Require Import proofmode par.
+From iris.bi.lib Require Import fractional.
+Set Default Proof Using "All".
+Require Import general_multicopy.
+
+Section upsert_proof.
+  Context {Σ} `{!heapG Σ, !multicopyG Σ}.
+  Notation iProp := (iProp Σ).  
+  Local Notation "m !1 i" := (nzmap_total_lookup i m) (at level 20).
+
+  Lemma upsert_spec N γ_te γ_he γ_s γ_t γ_I γ_R γ_f γ_gh lc r (k: K) :
+    ⊢ ⌜k ∈ KS⌝ -∗ 
+          mcs_inv N γ_te γ_he γ_s γ_t γ_I γ_R γ_f γ_gh lc r -∗
+                <<< ∀ t H, MCS γ_te γ_he t H >>> 
+                    upsert lc r #k @ ⊤ ∖ ↑N
+                <<< MCS γ_te γ_he (t + 1) (H ∪ {[(k, t)]}), RET #() >>>.
+  Proof.
+    iIntros "H". iDestruct "H" as %k_in_KS.
+    iIntros "#HInv". iLöb as "IH".
+    iIntros (Φ) "AU". wp_lam.
+    iApply fupd_wp. 
+    (** Open invariant to establish root node in footprint **)
+    iInv "HInv" as ">H".
+    iDestruct "H" as (T0 H0 hγ0 I0 R0) "(Hglob & Hstar)".
+    iDestruct "Hglob" as "(MCS_auth & HH & Hist & Ht & HI & Out_I & HR 
+            & Out_R & Inf_R & Hf & Hγ & #FP_r & Max_ts & domm_IR & domm_Iγ)".
+    iModIntro. iSplitR "AU". iNext. 
+    iExists T0, H0, hγ0, I0, R0. iFrame "∗ #". iModIntro.
+    (** Lock the node r **)
+    awp_apply lockNode_spec_high; try done.
+    iAaccIntro with ""; try eauto with iFrame. 
+    iIntros (Cr Br Qr)"HnP_n". iModIntro. wp_pures.
+    iDestruct "HnP_n" as (γ_er γ_cr γ_br γ_qr γ_cirr es T)
+                      "(node_r & HnP_gh & HnP_frac & HnP_C & HnP_t)".
+    iEval (rewrite decide_True) in "HnP_t".
+    wp_apply (readClock_spec with "[HnP_t]"); try done.
+    iIntros "HnP_t". wp_pures.
+    wp_apply (addContents_spec with "node_r").
+    iIntros (b Cr')"(node_r & Hif)".
+    (** Case analysis on whether addContents is successful **)
+    destruct b; last first.
+    - (** Case : addContents fails. Unlock root node and apply 
+                 inductive hypothesis IH **) 
+      iDestruct "Hif" as %HCr. replace Cr'. wp_pures.
+      awp_apply (unlockNode_spec_high with "[] [] [-AU]"); try done.
+      { iExists γ_er, γ_cr, γ_br, γ_qr, γ_cirr, es, T.
+        iFrame. iEval (rewrite decide_True); try done. }
+      iAaccIntro with ""; try eauto with iFrame.
+      iIntros "_". iModIntro. wp_pures.
+      by iApply "IH".
+    - (** Case : addContent successful **)
+      (** Linearization Point: open invariant and update the resources **)
+      awp_apply (incrementClock_spec γ_t lc T). iInv "HInv" as ">H". 
+      iDestruct "H" as (T1 H1 hγ1 I1 R1) "(Hglob & Hstar)".
+      iDestruct "Hglob" as "(MCS_auth & HH & Hist & Ht & HI & Out_I & HR 
+            & Out_R & Inf_R & Hf & Hγ & _ & Max_ts & domm_IR & domm_Iγ)".
+      iDestruct "Hif" as %HCr. wp_pures.
+      iAssert (⌜T = T1⌝)%I as %HT. 
+      { iDestruct "HnP_t" as "(HnP_t & Hc)".
+        iPoseProof ((own_valid_2 _ _ _) with "[$HnP_t] [$Ht]") as "H'".
+        iDestruct "H'" as %H'. 
+        pose proof (auth_auth_frac_op_inv _ _ _ _ H') as H''.
+        inversion H''. by iPureIntro. } replace T1.
+      (** Updating the clock value **)            
+      iAssert (own γ_t (● (MaxNat T)) ∗ clock lc T)%I 
+                                        with "[Ht HnP_t]" as "H".
+      { iDestruct "HnP_t" as "(Ht' & Hc)".
+        iCombine "Ht Ht'" as "H'". iFrame. }
+      iAaccIntro with "H".
+      { iIntros "H". iDestruct "H" as "(Ht & Hc)".
+        iDestruct "Ht" as "(Ht & HnP_t)".
+        iCombine "HnP_t Hc" as "HnP_t". 
+        iModIntro. iSplitR "AU HnP_gh HnP_frac HnP_C node_r HnP_t".
+        iNext. iExists T, H1, hγ1, I1, R1. iFrame "∗ #". iFrame.
+        by iPureIntro. }
+      iIntros "(Ht & Hc)".  
+      iDestruct "Ht" as "(Ht & HnP_t)".
+      iCombine "HnP_t Hc" as "HnP_t".
+      iPoseProof ((auth_own_incl γ_s H1 _) with "[$HH $HnP_C]") as "%".
+      rename H into Cr_sub_H1. apply gset_included in Cr_sub_H1.
+      iDestruct "Max_ts" as %Max_tsH1.
+      (** Re-establish maxTS for updated T and H **)
+      assert (maxTS (T+1) (H1 ∪ {[(k, T)]})) as Max_ts.
+      { split. intros k' t' H.
+        assert (((k',t') ∈ H1) ∨ (k' = k ∧ t' = T)) as Hor by set_solver.
+        destruct Hor as [Hor | Hor]. 
+        destruct Max_tsH1 as [Max_tsH1 _].
+        pose proof Max_tsH1 k' t' Hor as Hres. lia.
+        destruct Hor as [_ Hor]. replace t'. lia.
+        destruct Max_tsH1 as [_ Max_tsH1]. lia. }       
+      iAssert (⌜set_of_map Cr' ⊆ H1 ∪ {[(k,T)]}⌝)%I as %Cr_sub_H1'.
+      { iPureIntro. replace Cr'.
+        pose proof (set_of_map_insert_subseteq Cr k T) as H'.
+        assert (set_of_map Cr = set_of_map Cr) as H'' by done. 
+        set_solver. }
+      (** Update the (● H) resource **)  
+      iMod (own_update γ_s (● H1) (● (H1 ∪ {[(k,T)]})) with "[$HH]") as "HH".
+      { apply (auth_update_auth _ _ (H1 ∪ {[(k,T)]})).
+        apply gset_local_update. set_solver. }
+      iMod (own_update γ_s (● (H1 ∪ {[(k, T)]})) 
+             (● (H1 ∪ {[(k, T)]}) ⋅ ◯ (set_of_map Cr')) with "[$HH]") as "HH".
+      { apply (auth_update_alloc _ (H1 ∪ {[(k,T)]}) (set_of_map Cr')).
+        apply local_update_discrete. intros m Valid_H1 H1_eq.
+        split; try done. rewrite /(ε ⋅? m) in H1_eq.
+        destruct m. rewrite gset_op_union in H1_eq. 
+        rewrite left_id in H1_eq *; intros H1_eq.
+        rewrite <-H1_eq. 
+        rewrite /(set_of_map Cr' ⋅? Some (H1 ∪ {[k, T]})).
+        rewrite gset_op_union.
+        rewrite /(ε) in H1_eq. unfold ucmra_unit in H1_eq.
+        simpl in H1_eq.
+        assert ((k,T) ∈ set_of_map Cr') as H'.
+        { replace Cr'. apply set_of_map_member.
+          apply lookup_insert. } 
+        clear - H' Cr_sub_H1 Cr_sub_H1'. set_solver.
+        exfalso. clear -H1_eq. set_solver. }
+      (** Re-establish history_init **)   
+      iAssert (⌜history_init (H1 ∪ {[(k, T)]})⌝)%I with "[Hist]" as "Hist".
+      { iDestruct "Hist" as %Hist.
+        unfold history_init. iPureIntro.
+        clear -Hist k_in_KS. intros k' Hk'.
+        pose proof Hist k' Hk' as H'. set_solver. }  
+      iDestruct "HnP_C" as "_".  
+      iDestruct "HH" as "(HH & HnP_C)".   
+      iAssert (⌜r ∈ domm I1⌝)%I as %r_in_I.
+      { by iPoseProof (inFP_domm _ _ _ with "[$FP_r] [$Hf]") as "H'". }
+      rewrite (big_sepS_delete _ (domm I1) r); last by eauto.
+      iDestruct "Hstar" as "(H_r & Hstar')".
+      iDestruct "H_r" as (br Cr'' Br'' Qr'')"(Hl_r & Hlif_r & HnS_r)".
+      iAssert (⌜br = true⌝)%I as %Hbr.
+      { destruct br; try done.
+        iDestruct "Hlif_r" as 
+            (γ_er' γ_cr' γ_br' γ_qr' γ_cirr' es' T')"(node' & _)".
+        iPoseProof ((node_sep_star r r) with "[$]") as "%".
+        contradiction. } replace br.
+      iDestruct "HnS_r" as (γ_er' γ_cr' γ_br' γ_qr' γ_cirr' es' Ir Rr) 
+                    "(HnS_gh & HnS_frac & HnS_si & HnS_FP 
+                              & HnS_cl & HnS_oc & HnS_if & HnS_star & Hφ)".
+      iPoseProof (ghost_heap_sync with "[$HnP_gh] [$HnS_gh]") 
+                                as "(% & % & % & % & %)".
+      subst γ_er'. subst γ_cr'. subst γ_br'. subst γ_qr'. subst γ_cirr'.
+      iPoseProof (frac_eq with "[$HnP_frac] [$HnS_frac]") as "%".
+      destruct H as [Hes [Hc [Hb Hq]]]. 
+      subst es'. subst Cr''. subst Br''. subst Qr''.
+      (** Update contents-in-reach of r **)
+      set (Br' := <[k := T]>Br).
+      assert (Br' = <[k := T]>Br) as HBr'. try done.
+      iEval (rewrite decide_True) in "HnS_if".
+      iDestruct "HnS_if" as "(% & %)". 
+      rename H into Br_eq_H1. rename H2 into Infz_Ir.
+      iAssert (⌜Br' = map_of_set (H1 ∪ {[(k, T)]})⌝)%I as %Br'_eq_H1.
+      { iPureIntro.
+        apply map_of_set_insert_eq; try done.
+        intros t. 
+        destruct Max_tsH1 as [Max_tsH1 _].
+        by pose proof Max_tsH1 k t. }
+      iEval (rewrite (big_sepS_delete (_) (KS) k); last by eauto) in "HnS_star".
+      iDestruct "HnS_star" as "(Hk & HnS_star')".
+      iAssert (⌜Br !!! k ≤ T⌝)%I as %Br_le_T. 
+      { iDestruct "Hφ" as "(_&_&_&_&_&_&%&_)".
+        iPureIntro. rename H into H'.
+        by pose proof H' k k_in_KS. }
+      iMod (own_update (γ_cirr !!! k) (● (MaxNat (Br !!! k))) 
+                (● (MaxNat (Br' !!! k))) with "Hk") as "Hk".
+      { apply (auth_update_auth _ _ (MaxNat (Br' !!! k))).
+        apply max_nat_local_update.
+        simpl. rewrite HBr'.
+        by rewrite lookup_total_insert. }        
+      iAssert ([∗ set] k0 ∈ KS, own (γ_cirr !!! k0) 
+                  (● {| max_nat_car := Br' !!! k0 |}))%I 
+          with "[HnS_star' Hk]" as "HnS_star".
+      { iEval (rewrite (big_sepS_delete (_) (KS) k); last by eauto).
+        iFrame "Hk".        
+        iApply (big_opS_proper 
+             (λ y, own (γ_cirr !!! y) (● {| max_nat_car := Br' !!! y |}))
+             (λ y, own (γ_cirr !!! y) (● {| max_nat_car := Br !!! y |})) 
+             (KS ∖ {[k]})).
+        intros x Hx. assert (x ≠ k) as H' by set_solver.
+        iFrame. iSplit. 
+        iIntros "H". iEval (rewrite HBr') in "H".
+        assert (<[k:=T]> Br !!! x = Br !!! x) as H''. 
+        { apply lookup_total_insert_ne; try done. } 
+        by iEval (rewrite H'') in "H".       
+        iIntros "H". iEval (rewrite HBr').
+        assert (<[k:=T]> Br !!! x = Br !!! x) as H''. 
+        { apply lookup_total_insert_ne; try done. } 
+        by iEval (rewrite H'').
+        done. }
+      iMod ((frac_update γ_er γ_cr γ_br γ_qr es Cr Br Qr es Cr' Br' Qr) 
+                  with "[$HnP_frac $HnS_frac]") as "(HnP_frac & HnS_frac)".
+      iDestruct "Inf_R" as %Inf_R.
+      iPoseProof ((auth_own_incl γ_R R1 Rr) with "[HR HnS_si]")
+                                    as (Ro) "%". 
+      { unfold singleton_interfaces_ghost_state.
+        iDestruct "HnS_si" as "(_ & H' & _)". 
+        iFrame. } rename H into Incl_R1.
+      iPoseProof (own_valid with "HR") as "%".
+      rename H into Valid_R1.
+      iAssert (⌜domm Rr = {[r]}⌝)%I as "%".
+      { by iDestruct "HnS_si" as "(_&_&_&H')". }
+      rename H into Domm_Rr.
+      iAssert (⌜φ0 es Qr⌝ ∗ ⌜φ1 Br' Cr' Qr⌝ ∗ ⌜φ2 r Br' Ir⌝ 
+        ∗ ⌜φ3 r Br' Rr⌝ ∗ ⌜φ4 r Rr⌝ ∗ ⌜φ5 Br' Qr⌝ 
+        ∗ ⌜φ6 Br' (T+1)⌝ ∗ ⌜φ7 r es Rr Qr⌝ ∗ ⌜φ8 r Ir⌝)%I 
+            with "[Hφ]" as "Hφ".
+      { iDestruct "Hφ" as %Hφ. 
+        destruct Hφ as [Hφ0 [Hφ1 [Hφ2 [Hφ3 [Hφ4 [Hφ5 [Hφ6 [Hφ7 Hφ8]]]]]]]].
+        iPureIntro. repeat split; try done.
+        - destruct (decide (k0 = k)).
+          + subst k0. subst Cr' Br'.
+            rewrite !lookup_insert. try done.
+          + subst Cr' Br'. 
+            rewrite !lookup_insert_ne; try done.
+            by pose proof Hφ1 k0 as [H' _].
+        - destruct (decide (k0 = k)).
+          + subst k0. subst Cr' Br'.
+            rewrite !lookup_insert.
+            destruct Max_tsH1 as [_ H'].
+            intros H''; inversion H''.
+          + subst Cr' Br'. 
+            rewrite !lookup_insert_ne; try done.
+            by pose proof Hφ1 k0 as [_ H'].
+        - intros k' t' HKS Hins.
+          pose proof Infz_Ir r as Infz_Ir.
+          rewrite Infz_Ir in Hins.
+          exfalso. clear -Hins. set_solver.
+        - intros k' HKS. right.
+          apply (inset_monotone R1 Rr Ro); try done.
+          by rewrite <-auth_auth_valid.
+          pose proof Inf_R r k' HKS as Inf_R.
+          by rewrite decide_True in Inf_R.
+          rewrite Domm_Rr. clear. set_solver.
+        - intros k' HKS. subst Br'. destruct (decide (k' = k)).
+          + subst k'. rewrite lookup_total_insert.
+            apply (Nat.le_trans _ (Br !!! k) _); try done.
+            apply Hφ5; try done.
+          + rewrite lookup_total_insert_ne; try done.
+            apply Hφ5; try done.    
+        - intros k' HKS. destruct (decide (k' = k)).
+          + subst k' Br'. rewrite lookup_total_insert; lia.
+          + subst Br'. rewrite lookup_total_insert_ne; try done.
+            pose proof Hφ6 k' HKS. clear -H. 
+            apply (Nat.le_trans _ T _); try done. lia. }
+      (** Linearization **)    
+      iMod "AU" as (t' H')"[MCS [_ Hclose]]".
+      iAssert (⌜t' = T⌝)%I as %Ht'. 
+      { iPoseProof ((auth_agree γ_te) with "[MCS_auth] [MCS]") as "%".
+        unfold MCS_auth. by iDestruct "MCS_auth" as "(H' & _)".
+        by iDestruct "MCS" as "(H' & _)".
+        by iPureIntro. } replace t'.
+      iAssert (⌜H' = H1⌝)%I as %H1'.
+      { iPoseProof ((auth_agree' γ_he) with "[MCS_auth] [MCS]") as "%".
+        unfold MCS_auth. by iDestruct "MCS_auth" as "(_ & H'')".
+        by iDestruct "MCS" as "(_ & H')".
+        by iPureIntro. } replace H'.
+      iDestruct "MCS" as "(MCS◯t & MCS◯h)".
+      iDestruct "MCS_auth" as "(MCS●t & MCS●h)".
+      iMod ((auth_excl_update γ_te (T+1) T T) with "MCS●t MCS◯t") 
+                                          as "(MCS●t & MCS◯t)".
+      iMod ((auth_excl_update γ_he (H1 ∪ {[(k, T)]}) H1 H1) with "MCS●h MCS◯h") 
+                                          as "(MCS●h & MCS◯h)".
+      iCombine "MCS◯t MCS◯h" as "MCS".
+      iCombine "MCS●t MCS●h" as "MCS_auth".
+      iMod ("Hclose" with "MCS") as "HΦ".
+      
+      iModIntro.
+      iSplitR "HΦ node_r HnP_gh HnP_t HnP_C HnP_frac".
+      { iNext. iExists (T+1), (H1 ∪ {[(k, T)]}), hγ1, I1, R1.
+        iFrame "∗ %".   
+        rewrite (big_sepS_delete _ (domm I1) r); last by eauto.
+        iSplitR "Hstar'".
+        { iExists true, Cr', Br', Qr. iFrame.
+          iExists γ_er, γ_cr, γ_br, γ_qr, γ_cirr, es, Ir, Rr.
+          iFrame "∗#". iEval (rewrite decide_True). 
+          iFrame "%∗". }        
+        iApply (big_sepS_mono 
+                  (λ y, ∃ (bn : bool) (Cn Bn Qn : gmap K natUR),
+                          general_multicopy.lockLoc y ↦ #bn
+                        ∗ (if bn then True
+                           else nodePred γ_gh γ_t γ_s lc r y Cn Bn Qn)
+                        ∗ nodeShared γ_I γ_R γ_f γ_gh r y Cn Bn Qn H1 T )%I
+                  (λ y, ∃ (bn : bool) (Cn Bn Qn : gmap K natUR),
+                          general_multicopy.lockLoc y ↦ #bn
+                        ∗ (if bn then True
+                           else nodePred γ_gh γ_t γ_s lc r y Cn Bn Qn)
+                        ∗ nodeShared γ_I γ_R γ_f γ_gh r y Cn Bn Qn 
+                                                (H1 ∪ {[(k, T)]}) (T + 1))%I
+                  (domm I1 ∖ {[r]})); try done.
+        intros y y_dom. assert (y ≠ r) as Hy by set_solver. iFrame.
+        iIntros "Hstar". iDestruct "Hstar" as (b C B Q)"(Hl & Hlif & HnS)".
+        iExists b, C, B, Q. iFrame. 
+        iDestruct "HnS" as (γ_e γ_c γ_b γ_q γ_cir esy Iy Ry)
+                    "(HnS_gh & domm_γcir & HnS_frac & HnS_si & HnS_FP 
+                              & HnS_cl & HnS_oc & HnS_if & HnS_star 
+                              & Hφ0 & Hφ1 & Hφ2 & Hφ3 & Hφ4 & Hφ6 & Hφ7)".
+        iExists γ_e, γ_c, γ_b, γ_q, γ_cir, esy, Iy, Ry. iFrame.
+        iDestruct "Hφ6" as %Hφ6.
+        destruct (decide (y = r)); try done. 
+        iPureIntro. split; try done.
+        intros k' HKS. pose proof Hφ6 k' HKS. 
+        apply (Nat.le_trans _ T _); try done. lia. } 
+      wp_pures. 
+      (** Unlock node r **) 
+      awp_apply (unlockNode_spec_high with "[] [] 
+        [HnP_gh HnP_t HnP_C HnP_frac node_r]") without "HΦ"; try done. 
+      iExists γ_er, γ_cr, γ_br, γ_qr, γ_cirr, es, (T + 1).
+      iFrame. by iEval (rewrite decide_True).
+      iAaccIntro with ""; try done.
+      iIntros "_". iModIntro; iIntros "HΦ"; try done.
+      Unshelve. try done.
+  Qed.      
+
+End upsert_proof.
